<?xml version="1.0"?>
<rdf:RDF xmlns="http://ontology.mayo.edu/ontology/KAO/"
     xml:base="http://ontology.mayo.edu/ontology/KAO/"
     xmlns:rdf="http://www.w3.org/1999/02/22-rdf-syntax-ns#"
     xmlns:terms="http://purl.org/dc/terms/"
     xmlns:owl="http://www.w3.org/2002/07/owl#"
     xmlns:xml="http://www.w3.org/XML/1998/namespace"
     xmlns:kao="http://ontology.mayo.edu/ontology/KAO/"
     xmlns:xsd="http://www.w3.org/2001/XMLSchema#"
     xmlns:skos="http://www.w3.org/2004/02/skos/core#"
     xmlns:rdfs="http://www.w3.org/2000/01/rdf-schema#"
     xmlns:SpecificationMetadata="http://www.omg.org/techprocess/ab/SpecificationMetadata/"
     xmlns:dc="http://purl.org/dc/elements/1.1/"
     xmlns:api4kp="https://www.omg.org/spec/API4KP/api4kp/"
     xmlns:kmdo="http://ontology.mayo.edu/ontologies/20180601/KMDO/">
    <owl:Ontology rdf:about="http://ontology.mayo.edu/ontology/KAO/">
        <owl:versionIRI rdf:resource="http://ontology.mayo.edu/ontology/KAO/1.0"/>
        <owl:imports rdf:resource="https://www.omg.org/spec/API4KP/20190801/api4kp/"/>
        <owl:imports rdf:resource="http://ontology.mayo.edu/ontologies/20180601/KMDO/"/>
        <owl:imports rdf:resource="http://www.w3.org/2004/02/skos/core"/>
        <terms:creator>Davide Sottara (sottara.davide@mayo.edu)</terms:creator>
        <dc:title>Knowledge Asset Ontology</dc:title>
        <dc:description>An ontology of the Mayo Clinic KM endorsed categories and types of (Clinical) &apos;Knowledge Assets&apos;</dc:description>
    </owl:Ontology>
    


    <!-- 
    ///////////////////////////////////////////////////////////////////////////////////////
    //
    // Annotation properties
    //
    ///////////////////////////////////////////////////////////////////////////////////////
     -->

    


    <!-- http://www.w3.org/2004/02/skos/core#notation -->

    <owl:AnnotationProperty rdf:about="http://www.w3.org/2004/02/skos/core#notation"/>
    


    <!-- 
    ///////////////////////////////////////////////////////////////////////////////////////
    //
    // Object Properties
    //
    ///////////////////////////////////////////////////////////////////////////////////////
     -->

    


    <!-- https://www.omg.org/spec/API4KP/api4kp/defines -->

    <owl:ObjectProperty rdf:about="https://www.omg.org/spec/API4KP/api4kp/defines"/>
    


    <!-- https://www.omg.org/spec/API4KP/api4kp/has-part -->

    <owl:ObjectProperty rdf:about="https://www.omg.org/spec/API4KP/api4kp/has-part"/>
    


    <!-- https://www.omg.org/spec/API4KP/api4kp/part-of -->

    <owl:ObjectProperty rdf:about="https://www.omg.org/spec/API4KP/api4kp/part-of"/>
    


    <!-- https://www.omg.org/spec/API4KP/api4kp/uses-concept -->

    <owl:ObjectProperty rdf:about="https://www.omg.org/spec/API4KP/api4kp/uses-concept"/>
    


    <!-- 
    ///////////////////////////////////////////////////////////////////////////////////////
    //
    // Classes
    //
    ///////////////////////////////////////////////////////////////////////////////////////
     -->

    


    <!-- http://ontology.mayo.edu/ontologies/20180601/KMDO/DomainSpecificWorkOfKnowledge -->

    <owl:Class rdf:about="http://ontology.mayo.edu/ontologies/20180601/KMDO/DomainSpecificWorkOfKnowledge"/>
    


    <!-- http://ontology.mayo.edu/ontology/KAO/AnnotationLanguage -->

    <owl:Class rdf:about="http://ontology.mayo.edu/ontology/KAO/AnnotationLanguage">
        <rdfs:subClassOf rdf:resource="http://ontology.mayo.edu/ontology/KAO/DedicatedLanguage"/>
        <rdfs:label>annotation language</rdfs:label>
        <skos:definition>language used to express &quot;meta&quot; knowledge</skos:definition>
    </owl:Class>
    


    <!-- http://ontology.mayo.edu/ontology/KAO/AssessmentModel -->

    <owl:Class rdf:about="http://ontology.mayo.edu/ontology/KAO/AssessmentModel">
        <rdfs:subClassOf rdf:resource="http://ontology.mayo.edu/ontology/KAO/InferentialAsset"/>
        <rdfs:comment>knowledge that allows to infer an otherwise unknown or not directly observable state or situation</rdfs:comment>
        <rdfs:label>Assessment Model</rdfs:label>
    </owl:Class>
    


    <!-- http://ontology.mayo.edu/ontology/KAO/BusinessRuleAsset -->

    <owl:Class rdf:about="http://ontology.mayo.edu/ontology/KAO/BusinessRuleAsset">
        <rdfs:subClassOf rdf:resource="http://ontology.mayo.edu/ontology/KAO/CategorizedKnowledgeAsset"/>
        <rdfs:comment>Assets in this category describe or specify how to limit an agent&apos;s degree of freedom, to prevent undesirable behaviors, in favor of more desirable ones.</rdfs:comment>
        <rdfs:comment>At its essence, knowledge of this kind is expressed using &quot;IF..DO..&quot; rules, usually by means of constraint-oriented languages with ECA and/or deontic aspects</rdfs:comment>
        <rdfs:label>Rule-Oriented Knowledge Asset</rdfs:label>
        <skos:definition>Knowledge about the social, organizational and behavioral aspects of how business is (not) required, expected or permitted to be conducted, as determined by some party that has jurisdiction over an environment.</skos:definition>
        <skos:prefLabel>Rules, Policies and Guidelines</skos:prefLabel>
        <skos:scopeNote>Business rules are deontic in nature, whereas alethic rules are considered inferential models.</skos:scopeNote>
    </owl:Class>
    


    <!-- http://ontology.mayo.edu/ontology/KAO/CareProcessModel -->

    <owl:Class rdf:about="http://ontology.mayo.edu/ontology/KAO/CareProcessModel">
        <rdfs:subClassOf rdf:resource="http://ontology.mayo.edu/ontology/KAO/ClinicalKnowledgeAsset"/>
        <rdfs:subClassOf rdf:resource="http://ontology.mayo.edu/ontology/KAO/ProcessAsset"/>
        <rdfs:comment>Adaptive specification of how to perform (complex) clinical activities, properly orchestrated over time, so to achieve certain objectives and goals</rdfs:comment>
        <rdfs:isDefinedBy rdf:resource="http://ontology.mayo.edu/ontology/KAO"/>
        <rdfs:label xml:lang="en">Care Process Model</rdfs:label>
        <skos:altLabel xml:lang="en">CPM</skos:altLabel>
        <skos:example xml:lang="en">The Mayo Clinic Rectal Adenocarcinoma CPM</skos:example>
        <skos:scopeNote xml:lang="en">Includes AME Care Process Models (CPM)</skos:scopeNote>
    </owl:Class>
    <owl:Axiom>
        <owl:annotatedSource rdf:resource="http://ontology.mayo.edu/ontology/KAO/CareProcessModel"/>
        <owl:annotatedProperty rdf:resource="http://www.w3.org/2004/02/skos/core#example"/>
        <owl:annotatedTarget xml:lang="en">The Mayo Clinic Rectal Adenocarcinoma CPM</owl:annotatedTarget>
        <rdfs:seeAlso rdf:resource="https://clinicalknowledgemanagement.mayo.edu/topic/clinical-answers/CNT-20141231/CPM-20211573"/>
    </owl:Axiom>
    


    <!-- http://ontology.mayo.edu/ontology/KAO/CategorizedKnowledgeAsset -->

    <owl:Class rdf:about="http://ontology.mayo.edu/ontology/KAO/CategorizedKnowledgeAsset">
        <rdfs:subClassOf rdf:resource="https://www.omg.org/spec/API4KP/api4kp/KnowledgeAsset"/>
    </owl:Class>
    


    <!-- http://ontology.mayo.edu/ontology/KAO/ClinicalKnowledgeAsset -->

    <owl:Class rdf:about="http://ontology.mayo.edu/ontology/KAO/ClinicalKnowledgeAsset">
        <rdfs:subClassOf rdf:resource="http://ontology.mayo.edu/ontology/KAO/DomainSpecificKnowledgeAsset"/>
        <rdfs:label>clinical knowledge asset</rdfs:label>
        <skos:definition>knowledge asset that uses primarily concepts from the clinical business domain</skos:definition>
    </owl:Class>
    


    <!-- http://ontology.mayo.edu/ontology/KAO/ClinicalPracticeGuideline -->

    <owl:Class rdf:about="http://ontology.mayo.edu/ontology/KAO/ClinicalPracticeGuideline">
        <rdfs:subClassOf rdf:resource="http://ontology.mayo.edu/ontology/KAO/BusinessRuleAsset"/>
        <rdfs:subClassOf rdf:resource="http://ontology.mayo.edu/ontology/KAO/ClinicalKnowledgeAsset"/>
        <rdfs:comment xml:lang="en">Systematically developed statements to assist provider decisions about appropriate healthcare for specific clinical situations</rdfs:comment>
        <rdfs:isDefinedBy rdf:resource="http://ontology.mayo.edu/ontology/KAO"/>
        <rdfs:label xml:lang="en">Clinical Practice Guideline</rdfs:label>
        <skos:altLabel xml:lang="en">Clinical Practice Guideline</skos:altLabel>
        <skos:example xml:lang="en">The Mayo Clinic Sternotomy Guideline</skos:example>
    </owl:Class>
    <owl:Axiom>
        <owl:annotatedSource rdf:resource="http://ontology.mayo.edu/ontology/KAO/ClinicalPracticeGuideline"/>
        <owl:annotatedProperty rdf:resource="http://www.w3.org/2004/02/skos/core#example"/>
        <owl:annotatedTarget xml:lang="en">The Mayo Clinic Sternotomy Guideline</owl:annotatedTarget>
        <rdfs:seeAlso rdf:resource="http://mayoweb.mayo.edu/pmr/documents/PracticeGuidelineTemplateSternotomy.pdf"/>
    </owl:Axiom>
    


    <!-- http://ontology.mayo.edu/ontology/KAO/ClinicalRule -->

    <owl:Class rdf:about="http://ontology.mayo.edu/ontology/KAO/ClinicalRule">
        <rdfs:subClassOf rdf:resource="http://ontology.mayo.edu/ontology/KAO/BusinessRuleAsset"/>
        <rdfs:comment xml:lang="en">Computational logic to direct clinical interventions that is typically expressed as if/then statements but may also be represented by a diagram, decision table or other representation language</rdfs:comment>
        <rdfs:isDefinedBy rdf:resource="http://ontology.mayo.edu/ontology/KAO"/>
        <rdfs:label xml:lang="en">Clinical Business Rule</rdfs:label>
        <skos:altLabel xml:lang="en">CDS Rule</skos:altLabel>
        <skos:example xml:lang="en">The &apos;HGB value prior to RBC transfusion&apos; Recommendation Rule</skos:example>
        <skos:prefLabel xml:lang="en">Clinical Rule</skos:prefLabel>
    </owl:Class>
    <owl:Axiom>
        <owl:annotatedSource rdf:resource="http://ontology.mayo.edu/ontology/KAO/ClinicalRule"/>
        <owl:annotatedProperty rdf:resource="http://www.w3.org/2004/02/skos/core#example"/>
        <owl:annotatedTarget xml:lang="en">The &apos;HGB value prior to RBC transfusion&apos; Recommendation Rule</owl:annotatedTarget>
        <rdfs:seeAlso rdf:resource="https://clinicalknowledgemanagement.mayo.edu/mayo-clinic-rules-catalog/asset/km-asset/KAT-20323041"/>
    </owl:Axiom>
    


    <!-- http://ontology.mayo.edu/ontology/KAO/CognitiveCareProcessModel -->

    <owl:Class rdf:about="http://ontology.mayo.edu/ontology/KAO/CognitiveCareProcessModel">
        <rdfs:subClassOf rdf:resource="http://ontology.mayo.edu/ontology/KAO/CareProcessModel"/>
        <rdfs:subClassOf rdf:resource="http://ontology.mayo.edu/ontology/KAO/CognitiveProcessModel"/>
        <rdfs:comment>Knowledge whose primary subject is the cognitive aspects of a Care Process</rdfs:comment>
        <rdfs:label>Cognitive Care Process Model</rdfs:label>
    </owl:Class>
    


    <!-- http://ontology.mayo.edu/ontology/KAO/CognitiveProcessModel -->

    <owl:Class rdf:about="http://ontology.mayo.edu/ontology/KAO/CognitiveProcessModel">
        <rdfs:subClassOf rdf:resource="http://ontology.mayo.edu/ontology/KAO/ProcessAsset"/>
        <rdfs:subClassOf>
            <owl:Restriction>
                <owl:onProperty rdf:resource="https://www.omg.org/spec/API4KP/api4kp/has-part"/>
                <owl:someValuesFrom rdf:resource="http://ontology.mayo.edu/ontology/KAO/DecisionModel"/>
            </owl:Restriction>
        </rdfs:subClassOf>
        <rdfs:comment>Knowledge Asset that captures how information is processed internally by an intelligent agent</rdfs:comment>
        <rdfs:label>Cognitive Process Model</rdfs:label>
    </owl:Class>
    


    <!-- http://ontology.mayo.edu/ontology/KAO/CohortDefinition -->

    <owl:Class rdf:about="http://ontology.mayo.edu/ontology/KAO/CohortDefinition">
        <rdfs:subClassOf rdf:resource="http://ontology.mayo.edu/ontology/KAO/InferentialAsset"/>
        <rdfs:comment>Definition used to classify persons into classes defined by some common characteristic</rdfs:comment>
        <rdfs:label>Cohort Definition</rdfs:label>
    </owl:Class>
    


    <!-- http://ontology.mayo.edu/ontology/KAO/ComponentKnowledgeAsset -->

    <owl:Class rdf:about="http://ontology.mayo.edu/ontology/KAO/ComponentKnowledgeAsset">
        <rdfs:subClassOf rdf:resource="http://ontology.mayo.edu/ontology/KAO/ExplicitRoleKnowledgeAsset"/>
        <rdfs:label>Component Knowledge Asset</rdfs:label>
        <skos:definition>Knowledge Asset that is part of some other (Composite) Knowledge Asset. The component may play a specific role within the broader Composite Asset</skos:definition>
    </owl:Class>
    


    <!-- http://ontology.mayo.edu/ontology/KAO/CompositeKnowledgeAsset -->

    <owl:Class rdf:about="http://ontology.mayo.edu/ontology/KAO/CompositeKnowledgeAsset">
        <rdfs:subClassOf rdf:resource="http://ontology.mayo.edu/ontology/KAO/ExplicitRoleKnowledgeAsset"/>
        <rdfs:subClassOf rdf:resource="https://www.omg.org/spec/API4KP/api4kp/CompositeKnowledgeResource"/>
        <rdfs:label>Composite Knowledge Asset</rdfs:label>
        <skos:definition>Knowledge Asset that has part some other Knowledge Asset</skos:definition>
    </owl:Class>
    


    <!-- http://ontology.mayo.edu/ontology/KAO/ComputableDecisionModel -->

    <owl:Class rdf:about="http://ontology.mayo.edu/ontology/KAO/ComputableDecisionModel">
        <rdfs:subClassOf rdf:resource="http://ontology.mayo.edu/ontology/KAO/DecisionModel"/>
        <rdfs:comment>Decision Model that includes an explicit specification of its decision making logic, suitable to be faithfully expressed in a computable language</rdfs:comment>
        <rdfs:label>Computable Decision Model</rdfs:label>
    </owl:Class>
    


    <!-- http://ontology.mayo.edu/ontology/KAO/ComputationalTechnique -->

    <owl:Class rdf:about="http://ontology.mayo.edu/ontology/KAO/ComputationalTechnique">
        <rdfs:subClassOf rdf:resource="https://www.omg.org/spec/API4KP/api4kp/KnowledgeProcessingTechnique"/>
        <owl:disjointWith rdf:resource="http://ontology.mayo.edu/ontology/KAO/NaturalisticTechnique"/>
        <rdfs:label>computational technique</rdfs:label>
        <skos:definition>Technique used in some knowledge processing task method specification that can be faithfully expressed in some machine-computable language</skos:definition>
    </owl:Class>
    


    <!-- http://ontology.mayo.edu/ontology/KAO/ConceptualModel -->

    <owl:Class rdf:about="http://ontology.mayo.edu/ontology/KAO/ConceptualModel">
        <rdfs:subClassOf rdf:resource="http://ontology.mayo.edu/ontology/KAO/SemanticAsset"/>
        <rdfs:comment>Abstraction of the structure and/or behavior of the entities in a given domain</rdfs:comment>
        <rdfs:label>Conceptual (Domain) Model</rdfs:label>
        <skos:altLabel>domain conceptualization</skos:altLabel>
    </owl:Class>
    


    <!-- http://ontology.mayo.edu/ontology/KAO/ContextualizabledKnowledge -->

    <owl:Class rdf:about="http://ontology.mayo.edu/ontology/KAO/ContextualizabledKnowledge">
        <rdfs:subClassOf rdf:resource="http://ontology.mayo.edu/ontology/KAO/ConceptualModel"/>
        <rdfs:comment>Conceptual Work of Knowledge that has been adapted for a given context</rdfs:comment>
        <rdfs:label>Contextualizable Knowledge</rdfs:label>
    </owl:Class>
    


    <!-- http://ontology.mayo.edu/ontology/KAO/DecisionMakingTask -->

    <owl:Class rdf:about="http://ontology.mayo.edu/ontology/KAO/DecisionMakingTask">
        <rdfs:subClassOf rdf:resource="https://www.omg.org/spec/API4KP/api4kp/InformationProcessingTask"/>
        <rdfs:label>decision making task</rdfs:label>
    </owl:Class>
    


    <!-- http://ontology.mayo.edu/ontology/KAO/DecisionModel -->

    <owl:Class rdf:about="http://ontology.mayo.edu/ontology/KAO/DecisionModel">
        <rdfs:subClassOf rdf:resource="http://ontology.mayo.edu/ontology/KAO/AssessmentModel"/>
        <rdfs:comment>Assessment that can be abstracted by means of a question, which requires to select one out of a set of admissible options</rdfs:comment>
        <rdfs:label>Decision Model</rdfs:label>
    </owl:Class>
    


    <!-- http://ontology.mayo.edu/ontology/KAO/DecisionTaskModel -->

    <owl:Class rdf:about="http://ontology.mayo.edu/ontology/KAO/DecisionTaskModel">
        <rdfs:subClassOf rdf:resource="http://ontology.mayo.edu/ontology/KAO/CognitiveProcessModel"/>
        <rdfs:subClassOf>
            <owl:Restriction>
                <owl:onProperty rdf:resource="https://www.omg.org/spec/API4KP/api4kp/defines"/>
                <owl:someValuesFrom rdf:resource="http://ontology.mayo.edu/ontology/KAO/DecisionMakingTask"/>
            </owl:Restriction>
        </rdfs:subClassOf>
        <rdfs:subClassOf>
            <owl:Restriction>
                <owl:onProperty rdf:resource="https://www.omg.org/spec/API4KP/api4kp/part-of"/>
                <owl:someValuesFrom rdf:resource="http://ontology.mayo.edu/ontology/KAO/CognitiveProcessModel"/>
            </owl:Restriction>
        </rdfs:subClassOf>
        <rdfs:comment>Model of who, when, where and why a Decision is made, usually as part of a broader process. Also known as Decision Making Process Model, usually includes a Decision Model that specifies how to actually choose the optimal option</rdfs:comment>
        <rdfs:label>Decision Task Model</rdfs:label>
    </owl:Class>
    


    <!-- http://ontology.mayo.edu/ontology/KAO/DedicatedLanguage -->

    <owl:Class rdf:about="http://ontology.mayo.edu/ontology/KAO/DedicatedLanguage">
        <rdfs:subClassOf rdf:resource="https://www.omg.org/spec/API4KP/api4kp/ConstructedLanguage"/>
        <rdfs:label>Dedicated Language</rdfs:label>
        <skos:definition>Language that has been designed specifically, and thus can be used, to faithfully express certain categories of works of knowledge, i.e. language that is known to provide constructs for some of the concepts that are expected (implied) by the type of knowledge being expressed</skos:definition>
        <skos:editorialNote>Need a better term than &quot;Dedicated&quot;?
&quot;Committed&quot; is an option, but seems too strong, e.g. see Ontologically Committed Language</skos:editorialNote>
    </owl:Class>
    


    <!-- http://ontology.mayo.edu/ontology/KAO/DocumentationTemplate -->

    <owl:Class rdf:about="http://ontology.mayo.edu/ontology/KAO/DocumentationTemplate">
        <rdfs:subClassOf rdf:resource="http://ontology.mayo.edu/ontology/KAO/InformationAsset"/>
        <rdfs:comment>An organized collection of determinable concepts, possibly associated to questions, which are meant to be resolved in a particular context</rdfs:comment>
        <rdfs:label>Documentation Template</rdfs:label>
        <skos:scopeNote>more general than questionnaires, whose questions are meant to be answered by a human agent (possibly with computer aid), documentation templates can be used  by software agents as well</skos:scopeNote>
    </owl:Class>
    


    <!-- http://ontology.mayo.edu/ontology/KAO/DomainSpecificKnowledgeAsset -->

    <owl:Class rdf:about="http://ontology.mayo.edu/ontology/KAO/DomainSpecificKnowledgeAsset">
        <rdfs:subClassOf rdf:resource="http://ontology.mayo.edu/ontologies/20180601/KMDO/DomainSpecificWorkOfKnowledge"/>
        <rdfs:subClassOf rdf:resource="https://www.omg.org/spec/API4KP/api4kp/KnowledgeAsset"/>
    </owl:Class>
    


    <!-- http://ontology.mayo.edu/ontology/KAO/Equation -->

    <owl:Class rdf:about="http://ontology.mayo.edu/ontology/KAO/Equation">
        <rdfs:subClassOf rdf:resource="http://ontology.mayo.edu/ontology/KAO/FunctionalExpression"/>
        <rdfs:comment>A functional expression, defined in terms of two functional expressions connected by means of the well known equality operator.</rdfs:comment>
        <rdfs:label>Equation</rdfs:label>
    </owl:Class>
    


    <!-- http://ontology.mayo.edu/ontology/KAO/ExplicitRoleKnowledgeAsset -->

    <owl:Class rdf:about="http://ontology.mayo.edu/ontology/KAO/ExplicitRoleKnowledgeAsset">
        <rdfs:subClassOf rdf:resource="https://www.omg.org/spec/API4KP/api4kp/KnowledgeAsset"/>
        <rdfs:comment>Asset that is necessarily related to some entity, which has a specific type itself</rdfs:comment>
        <rdfs:label>Explicit Role Knowledge Asset</rdfs:label>
    </owl:Class>
    


    <!-- http://ontology.mayo.edu/ontology/KAO/ExpressionLanguage -->

    <owl:Class rdf:about="http://ontology.mayo.edu/ontology/KAO/ExpressionLanguage">
        <rdfs:subClassOf rdf:resource="http://ontology.mayo.edu/ontology/KAO/DedicatedLanguage"/>
        <rdfs:label>expression language</rdfs:label>
        <skos:definition>language used to express functional derivations</skos:definition>
    </owl:Class>
    


    <!-- http://ontology.mayo.edu/ontology/KAO/FactualKnowledg -->

    <owl:Class rdf:about="http://ontology.mayo.edu/ontology/KAO/FactualKnowledg">
        <rdfs:subClassOf rdf:resource="http://ontology.mayo.edu/ontology/KAO/ConceptualModel"/>
        <rdfs:comment>Facts are suitable to be asserted</rdfs:comment>
        <rdfs:comment>Knowledge that is held to be a faithful conceptualization of the state of affairs in a given domain by all agents that share (and understand) it.</rdfs:comment>
        <rdfs:label>Factual Knowledge</rdfs:label>
    </owl:Class>
    


    <!-- http://ontology.mayo.edu/ontology/KAO/FormalOntology -->

    <owl:Class rdf:about="http://ontology.mayo.edu/ontology/KAO/FormalOntology">
        <rdfs:subClassOf rdf:resource="http://ontology.mayo.edu/ontology/KAO/ConceptualModel"/>
        <rdfs:comment>conceptual model that is based on formal principles, such as that allow to make inferences and/or verify the consistency of the model</rdfs:comment>
        <rdfs:label>Formal Ontology</rdfs:label>
    </owl:Class>
    


    <!-- http://ontology.mayo.edu/ontology/KAO/FunctionalExpression -->

    <owl:Class rdf:about="http://ontology.mayo.edu/ontology/KAO/FunctionalExpression">
        <rdfs:subClassOf rdf:resource="http://ontology.mayo.edu/ontology/KAO/AssessmentModel"/>
        <rdfs:comment>Knowledge about the application of well-known information processing methods, possibly chained together, which are stateless, functional and idempotent in nature.</rdfs:comment>
        <rdfs:label>Functional Expression</rdfs:label>
        <skos:example>&apos;mass&apos; times the square of the speed of light</skos:example>
    </owl:Class>
    


    <!-- http://ontology.mayo.edu/ontology/KAO/InferentialAsset -->

    <owl:Class rdf:about="http://ontology.mayo.edu/ontology/KAO/InferentialAsset">
        <rdfs:subClassOf rdf:resource="http://ontology.mayo.edu/ontology/KAO/CategorizedKnowledgeAsset"/>
        <rdfs:subClassOf rdf:resource="https://www.omg.org/spec/API4KP/api4kp/Definition"/>
        <rdfs:comment>When qualitiative, knowledge of this kind can be generally abstracted by means of &quot;if..then..&quot; rules (or analogous formalisms). The quantitative counterpart is expressed by means of mathematical formulas. 

Either way, expressions are expected to be pure, functional and idempotent, even when they handle uncertainty.</rdfs:comment>
        <rdfs:isDefinedBy rdf:resource="http://ontology.mayo.edu/ontology/KAO"/>
        <rdfs:label xml:lang="en">Inference-Oriented Knowledge Asset</rdfs:label>
        <skos:definition>Knowledge about how to assess the current, or predict the future state of a variable, quality or other characteristic of a system (e.g. a patient) which may not be directly observable, but can be estimated on the basis of other more primitive pieces of data.</skos:definition>
        <skos:example>A BMI Calculator</skos:example>
        <skos:example xml:lang="en">A FRAX Fracture Risk Score Calculator</skos:example>
        <skos:example xml:lang="en">A Pain assessment scale</skos:example>
        <skos:example xml:lang="en">The Cockcroft-Gault equation</skos:example>
        <skos:example xml:lang="en">The Scoring Model used to calculate the CHA2DS2-VASc score</skos:example>
        <skos:prefLabel xml:lang="en">Assessment, Predictive and Inferential Models</skos:prefLabel>
        <skos:scopeNote xml:lang="en">This is a broad category that includes e.g.: 
a) Mathematical equations and models used in a clinical or health-related calculation
b) Clinical or health-related scoring formulas for the purposes of predicting or classifying something, often by assigning points based on observations (e.g. stroke risk, asthma severity, mortality); includes information about the required inputs and the interpretation of the resulting score/s  
c) Associations, Correlations and Causal Relationships between phenomena, some of which may not be directly observable</skos:scopeNote>
    </owl:Class>
    <owl:Axiom>
        <owl:annotatedSource rdf:resource="http://ontology.mayo.edu/ontology/KAO/InferentialAsset"/>
        <owl:annotatedProperty rdf:resource="http://www.w3.org/2004/02/skos/core#example"/>
        <owl:annotatedTarget xml:lang="en">The Cockcroft-Gault equation</owl:annotatedTarget>
        <rdfs:seeAlso rdf:resource="https://clinicalknowledgemanagement.mayo.edu/mayo-clinic-rules-catalog/asset/km-asset/KAT-20359526"/>
    </owl:Axiom>
    <owl:Axiom>
        <owl:annotatedSource rdf:resource="http://ontology.mayo.edu/ontology/KAO/InferentialAsset"/>
        <owl:annotatedProperty rdf:resource="http://www.w3.org/2004/02/skos/core#example"/>
        <owl:annotatedTarget xml:lang="en">The Scoring Model used to calculate the CHA2DS2-VASc score</owl:annotatedTarget>
        <rdfs:seeAlso rdf:resource="https://clinicalknowledgemanagement.mayo.edu/mayo-clinic-rules-catalog/asset/km-asset/KAT-20359512"/>
    </owl:Axiom>
    <owl:Axiom>
        <owl:annotatedSource rdf:resource="http://ontology.mayo.edu/ontology/KAO/InferentialAsset"/>
        <owl:annotatedProperty rdf:resource="http://www.w3.org/2004/02/skos/core#example"/>
        <owl:annotatedTarget>A BMI Calculator</owl:annotatedTarget>
        <rdfs:seeAlso rdf:resource="https://clinicalknowledgemanagement.mayo.edu/mayo-clinic-rules-catalog/asset/assessment-tool/LNK-20146551"/>
    </owl:Axiom>
    <owl:Axiom>
        <owl:annotatedSource rdf:resource="http://ontology.mayo.edu/ontology/KAO/InferentialAsset"/>
        <owl:annotatedProperty rdf:resource="http://www.w3.org/2004/02/skos/core#example"/>
        <owl:annotatedTarget xml:lang="en">A FRAX Fracture Risk Score Calculator</owl:annotatedTarget>
        <rdfs:seeAlso rdf:resource="https://clinicalknowledgemanagement.mayo.edu/mayo-clinic-rules-catalog/asset/assessment-tool/LNK-20147628"/>
    </owl:Axiom>
    <owl:Axiom>
        <owl:annotatedSource rdf:resource="http://ontology.mayo.edu/ontology/KAO/InferentialAsset"/>
        <owl:annotatedProperty rdf:resource="http://www.w3.org/2004/02/skos/core#example"/>
        <owl:annotatedTarget xml:lang="en">A Pain assessment scale</owl:annotatedTarget>
        <rdfs:seeAlso rdf:resource="https://clinicalknowledgemanagement.mayo.edu/mayo-clinic-rules-catalog/asset/km-asset/KAT-20381849"/>
    </owl:Axiom>
    


    <!-- http://ontology.mayo.edu/ontology/KAO/InformationAsset -->

    <owl:Class rdf:about="http://ontology.mayo.edu/ontology/KAO/InformationAsset">
        <rdfs:subClassOf rdf:resource="http://ontology.mayo.edu/ontology/KAO/CategorizedKnowledgeAsset"/>
        <rdfs:label>Information-Oriented Knowledge Asset</rdfs:label>
        <skos:definition>Knowledge about how to acquire, represent, organize, store and distribute data, about some domain of interest, using structured formats.</skos:definition>
        <skos:example>A logical information model for the documentation of a Blood Pressure test panel, such that it could be expressed by means of a CIMI model</skos:example>
        <skos:example>A pediatric documentation template, such that it could be manifested in a digital, interactive, form-based data acquisition tool</skos:example>
        <skos:prefLabel>Structured Information and Data Capture Models</skos:prefLabel>
        <skos:scopeNote>Notice that conceptual models of the domain, as opposed to logical models of information about the domain, are categorized under &quot;Terminology, Ontology and Assertional KBs&quot;.</skos:scopeNote>
        <skos:scopeNote>This category includes assets whose manifestations are meant to be used during the entire lifecycle, including documentation templates and questionnaires (acquisition), as well as logical information models and schemas (storage) and messaging models used for data sharing and interoperability.</skos:scopeNote>
    </owl:Class>
    <owl:Axiom>
        <owl:annotatedSource rdf:resource="http://ontology.mayo.edu/ontology/KAO/InformationAsset"/>
        <owl:annotatedProperty rdf:resource="http://www.w3.org/2004/02/skos/core#example"/>
        <owl:annotatedTarget>A logical information model for the documentation of a Blood Pressure test panel, such that it could be expressed by means of a CIMI model</owl:annotatedTarget>
        <rdfs:seeAlso rdf:resource="http://www.clinicalelement.com/cimi-browser/#/20180124/CIMI/CIMI-CORE-CompoundClinicalStatement.blood_pressure_panel.v1.0.0"/>
    </owl:Axiom>
    <owl:Axiom>
        <owl:annotatedSource rdf:resource="http://ontology.mayo.edu/ontology/KAO/InformationAsset"/>
        <owl:annotatedProperty rdf:resource="http://www.w3.org/2004/02/skos/core#example"/>
        <owl:annotatedTarget>A pediatric documentation template, such that it could be manifested in a digital, interactive, form-based data acquisition tool</owl:annotatedTarget>
        <rdfs:seeAlso>https://healthit.ahrq.gov/health-it-tools-and-resources/pediatric-resources/pediatric-documentation-templates/pediatric-asthma-template</rdfs:seeAlso>
    </owl:Axiom>
    


    <!-- http://ontology.mayo.edu/ontology/KAO/InformationModel -->

    <owl:Class rdf:about="http://ontology.mayo.edu/ontology/KAO/InformationModel">
        <rdfs:subClassOf rdf:resource="http://ontology.mayo.edu/ontology/KAO/InformationAsset"/>
        <rdfs:comment>(Meta) model that defines which information should be captured about some kind of domain</rdfs:comment>
        <rdfs:label>Information Model</rdfs:label>
        <skos:altLabel>logical data model</skos:altLabel>
    </owl:Class>
    


    <!-- http://ontology.mayo.edu/ontology/KAO/InquirySpecification -->

    <owl:Class rdf:about="http://ontology.mayo.edu/ontology/KAO/InquirySpecification">
        <rdfs:subClassOf rdf:resource="http://ontology.mayo.edu/ontology/KAO/ProcessAsset"/>
        <rdfs:comment>The definition of how (and possibly when and where) to ask a question, following some kind of protocol, for the purpose of receiving a specific answer, with the goal of gaining information in the process</rdfs:comment>
        <rdfs:label>Inquiry Specification</rdfs:label>
    </owl:Class>
    


    <!-- http://ontology.mayo.edu/ontology/KAO/InteractiveTechnique -->

    <owl:Class rdf:about="http://ontology.mayo.edu/ontology/KAO/InteractiveTechnique">
        <rdfs:subClassOf rdf:resource="https://www.omg.org/spec/API4KP/api4kp/KnowledgeProcessingTechnique"/>
        <rdfs:subClassOf>
            <owl:Restriction>
                <owl:onProperty rdf:resource="https://www.omg.org/spec/API4KP/api4kp/has-part"/>
                <owl:someValuesFrom rdf:resource="http://ontology.mayo.edu/ontology/KAO/ComputationalTechnique"/>
            </owl:Restriction>
        </rdfs:subClassOf>
        <rdfs:subClassOf>
            <owl:Restriction>
                <owl:onProperty rdf:resource="https://www.omg.org/spec/API4KP/api4kp/has-part"/>
                <owl:someValuesFrom rdf:resource="http://ontology.mayo.edu/ontology/KAO/NaturalisticTechnique"/>
            </owl:Restriction>
        </rdfs:subClassOf>
        <rdfs:label>HCI interactive technique</rdfs:label>
        <skos:definition>Technique that is based on the interaction of a Human and a Computer, in the context of a task where at least one of each participates as an agent</skos:definition>
    </owl:Class>
    


    <!-- http://ontology.mayo.edu/ontology/KAO/LogicBasedTechnique -->

    <owl:Class rdf:about="http://ontology.mayo.edu/ontology/KAO/LogicBasedTechnique">
        <rdfs:subClassOf rdf:resource="http://ontology.mayo.edu/ontology/KAO/QualitativeTechnique"/>
        <rdfs:comment>Technique based on formal logic</rdfs:comment>
        <rdfs:label>logic based technique</rdfs:label>
    </owl:Class>
    


    <!-- http://ontology.mayo.edu/ontology/KAO/MetricAsset -->

    <owl:Class rdf:about="http://ontology.mayo.edu/ontology/KAO/MetricAsset">
        <rdfs:subClassOf rdf:resource="http://ontology.mayo.edu/ontology/KAO/CategorizedKnowledgeAsset"/>
        <rdfs:comment>Knowledge of this kind usually builds directly on Assessment Models (for the quantification) and Process Models (to relate the measures to the processes and their goals).</rdfs:comment>
        <rdfs:isDefinedBy>http://ontology.mayo.edu/ontology/KAO</rdfs:isDefinedBy>
        <rdfs:label>Metric-Oriented Knowledge Asset</rdfs:label>
        <rdfs:seeAlso rdf:resource="https://www.cms.gov/Medicare/Quality-Initiatives-Patient-Assessment-Instruments/QualityMeasures/index.html"/>
        <skos:definition>Knowledge that pertains to how certain features (qualitative and/or quantitative) of a system can be observed, quantified, aggregated, compared to a baseline and objective values and ultimately used to evaluate the performance of (parts of) that system and its processes</skos:definition>
        <skos:prefLabel>KPIs, Measurements and Metrics</skos:prefLabel>
    </owl:Class>
    


    <!-- http://ontology.mayo.edu/ontology/KAO/MultiAgentDecisionTaskModel -->

    <owl:Class rdf:about="http://ontology.mayo.edu/ontology/KAO/MultiAgentDecisionTaskModel">
        <rdfs:subClassOf rdf:resource="http://ontology.mayo.edu/ontology/KAO/DecisionTaskModel"/>
        <rdfs:comment>Decision Task Model that requires the participation of two or more agents</rdfs:comment>
        <rdfs:label>Multi-Agent Decision Task Model</rdfs:label>
    </owl:Class>
    


    <!-- http://ontology.mayo.edu/ontology/KAO/NLPTechnique -->

    <owl:Class rdf:about="http://ontology.mayo.edu/ontology/KAO/NLPTechnique">
        <rdfs:subClassOf rdf:resource="http://ontology.mayo.edu/ontology/KAO/ComputationalTechnique"/>
        <rdfs:label>natural language processing technique</rdfs:label>
        <skos:definition>Computational Technique based on computations applied to expressions in natural language</skos:definition>
    </owl:Class>
    


    <!-- http://ontology.mayo.edu/ontology/KAO/NaturalisticTechnique -->

    <owl:Class rdf:about="http://ontology.mayo.edu/ontology/KAO/NaturalisticTechnique">
        <rdfs:subClassOf rdf:resource="https://www.omg.org/spec/API4KP/api4kp/KnowledgeProcessingTechnique"/>
        <rdfs:comment>I.e. technique such that a computer would not be able to apply it, and achieve the goal of a task executed (following a method) using this technique</rdfs:comment>
        <rdfs:label>naturalistic technique</rdfs:label>
        <skos:definition>Technique that requires a human agent to be leveraged to full effectiveness</skos:definition>
    </owl:Class>
    


    <!-- http://ontology.mayo.edu/ontology/KAO/OntologyLanguage -->

    <owl:Class rdf:about="http://ontology.mayo.edu/ontology/KAO/OntologyLanguage">
        <rdfs:subClassOf rdf:resource="http://ontology.mayo.edu/ontology/KAO/DedicatedLanguage"/>
        <rdfs:label>ontology language</rdfs:label>
        <skos:definition>Language used to express ontological Knowledge</skos:definition>
    </owl:Class>
    


    <!-- http://ontology.mayo.edu/ontology/KAO/OperationalConceptDefinition -->

    <owl:Class rdf:about="http://ontology.mayo.edu/ontology/KAO/OperationalConceptDefinition">
        <rdfs:subClassOf rdf:resource="http://ontology.mayo.edu/ontology/KAO/ExplicitRoleKnowledgeAsset"/>
        <rdfs:subClassOf rdf:resource="https://www.omg.org/spec/API4KP/api4kp/ConstructiveDefinition"/>
        <rdfs:subClassOf rdf:resource="https://www.omg.org/spec/API4KP/api4kp/KnowledgeProcessingMethodSpecification"/>
        <rdfs:subClassOf>
            <owl:Restriction>
                <owl:onProperty rdf:resource="https://www.omg.org/spec/API4KP/api4kp/defines"/>
                <owl:someValuesFrom rdf:resource="https://www.omg.org/spec/API4KP/api4kp/ResolvableConcept"/>
            </owl:Restriction>
        </rdfs:subClassOf>
        <rdfs:comment>Constructive Definition of a (resolvable) Concept that specifies how to resolve that Concept in some context or situation.
Some definitions have conditional applicability, limiting the class of situations in which they can be used</rdfs:comment>
        <rdfs:label>Operational Concept Definition</rdfs:label>
    </owl:Class>
    


    <!-- http://ontology.mayo.edu/ontology/KAO/OrderSet -->

    <owl:Class rdf:about="http://ontology.mayo.edu/ontology/KAO/OrderSet">
        <rdfs:subClassOf rdf:resource="http://ontology.mayo.edu/ontology/KAO/ClinicalKnowledgeAsset"/>
        <rdfs:subClassOf rdf:resource="http://ontology.mayo.edu/ontology/KAO/ProcessAsset"/>
        <rdfs:comment xml:lang="en">A standardized list of orders for a specific diagnosis</rdfs:comment>
        <rdfs:isDefinedBy rdf:resource="http://ontology.mayo.edu/ontology/KAO"/>
        <rdfs:label xml:lang="en">Order Set</rdfs:label>
        <skos:editorialNote xml:lang="en">Verify the defintion that restricts the ordersets to be developed by OSPAG, vs produced or endorsed</skos:editorialNote>
        <skos:example xml:lang="en">The Heart Failure Medication Titration Order Set</skos:example>
    </owl:Class>
    <owl:Axiom>
        <owl:annotatedSource rdf:resource="http://ontology.mayo.edu/ontology/KAO/OrderSet"/>
        <owl:annotatedProperty rdf:resource="http://www.w3.org/2004/02/skos/core#example"/>
        <owl:annotatedTarget xml:lang="en">The Heart Failure Medication Titration Order Set</owl:annotatedTarget>
        <rdfs:seeAlso rdf:resource="http://forms.mayo.edu/index.html?orderset#MC1156-1356"/>
    </owl:Axiom>
    


    <!-- http://ontology.mayo.edu/ontology/KAO/PredictiveModel -->

    <owl:Class rdf:about="http://ontology.mayo.edu/ontology/KAO/PredictiveModel">
        <rdfs:subClassOf rdf:resource="http://ontology.mayo.edu/ontology/KAO/AssessmentModel"/>
        <rdfs:comment>assessment of some state that is unobservable due to being in the future</rdfs:comment>
        <rdfs:label>Predictive Model</rdfs:label>
    </owl:Class>
    


    <!-- http://ontology.mayo.edu/ontology/KAO/ProcessAsset -->

    <owl:Class rdf:about="http://ontology.mayo.edu/ontology/KAO/ProcessAsset">
        <rdfs:subClassOf rdf:resource="http://ontology.mayo.edu/ontology/KAO/CategorizedKnowledgeAsset"/>
        <rdfs:comment>Specifications can be imperative (define what to do) or adaptive (define what not to do), depending on how many degrees of freedom are left to an agent</rdfs:comment>
        <rdfs:comment>The knowledge pertains specifically to the orchestration of the activities in relation to the goals, but usually relies on more ontologic, foundational definitions of the tasks to be performed as part of the process (as well as their related participants, roles, resources, etc.)</rdfs:comment>
        <rdfs:label>Process-Oriented Knowledge Asset</rdfs:label>
        <skos:definition>Knowledge about how to perform (complex) activities, properly orchestrated over time, so to achieve certain objectives and goals</skos:definition>
        <skos:prefLabel>Plans, Processes, Pathways and Protocol Definitions</skos:prefLabel>
        <skos:scopeNote>Does not cover &apos;natural&apos; processes that do not occur as a consequence of an agent&apos;s explicit intentions</skos:scopeNote>
    </owl:Class>
    


    <!-- http://ontology.mayo.edu/ontology/KAO/QualitativeTechnique -->

    <owl:Class rdf:about="http://ontology.mayo.edu/ontology/KAO/QualitativeTechnique">
        <rdfs:subClassOf rdf:resource="http://ontology.mayo.edu/ontology/KAO/ComputationalTechnique"/>
        <rdfs:label>qualitative computational technique</rdfs:label>
        <skos:altLabel>Symbolic Technique</skos:altLabel>
        <skos:definition>Computational Technique based on symbolic and/or logic-based principles</skos:definition>
    </owl:Class>
    


    <!-- http://ontology.mayo.edu/ontology/KAO/QualityMeasure -->

    <owl:Class rdf:about="http://ontology.mayo.edu/ontology/KAO/QualityMeasure">
        <rdfs:subClassOf rdf:resource="http://ontology.mayo.edu/ontology/KAO/ClinicalKnowledgeAsset"/>
        <rdfs:subClassOf rdf:resource="http://ontology.mayo.edu/ontology/KAO/MetricAsset"/>
        <rdfs:comment>CQMs are tools that help measure or quantify healthcare processes, outcomes, patient
perceptions and organizational structure and/or systems that are associated with the ability to provide high-
quality healthcare and/or that relate to one or more quality goals</rdfs:comment>
        <rdfs:isDefinedBy rdf:resource="http://ontology.mayo.edu/ontology/KAO"/>
        <rdfs:seeAlso rdf:resource="https://www.cms.gov/Medicare/Quality-Initiatives-Patient-Assessment-Instruments/QualityMeasures/index.html"/>
        <skos:prefLabel>Clinical Quality Measure</skos:prefLabel>
    </owl:Class>
    


    <!-- http://ontology.mayo.edu/ontology/KAO/QuantitativeTechnique -->

    <owl:Class rdf:about="http://ontology.mayo.edu/ontology/KAO/QuantitativeTechnique">
        <rdfs:subClassOf rdf:resource="http://ontology.mayo.edu/ontology/KAO/ComputationalTechnique"/>
        <rdfs:label>quantitative computational technique</rdfs:label>
        <skos:altLabel>Subsymbolic Technique</skos:altLabel>
        <skos:definition>Computational Technique that is based on mathematical, statistical and/or numerical principles</skos:definition>
    </owl:Class>
    


    <!-- http://ontology.mayo.edu/ontology/KAO/QueryLanguage -->

    <owl:Class rdf:about="http://ontology.mayo.edu/ontology/KAO/QueryLanguage">
        <rdfs:subClassOf rdf:resource="http://ontology.mayo.edu/ontology/KAO/DedicatedLanguage"/>
        <rdfs:label>query language</rdfs:label>
        <skos:definition>language used to express queries</skos:definition>
    </owl:Class>
    


    <!-- http://ontology.mayo.edu/ontology/KAO/QueryTechnique -->

    <owl:Class rdf:about="http://ontology.mayo.edu/ontology/KAO/QueryTechnique">
        <rdfs:subClassOf rdf:resource="https://www.omg.org/spec/API4KP/api4kp/KnowledgeProcessingTechnique"/>
        <rdfs:label>query based technique</rdfs:label>
        <skos:definition>Technique that involves requesting another agent to actually perform the task, from which the products can be obtained</skos:definition>
    </owl:Class>
    


    <!-- http://ontology.mayo.edu/ontology/KAO/Questionnaire -->

    <owl:Class rdf:about="http://ontology.mayo.edu/ontology/KAO/Questionnaire">
        <rdfs:subClassOf rdf:resource="http://ontology.mayo.edu/ontology/KAO/DocumentationTemplate"/>
        <rdfs:comment xml:lang="en">An organized collection of questions intended to solicit information from patients, providers or other individuals in the healthcare domain</rdfs:comment>
        <rdfs:isDefinedBy rdf:resource="http://ontology.mayo.edu/ontology/KAO"/>
        <rdfs:label xml:lang="en">Questionnaire</rdfs:label>
        <skos:example xml:lang="en">First Visit Questionnaire</skos:example>
        <skos:prefLabel xml:lang="en">Questionnaire</skos:prefLabel>
    </owl:Class>
    <owl:Axiom>
        <owl:annotatedSource rdf:resource="http://ontology.mayo.edu/ontology/KAO/Questionnaire"/>
        <owl:annotatedProperty rdf:resource="http://www.w3.org/2004/02/skos/core#example"/>
        <owl:annotatedTarget xml:lang="en">First Visit Questionnaire</owl:annotatedTarget>
        <rdfs:seeAlso rdf:resource="http://mayoweb.mayo.edu/sp-forms/mc20600-mc20699/mchs20617.pdf"/>
    </owl:Axiom>
    


    <!-- http://ontology.mayo.edu/ontology/KAO/RuleLanguage -->

    <owl:Class rdf:about="http://ontology.mayo.edu/ontology/KAO/RuleLanguage">
        <rdfs:subClassOf rdf:resource="http://ontology.mayo.edu/ontology/KAO/DedicatedLanguage"/>
        <rdfs:label>rule language</rdfs:label>
        <skos:definition>Language used in the expression of (business) formal rules</skos:definition>
    </owl:Class>
    


    <!-- http://ontology.mayo.edu/ontology/KAO/SchemaLanguage -->

    <owl:Class rdf:about="http://ontology.mayo.edu/ontology/KAO/SchemaLanguage">
        <rdfs:subClassOf rdf:resource="http://ontology.mayo.edu/ontology/KAO/DedicatedLanguage"/>
        <rdfs:label>schema language</rdfs:label>
        <skos:definition>Language used for data and information (meta)modeling</skos:definition>
    </owl:Class>
    


    <!-- http://ontology.mayo.edu/ontology/KAO/SemanticAsset -->

    <owl:Class rdf:about="http://ontology.mayo.edu/ontology/KAO/SemanticAsset">
        <rdfs:subClassOf rdf:resource="http://ontology.mayo.edu/ontology/KAO/CategorizedKnowledgeAsset"/>
        <rdfs:comment>Assets in this category can be classified along the semantic spectrum</rdfs:comment>
        <rdfs:comment>Knowledge of this kind is usually structural, universal, and expressed using declarative languages</rdfs:comment>
        <rdfs:isDefinedBy>http://ontology.mayo.edu/ontology/KAO</rdfs:isDefinedBy>
        <rdfs:label>Semantic-Oriented Knowledge Asset</rdfs:label>
        <rdfs:seeAlso rdf:datatype="http://www.w3.org/2001/XMLSchema#anyURI">http://slidegur.com/doc/5719791/presentation</rdfs:seeAlso>
        <skos:definition>Foundational Knowledge about (Clinical) Concepts, their definitions and mutual relationships, together with their linguistic and syntactic expressions.</skos:definition>
        <skos:example rdf:datatype="http://www.w3.org/2001/XMLSchema#anyURI">A Drug/Drug interaction Assertional KB</skos:example>
        <skos:example>The Mayo Clinic Asthma Value Set</skos:example>
        <skos:example>The Ontology of Knowledge Assets, of which this OWL-based representation is an expression</skos:example>
        <skos:prefLabel>Terminology, Ontology and Assertional KBs</skos:prefLabel>
    </owl:Class>
    <owl:Axiom>
        <owl:annotatedSource rdf:resource="http://ontology.mayo.edu/ontology/KAO/SemanticAsset"/>
        <owl:annotatedProperty rdf:resource="http://www.w3.org/2004/02/skos/core#example"/>
        <owl:annotatedTarget>The Mayo Clinic Asthma Value Set</owl:annotatedTarget>
        <rdfs:seeAlso rdf:resource="http://ckm.ontology.mayo.edu/ontology/%5C%5Cmfad.mfroot.org%5Crchdept%5CTerms%5CTerminology%20Web%5C2_ValueSets%5CMCBT_ClinicalProblemAsthma.pdf"/>
    </owl:Axiom>
    


    <!-- http://ontology.mayo.edu/ontology/KAO/SemanticDecisionModel -->

    <owl:Class rdf:about="http://ontology.mayo.edu/ontology/KAO/SemanticDecisionModel">
        <rdfs:subClassOf rdf:resource="http://ontology.mayo.edu/ontology/KAO/DecisionModel"/>
        <rdfs:comment>Decision Model that includes an unambiguous definition of every concept involved</rdfs:comment>
        <rdfs:label>Semantic Decision Model</rdfs:label>
    </owl:Class>
    


    <!-- http://ontology.mayo.edu/ontology/KAO/SemanticInformationModel -->

    <owl:Class rdf:about="http://ontology.mayo.edu/ontology/KAO/SemanticInformationModel">
        <rdfs:subClassOf rdf:resource="http://ontology.mayo.edu/ontology/KAO/InformationModel"/>
        <rdfs:subClassOf>
            <owl:Restriction>
                <owl:onProperty rdf:resource="https://www.omg.org/spec/API4KP/api4kp/has-part"/>
                <owl:someValuesFrom rdf:resource="http://ontology.mayo.edu/ontology/KAO/SemanticInformationModel"/>
            </owl:Restriction>
        </rdfs:subClassOf>
        <rdfs:comment>Information Model designed such that instances have one and only one interpretation</rdfs:comment>
        <rdfs:label>Semantic Information Model</rdfs:label>
    </owl:Class>
    


    <!-- http://ontology.mayo.edu/ontology/KAO/ServiceBasedTechnique -->

    <owl:Class rdf:about="http://ontology.mayo.edu/ontology/KAO/ServiceBasedTechnique">
        <rdfs:subClassOf rdf:resource="https://www.omg.org/spec/API4KP/api4kp/KnowledgeProcessingTechnique"/>
        <rdfs:comment>Technique based on delegation to another entity</rdfs:comment>
        <rdfs:label>service based technique</rdfs:label>
    </owl:Class>
    


    <!-- http://ontology.mayo.edu/ontology/KAO/ServiceDescription -->

    <owl:Class rdf:about="http://ontology.mayo.edu/ontology/KAO/ServiceDescription">
        <rdfs:subClassOf rdf:resource="http://ontology.mayo.edu/ontology/KAO/ProcessAsset"/>
        <rdfs:label>Service Description</rdfs:label>
    </owl:Class>
    


    <!-- http://ontology.mayo.edu/ontology/KAO/ServiceProfile -->

    <owl:Class rdf:about="http://ontology.mayo.edu/ontology/KAO/ServiceProfile">
        <rdfs:subClassOf rdf:resource="http://ontology.mayo.edu/ontology/KAO/ServiceDescription"/>
        <rdfs:comment>Service Description that refines (by constraint), and thus depends on, some Service Description</rdfs:comment>
        <rdfs:label>Service Profile</rdfs:label>
    </owl:Class>
    


    <!-- http://ontology.mayo.edu/ontology/KAO/ValueSet -->

    <owl:Class rdf:about="http://ontology.mayo.edu/ontology/KAO/ValueSet">
        <rdfs:subClassOf rdf:resource="http://ontology.mayo.edu/ontology/KAO/SemanticAsset"/>
        <rdfs:comment xml:lang="en">A set of pairs of &quot;codes&quot;, drawn from one or more code systems, and human-readable terms that represent clinical concepts (e.g. &quot;diabetes type II&quot;)</rdfs:comment>
        <rdfs:isDefinedBy rdf:resource="http://ontology.mayo.edu/ontology/KAO"/>
        <rdfs:label xml:lang="en">Value Set</rdfs:label>
        <skos:example xml:lang="en">The Asthma Value Set</skos:example>
        <skos:prefLabel xml:lang="en">Value Set</skos:prefLabel>
    </owl:Class>
    <owl:Axiom>
        <owl:annotatedSource rdf:resource="http://ontology.mayo.edu/ontology/KAO/ValueSet"/>
        <owl:annotatedProperty rdf:resource="http://www.w3.org/2004/02/skos/core#example"/>
        <owl:annotatedTarget xml:lang="en">The Asthma Value Set</owl:annotatedTarget>
        <rdfs:seeAlso rdf:resource="http://ckm.ontology.mayo.edu/ontology/%5C%5Cmfad.mfroot.org%5Crchdept%5CTerms%5CTerminology%20Web%5C2_ValueSets%5CMCBT_ClinicalProblemAsthma.pdf"/>
    </owl:Axiom>
    


    <!-- https://www.omg.org/spec/API4KP/api4kp/CompositeKnowledgeResource -->

    <owl:Class rdf:about="https://www.omg.org/spec/API4KP/api4kp/CompositeKnowledgeResource"/>
    


    <!-- https://www.omg.org/spec/API4KP/api4kp/ConstructedLanguage -->

    <owl:Class rdf:about="https://www.omg.org/spec/API4KP/api4kp/ConstructedLanguage"/>
    


    <!-- https://www.omg.org/spec/API4KP/api4kp/ConstructiveDefinition -->

    <owl:Class rdf:about="https://www.omg.org/spec/API4KP/api4kp/ConstructiveDefinition"/>
    


    <!-- https://www.omg.org/spec/API4KP/api4kp/Definition -->

    <owl:Class rdf:about="https://www.omg.org/spec/API4KP/api4kp/Definition"/>
    


    <!-- https://www.omg.org/spec/API4KP/api4kp/Grammar -->

    <owl:Class rdf:about="https://www.omg.org/spec/API4KP/api4kp/Grammar">
        <rdfs:subClassOf rdf:resource="http://ontology.mayo.edu/ontology/KAO/InformationAsset"/>
    </owl:Class>
    


    <!-- https://www.omg.org/spec/API4KP/api4kp/InformationProcessingTask -->

    <owl:Class rdf:about="https://www.omg.org/spec/API4KP/api4kp/InformationProcessingTask"/>
    


    <!-- https://www.omg.org/spec/API4KP/api4kp/KnowledgeAsset -->

    <owl:Class rdf:about="https://www.omg.org/spec/API4KP/api4kp/KnowledgeAsset"/>
    


    <!-- https://www.omg.org/spec/API4KP/api4kp/KnowledgeProcessingMethodSpecification -->

    <owl:Class rdf:about="https://www.omg.org/spec/API4KP/api4kp/KnowledgeProcessingMethodSpecification"/>
    


    <!-- https://www.omg.org/spec/API4KP/api4kp/KnowledgeProcessingTechnique -->

    <owl:Class rdf:about="https://www.omg.org/spec/API4KP/api4kp/KnowledgeProcessingTechnique"/>
    


    <!-- https://www.omg.org/spec/API4KP/api4kp/Lexicon -->

    <owl:Class rdf:about="https://www.omg.org/spec/API4KP/api4kp/Lexicon">
        <rdfs:subClassOf rdf:resource="http://ontology.mayo.edu/ontology/KAO/SemanticAsset"/>
    </owl:Class>
    


    <!-- https://www.omg.org/spec/API4KP/api4kp/ResolvableConcept -->

    <owl:Class rdf:about="https://www.omg.org/spec/API4KP/api4kp/ResolvableConcept"/>
</rdf:RDF>



<!-- Generated by the OWL API (version 4.2.8.20170104-2310) https://github.com/owlcs/owlapi -->

