<?xml version="1.0" encoding="UTF-8"?>
<!DOCTYPE rdf:RDF [
	<!ENTITY api4kp "https://www.omg.org/spec/API4KP/api4kp/">
	<!ENTITY api4kp-krr "https://www.omg.org/spec/API4KP/api4kp-krr/">
	<!ENTITY api4kp-lang "https://www.omg.org/spec/API4KP/api4kp-lang/">
	<!ENTITY api4kp-ops "https://www.omg.org/spec/API4KP/api4kp-ops/">
	<!ENTITY api4kp-rel "https://www.omg.org/spec/API4KP/api4kp-rel/">
	<!ENTITY api4kp-series "https://www.omg.org/spec/API4KP/api4kp-series/">
	<!ENTITY dct "http://purl.org/dc/terms/">
	<!ENTITY dol "http://www.omg.org/spec/DOL/DOL-terms/">
	<!ENTITY lcc-lr "https://www.omg.org/spec/LCC/Languages/LanguageRepresentation/">
	<!ENTITY owl "http://www.w3.org/2002/07/owl#">
	<!ENTITY rdf "http://www.w3.org/1999/02/22-rdf-syntax-ns#">
	<!ENTITY rdfs "http://www.w3.org/2000/01/rdf-schema#">
	<!ENTITY skos "http://www.w3.org/2004/02/skos/core#">
	<!ENTITY sm "http://www.omg.org/techprocess/ab/SpecificationMetadata/">
	<!ENTITY xsd "http://www.w3.org/2001/XMLSchema#">
]>
<rdf:RDF xml:base="https://www.omg.org/spec/API4KP/api4kp-ops/"
	xmlns:api4kp="https://www.omg.org/spec/API4KP/api4kp/"
	xmlns:api4kp-krr="https://www.omg.org/spec/API4KP/api4kp-krr/"
	xmlns:api4kp-lang="https://www.omg.org/spec/API4KP/api4kp-lang/"
	xmlns:api4kp-ops="https://www.omg.org/spec/API4KP/api4kp-ops/"
	xmlns:api4kp-rel="https://www.omg.org/spec/API4KP/api4kp-rel/"
	xmlns:api4kp-series="https://www.omg.org/spec/API4KP/api4kp-series/"
	xmlns:dct="http://purl.org/dc/terms/"
	xmlns:dol="http://www.omg.org/spec/DOL/DOL-terms/"
	xmlns:lcc-lr="https://www.omg.org/spec/LCC/Languages/LanguageRepresentation/"
	xmlns:owl="http://www.w3.org/2002/07/owl#"
	xmlns:rdf="http://www.w3.org/1999/02/22-rdf-syntax-ns#"
	xmlns:rdfs="http://www.w3.org/2000/01/rdf-schema#"
	xmlns:skos="http://www.w3.org/2004/02/skos/core#"
	xmlns:sm="http://www.omg.org/techprocess/ab/SpecificationMetadata/"
	xmlns:xsd="http://www.w3.org/2001/XMLSchema#">
	
	<owl:Ontology rdf:about="https://www.omg.org/spec/API4KP/api4kp-ops/">
		<rdfs:label>Ontology of API4KP Operations</rdfs:label>
		<dct:abstract>This ontology focuses on the definition of operations used by API4KP, including but not limited to access and transformation services.</dct:abstract>
		<dct:creator>Davide Sottara (sottara.davide at mayo.edu)</dct:creator>
		<dct:license rdf:datatype="&xsd;anyURI">http://opensource.org/licenses/MIT</dct:license>
		<sm:contentLanguage rdf:datatype="&xsd;anyURI">https://www.w3.org/TR/owl2-quick-reference/</sm:contentLanguage>
		<sm:copyright>Copyright (c) 2014-2020 Athan Services</sm:copyright>
		<sm:copyright>Copyright (c) 2014-2020 Fraunhofer Gesellschaft</sm:copyright>
		<sm:copyright>Copyright (c) 2014-2020 Freie Universität Berlin</sm:copyright>
		<sm:copyright>Copyright (c) 2014-2020 Mayo Foundation for Medical Education and Research (MFMER)</sm:copyright>
		<sm:copyright>Copyright (c) 2014-2020 Thematix Partners LLC</sm:copyright>
		<sm:copyright>Copyright (c) 2015-2020 Object Management Group, Inc.</sm:copyright>
		<sm:copyright>Copyright (c) 2019-2020 Universität Leipzig</sm:copyright>
		<sm:copyright>Copyright (c) 2020 Micro Focus</sm:copyright>
		<sm:dependsOn rdf:datatype="&xsd;anyURI">https://www.omg.org/spec/API4KP/api4kp-krr/</sm:dependsOn>
		<sm:dependsOn rdf:datatype="&xsd;anyURI">https://www.omg.org/spec/API4KP/api4kp-lang/</sm:dependsOn>
		<sm:dependsOn rdf:datatype="&xsd;anyURI">https://www.omg.org/spec/API4KP/api4kp-rel/</sm:dependsOn>
		<sm:dependsOn rdf:datatype="&xsd;anyURI">https://www.omg.org/spec/API4KP/api4kp-series/</sm:dependsOn>
		<sm:dependsOn rdf:datatype="&xsd;anyURI">https://www.omg.org/spec/API4KP/api4kp/</sm:dependsOn>
		<sm:dependsOn rdf:datatype="&xsd;anyURI">https://www.omg.org/spec/DOL/</sm:dependsOn>
		<sm:dependsOn rdf:datatype="&xsd;anyURI">https://www.omg.org/spec/LCC/</sm:dependsOn>
		<sm:fileAbbreviation>api4kp-ops</sm:fileAbbreviation>
		<sm:filename>api4kp-ops.rdf</sm:filename>
		<owl:imports rdf:resource="http://www.omg.org/techprocess/ab/SpecificationMetadata/"/>
		<owl:imports rdf:resource="https://www.omg.org/spec/API4KP/api4kp-krr/"/>
		<owl:imports rdf:resource="https://www.omg.org/spec/API4KP/api4kp-lang/"/>
		<owl:imports rdf:resource="https://www.omg.org/spec/API4KP/api4kp-rel/"/>
		<owl:imports rdf:resource="https://www.omg.org/spec/API4KP/api4kp-series/"/>
		<owl:imports rdf:resource="https://www.omg.org/spec/API4KP/api4kp/"/>
		<owl:imports rdf:resource="https://www.omg.org/spec/DOL/20171106/DOL-terms.rdf"/>
		<owl:imports rdf:resource="https://www.omg.org/spec/LCC/Languages/LanguageRepresentation/"/>
		<owl:versionIRI rdf:resource="https://www.omg.org/spec/API4KP/20200801/api4kp-ops/"/>
	</owl:Ontology>
	
	<owl:Class rdf:about="&api4kp-ops;AbridgmentTask">
		<rdfs:subClassOf rdf:resource="&api4kp-ops;ParaphraseTask"/>
		<rdfs:label>abdrigment task</rdfs:label>
		<skos:definition>paraphrase that eliminates element of an expression that are not essential to reconstruct its meaning</skos:definition>
	</owl:Class>
	
	<owl:Class rdf:about="&api4kp-ops;CarvingTask">
		<rdfs:subClassOf rdf:resource="&api4kp-ops;SelectionTask"/>
		<rdfs:label>carving task</rdfs:label>
		<skos:definition>selection based on the inclusion of fragments that evoke certain concepts</skos:definition>
	</owl:Class>
	
	<owl:Class rdf:about="&api4kp-ops;CherryPickingTask">
		<rdfs:subClassOf rdf:resource="&api4kp-ops;SelectionTask"/>
		<rdfs:label>cherry-picking task</rdfs:label>
		<skos:definition>selection task where the concepts to be included are enumerated explicitly</skos:definition>
	</owl:Class>
	
	<owl:Class rdf:about="&api4kp-ops;ClassificationTask">
		<rdfs:subClassOf rdf:resource="&api4kp-ops;LogicBasedReasoningTask"/>
		<rdfs:label>classification task</rdfs:label>
		<skos:note>reasoning Task such that, given an individual and a set of concepts (classes), determines which concepts (classes) that individual is an instance (member) of</skos:note>
	</owl:Class>
	
	<owl:Class rdf:about="&api4kp-ops;ClearRepositoryLocationTask">
		<rdfs:subClassOf rdf:resource="&api4kp-ops;KnowledgeArtifactRepositoryTask"/>
		<rdfs:label>clear repository location task</rdfs:label>
		<skos:definition>ensures that no artifact is stored at a given location</skos:definition>
	</owl:Class>
	
	<owl:Class rdf:about="&api4kp-ops;ComplexityDetectionTask">
		<rdfs:subClassOf rdf:resource="&api4kp-ops;KnowledgeAnalyticTask"/>
		<rdfs:subClassOf>
			<owl:Restriction>
				<owl:onProperty rdf:resource="&api4kp-ops;hasSubtask"/>
				<owl:someValuesFrom rdf:resource="&api4kp-ops;ParsingTask"/>
			</owl:Restriction>
		</rdfs:subClassOf>
		<rdfs:subClassOf>
			<owl:Restriction>
				<owl:onProperty rdf:resource="&api4kp-ops;involvesRole"/>
				<owl:someValuesFrom>
					<owl:Class>
						<owl:intersectionOf rdf:parseType="Collection">
							<rdf:Description rdf:about="&api4kp-ops;Product">
							</rdf:Description>
							<owl:Restriction>
								<owl:onProperty rdf:resource="&api4kp-ops;isFilledBy"/>
								<owl:someValuesFrom rdf:resource="&api4kp-krr;ComputationalComplexityClass"/>
							</owl:Restriction>
						</owl:intersectionOf>
					</owl:Class>
				</owl:someValuesFrom>
			</owl:Restriction>
		</rdfs:subClassOf>
		<rdfs:label>complexity detection task</rdfs:label>
		<skos:definition>analytic task that detects the computational complexity (space and/or time) of a given knowledge expression</skos:definition>
	</owl:Class>
	
	<owl:Class rdf:about="&api4kp-ops;ConfigurationParameter">
		<rdfs:subClassOf rdf:resource="&api4kp-ops;KnowledgeProcessingTaskRole"/>
		<rdfs:label>configuration parameter</rdfs:label>
		<skos:definition>role played by a value, selected from a &apos;region&apos; of admissible values, that can remove a degree of freedom from the execution of a (knowledge processing) task, without changing the nature of the task</skos:definition>
	</owl:Class>
	
	<owl:Class rdf:about="&api4kp-ops;ConsistencyCheckTask">
		<rdfs:subClassOf rdf:resource="&api4kp-ops;LogicBasedReasoningTask"/>
		<rdfs:label>consistency checking task</rdfs:label>
		<rdfs:seeAlso>https://en.wikipedia.org/wiki/Consistency</rdfs:seeAlso>
		<skos:definition>reasoning task that determines whether a knowledge base is inconsistent, i.e. it allows derivation of a logical contradication</skos:definition>
	</owl:Class>
	
	<owl:Class rdf:about="&api4kp-ops;DecodingTask">
		<rdfs:subClassOf rdf:resource="&api4kp-ops;LiftingTask"/>
		<rdfs:subClassOf>
			<owl:Restriction>
				<owl:onProperty rdf:resource="&api4kp-ops;involvesRole"/>
				<owl:someValuesFrom>
					<owl:Class>
						<owl:intersectionOf rdf:parseType="Collection">
							<rdf:Description rdf:about="&api4kp-ops;Input">
							</rdf:Description>
							<owl:Restriction>
								<owl:onProperty rdf:resource="&api4kp-ops;isFilledBy"/>
								<owl:someValuesFrom rdf:resource="&api4kp;EncodedKnowledgeExpression"/>
							</owl:Restriction>
						</owl:intersectionOf>
					</owl:Class>
				</owl:someValuesFrom>
			</owl:Restriction>
		</rdfs:subClassOf>
		<rdfs:subClassOf>
			<owl:Restriction>
				<owl:onProperty rdf:resource="&api4kp-ops;involvesRole"/>
				<owl:someValuesFrom>
					<owl:Class>
						<owl:intersectionOf rdf:parseType="Collection">
							<rdf:Description rdf:about="&api4kp-ops;Product">
							</rdf:Description>
							<owl:Restriction>
								<owl:onProperty rdf:resource="&api4kp-ops;isFilledBy"/>
								<owl:someValuesFrom rdf:resource="&api4kp;ConcreteKnowledgeExpression"/>
							</owl:Restriction>
						</owl:intersectionOf>
					</owl:Class>
				</owl:someValuesFrom>
			</owl:Restriction>
		</rdfs:subClassOf>
		<rdfs:label>decoding task</rdfs:label>
		<skos:definition>the act of recreating a concrete expression from its encoded version</skos:definition>
	</owl:Class>
	
	<owl:Class rdf:about="&api4kp-ops;DependencyResolutionTask">
		<rdfs:subClassOf rdf:resource="&api4kp-ops;KnowledgeResourceDiscoveryTask"/>
		<rdfs:subClassOf>
			<owl:Restriction>
				<owl:onProperty rdf:resource="&api4kp-ops;involvesRole"/>
				<owl:someValuesFrom>
					<owl:Class>
						<owl:intersectionOf rdf:parseType="Collection">
							<rdf:Description rdf:about="&api4kp-ops;Input">
							</rdf:Description>
							<owl:Restriction>
								<owl:onProperty rdf:resource="&api4kp-ops;isFilledBy"/>
								<owl:someValuesFrom rdf:resource="&api4kp;KnowledgeResource"/>
							</owl:Restriction>
						</owl:intersectionOf>
					</owl:Class>
				</owl:someValuesFrom>
			</owl:Restriction>
		</rdfs:subClassOf>
		<rdfs:subClassOf>
			<owl:Restriction>
				<owl:onProperty rdf:resource="&api4kp-ops;involvesRole"/>
				<owl:someValuesFrom>
					<owl:Class>
						<owl:intersectionOf rdf:parseType="Collection">
							<rdf:Description rdf:about="&api4kp-ops;Product">
							</rdf:Description>
							<owl:Restriction>
								<owl:onProperty rdf:resource="&api4kp-ops;isFilledBy"/>
								<owl:someValuesFrom rdf:resource="&api4kp;KnowledgeResource"/>
							</owl:Restriction>
						</owl:intersectionOf>
					</owl:Class>
				</owl:someValuesFrom>
			</owl:Restriction>
		</rdfs:subClassOf>
		<rdfs:label>dependency resolution task</rdfs:label>
		<skos:definition>knowledge resource discovery task that resolves dependency relationships between knowledge resources</skos:definition>
	</owl:Class>
	
	<owl:Class rdf:about="&api4kp-ops;DiffingTask">
		<rdfs:subClassOf rdf:resource="&api4kp-ops;KnowledgeAnalyticTask"/>
		<rdfs:label>diffing task</rdfs:label>
		<skos:definition>analytic task that detects the differences between two knowledge expressions</skos:definition>
	</owl:Class>
	
	<owl:Class rdf:about="&api4kp-ops;EncodingTask">
		<rdfs:subClassOf rdf:resource="&api4kp-ops;LoweringTask"/>
		<rdfs:subClassOf>
			<owl:Restriction>
				<owl:onProperty rdf:resource="&api4kp-ops;involvesRole"/>
				<owl:someValuesFrom>
					<owl:Class>
						<owl:intersectionOf rdf:parseType="Collection">
							<rdf:Description rdf:about="&api4kp-ops;Input">
							</rdf:Description>
							<owl:Restriction>
								<owl:onProperty rdf:resource="&api4kp-ops;isFilledBy"/>
								<owl:someValuesFrom rdf:resource="&api4kp-lang;Encoding"/>
							</owl:Restriction>
						</owl:intersectionOf>
					</owl:Class>
				</owl:someValuesFrom>
			</owl:Restriction>
		</rdfs:subClassOf>
		<rdfs:subClassOf>
			<owl:Restriction>
				<owl:onProperty rdf:resource="&api4kp-ops;involvesRole"/>
				<owl:someValuesFrom>
					<owl:Class>
						<owl:intersectionOf rdf:parseType="Collection">
							<rdf:Description rdf:about="&api4kp-ops;Input">
							</rdf:Description>
							<owl:Restriction>
								<owl:onProperty rdf:resource="&api4kp-ops;isFilledBy"/>
								<owl:someValuesFrom rdf:resource="&api4kp;ConcreteKnowledgeExpression"/>
							</owl:Restriction>
						</owl:intersectionOf>
					</owl:Class>
				</owl:someValuesFrom>
			</owl:Restriction>
		</rdfs:subClassOf>
		<rdfs:subClassOf>
			<owl:Restriction>
				<owl:onProperty rdf:resource="&api4kp-ops;involvesRole"/>
				<owl:someValuesFrom>
					<owl:Class>
						<owl:intersectionOf rdf:parseType="Collection">
							<rdf:Description rdf:about="&api4kp-ops;Product">
							</rdf:Description>
							<owl:Restriction>
								<owl:onProperty rdf:resource="&api4kp-ops;isFilledBy"/>
								<owl:someValuesFrom rdf:resource="&api4kp;EncodedKnowledgeExpression"/>
							</owl:Restriction>
						</owl:intersectionOf>
					</owl:Class>
				</owl:someValuesFrom>
			</owl:Restriction>
		</rdfs:subClassOf>
		<rdfs:label>encoding task</rdfs:label>
		<skos:definition></skos:definition>
		<skos:definition>lowering task that applies an encoding to a concrete expression</skos:definition>
		<skos:example>converting characters into sequences of bits, according to an encoding method, so that they can be written to a RAM, ROM or magnetic disk</skos:example>
	</owl:Class>
	
	<owl:Class rdf:about="&api4kp-ops;EntailmentCheckTask">
		<rdfs:subClassOf rdf:resource="&api4kp-ops;LogicBasedReasoningTask"/>
		<rdfs:label>entailment check test</rdfs:label>
		<skos:definition>reasoning task that determines whether a given working knowledge base is entailed by a reference working knowledge base through logical consequence</skos:definition>
	</owl:Class>
	
	<owl:Class rdf:about="&api4kp-ops;Explanation">
		<rdfs:subClassOf rdf:resource="&api4kp-ops;KnowledgeProcessingTaskRole"/>
		<rdfs:label>explanation</rdfs:label>
		<skos:definition>role played by an expression, generated as part of the execution of a (knowledge processing) activity, that captures knowledge about the course of that activity and/or its inputs, outputs and substrate</skos:definition>
	</owl:Class>
	
	<owl:Class rdf:about="&api4kp-ops;ExpressionTask">
		<rdfs:subClassOf rdf:resource="&api4kp-ops;LoweringTask"/>
		<rdfs:subClassOf>
			<owl:Restriction>
				<owl:onProperty rdf:resource="&api4kp-ops;involvesRole"/>
				<owl:someValuesFrom>
					<owl:Class>
						<owl:intersectionOf rdf:parseType="Collection">
							<rdf:Description rdf:about="&api4kp-ops;Input">
							</rdf:Description>
							<owl:Restriction>
								<owl:onProperty rdf:resource="&api4kp-ops;isFilledBy"/>
								<owl:someValuesFrom rdf:resource="&api4kp-lang;AbstractSyntax"/>
							</owl:Restriction>
						</owl:intersectionOf>
					</owl:Class>
				</owl:someValuesFrom>
			</owl:Restriction>
		</rdfs:subClassOf>
		<rdfs:subClassOf>
			<owl:Restriction>
				<owl:onProperty rdf:resource="&api4kp-ops;involvesRole"/>
				<owl:someValuesFrom>
					<owl:Class>
						<owl:intersectionOf rdf:parseType="Collection">
							<rdf:Description rdf:about="&api4kp-ops;Input">
							</rdf:Description>
							<owl:Restriction>
								<owl:onProperty rdf:resource="&api4kp-ops;isFilledBy"/>
								<owl:someValuesFrom rdf:resource="&api4kp-lang;Lexicon"/>
							</owl:Restriction>
						</owl:intersectionOf>
					</owl:Class>
				</owl:someValuesFrom>
			</owl:Restriction>
		</rdfs:subClassOf>
		<rdfs:subClassOf>
			<owl:Restriction>
				<owl:onProperty rdf:resource="&api4kp-ops;involvesRole"/>
				<owl:someValuesFrom>
					<owl:Class>
						<owl:intersectionOf rdf:parseType="Collection">
							<rdf:Description rdf:about="&api4kp-ops;Input">
							</rdf:Description>
							<owl:Restriction>
								<owl:onProperty rdf:resource="&api4kp-ops;isFilledBy"/>
								<owl:someValuesFrom rdf:resource="&api4kp;WorkOfKnowledge"/>
							</owl:Restriction>
						</owl:intersectionOf>
					</owl:Class>
				</owl:someValuesFrom>
			</owl:Restriction>
		</rdfs:subClassOf>
		<rdfs:subClassOf>
			<owl:Restriction>
				<owl:onProperty rdf:resource="&api4kp-ops;involvesRole"/>
				<owl:someValuesFrom>
					<owl:Class>
						<owl:intersectionOf rdf:parseType="Collection">
							<rdf:Description rdf:about="&api4kp-ops;Product">
							</rdf:Description>
							<owl:Restriction>
								<owl:onProperty rdf:resource="&api4kp-ops;isFilledBy"/>
								<owl:someValuesFrom rdf:resource="&api4kp;AbstractKnowledgeExpression"/>
							</owl:Restriction>
						</owl:intersectionOf>
					</owl:Class>
				</owl:someValuesFrom>
			</owl:Restriction>
		</rdfs:subClassOf>
		<rdfs:label>expression task</rdfs:label>
		<skos:definition>lowering task that creates an expression in a given language (sytnax and lexicon), from the information content of a work of knowledge</skos:definition>
	</owl:Class>
	
	<owl:Class rdf:about="&api4kp-ops;ExtensionTask">
		<rdfs:subClassOf rdf:resource="&api4kp-ops;InjectionTask"/>
		<rdfs:label>extension task</rdfs:label>
		<skos:definition>injection of a resource into a second resource, which plays the role of &apos;extension&apos;, providing a wrapping context</skos:definition>
	</owl:Class>
	
	<owl:Class rdf:about="&api4kp-ops;ExtractionTask">
		<rdfs:subClassOf rdf:resource="&api4kp-ops;SeparationTask"/>
		<rdfs:label>extraction task</rdfs:label>
		<skos:definition>separation based on a tree-oriented deconstruction, where the resources that are part of a subtree of the underlying structure are returned</skos:definition>
	</owl:Class>
	
	<owl:Class rdf:about="&api4kp-ops;FilteringTask">
		<rdfs:subClassOf rdf:resource="&api4kp-ops;SimplificationTask"/>
		<rdfs:label>censoring task</rdfs:label>
		<skos:definition>simplification aimed at removing one or more concepts, and their transitive associations, from the input work of knowledge</skos:definition>
		<skos:note>The expression of the resulting WoK will not contain any linguistic element that evokes the redacted concepts.</skos:note>
	</owl:Class>
	
	<owl:Class rdf:about="&api4kp-ops;FusionTask">
		<rdfs:subClassOf rdf:resource="&api4kp-ops;KnowledgeReshapingTask"/>
		<rdfs:label>fusion task</rdfs:label>
		<skos:definition>reshaping task that consists in combining two resources into a new, distinct resource</skos:definition>
		<skos:note>conceptually equivalent to structuring two or more resources by construction, then flattening the structure so obtained</skos:note>
	</owl:Class>
	
	<owl:Class rdf:about="&api4kp-ops;HorizontalKnowledgeProcessingTask">
		<rdfs:subClassOf rdf:resource="&api4kp-ops;SyntacticKnowledgeProcessingTask"/>
		<rdfs:subClassOf>
			<owl:Restriction>
				<owl:onProperty rdf:resource="&api4kp-ops;involvesRole"/>
				<owl:someValuesFrom>
					<owl:Class>
						<owl:intersectionOf rdf:parseType="Collection">
							<rdf:Description rdf:about="&api4kp-ops;Input">
							</rdf:Description>
							<owl:Restriction>
								<owl:onProperty rdf:resource="&api4kp-ops;isFilledBy"/>
								<owl:someValuesFrom rdf:resource="&api4kp;KnowledgeResource"/>
							</owl:Restriction>
						</owl:intersectionOf>
					</owl:Class>
				</owl:someValuesFrom>
			</owl:Restriction>
		</rdfs:subClassOf>
		<rdfs:subClassOf>
			<owl:Restriction>
				<owl:onProperty rdf:resource="&api4kp-ops;involvesRole"/>
				<owl:someValuesFrom>
					<owl:Class>
						<owl:intersectionOf rdf:parseType="Collection">
							<rdf:Description rdf:about="&api4kp-ops;Product">
							</rdf:Description>
							<owl:Restriction>
								<owl:onProperty rdf:resource="&api4kp-ops;isFilledBy"/>
								<owl:someValuesFrom rdf:resource="&api4kp;KnowledgeResource"/>
							</owl:Restriction>
						</owl:intersectionOf>
					</owl:Class>
				</owl:someValuesFrom>
			</owl:Restriction>
		</rdfs:subClassOf>
		<rdfs:subClassOf>
			<owl:Restriction>
				<owl:onProperty rdf:resource="&api4kp-ops;retains"/>
				<owl:someValuesFrom rdf:resource="&api4kp;WorkOfKnowledge"/>
			</owl:Restriction>
		</rdfs:subClassOf>
		<rdfs:label>horizontal knowledge processing task</rdfs:label>
		<skos:definition>syntactic processing task that consumes and produces resources at the same level of abstraction, altering the primary characteristic that is defined at level of abstraction (abstract syntax/lexicon, concrete syntax, encoding)</skos:definition>
		<skos:note>While the input I and the product O are different entities, both will refer to the same entities at the higher levels of abstraction: i.e. lift(O) sameAs lift(I), where &apos;lift&apos; is the execution of any lifting vertical task</skos:note>
	</owl:Class>
	
	<owl:Class rdf:about="&api4kp-ops;InferenceTask">
		<rdfs:subClassOf rdf:resource="&api4kp-ops;LogicBasedReasoningTask"/>
		<rdfs:subClassOf>
			<owl:Restriction>
				<owl:onProperty rdf:resource="&api4kp-ops;involvesRole"/>
				<owl:someValuesFrom>
					<owl:Class>
						<owl:intersectionOf rdf:parseType="Collection">
							<rdf:Description rdf:about="&api4kp-ops;Product">
							</rdf:Description>
							<owl:Restriction>
								<owl:onProperty rdf:resource="&api4kp-ops;isFilledBy"/>
								<owl:someValuesFrom rdf:resource="&api4kp;KnowledgeResource"/>
							</owl:Restriction>
						</owl:intersectionOf>
					</owl:Class>
				</owl:someValuesFrom>
			</owl:Restriction>
		</rdfs:subClassOf>
		<rdfs:subClassOf>
			<owl:Restriction>
				<owl:onProperty rdf:resource="&api4kp-ops;involvesRole"/>
				<owl:someValuesFrom>
					<owl:Class>
						<owl:intersectionOf rdf:parseType="Collection">
							<rdf:Description rdf:about="&api4kp-ops;Substrate">
							</rdf:Description>
							<owl:Restriction>
								<owl:onProperty rdf:resource="&api4kp-ops;isFilledBy"/>
								<owl:someValuesFrom rdf:resource="&api4kp-krr;KnowledgeBase"/>
							</owl:Restriction>
						</owl:intersectionOf>
					</owl:Class>
				</owl:someValuesFrom>
			</owl:Restriction>
		</rdfs:subClassOf>
		<rdfs:label>inference task</rdfs:label>
		<rdfs:seeAlso>https://en.wikipedia.org/wiki/Logical_consequence</rdfs:seeAlso>
		<skos:definition>reasoning task that materializes the logical consequence(s) entailed by a given knowledge base</skos:definition>
		<skos:scopeNote>The inferred knowledge may be returned independently, or added to (a new version of) the input knowledge base</skos:scopeNote>
	</owl:Class>
	
	<owl:Class rdf:about="&api4kp-ops;InjectionTask">
		<rdfs:subClassOf rdf:resource="&api4kp-ops;FusionTask"/>
		<rdfs:label>injection task</rdfs:label>
		<skos:definition>fusion in terms of an implicit tree-oriented structure.</skos:definition>
	</owl:Class>
	
	<owl:Class rdf:about="&api4kp-ops;Input">
		<rdfs:subClassOf rdf:resource="&api4kp-ops;KnowledgeProcessingTaskRole"/>
		<rdfs:label>input</rdfs:label>
		<skos:definition>role played by a resource that is used in an activity of a given type, exists before that activity is started, and is made available to the agent executing that activity by a different party</skos:definition>
	</owl:Class>
	
	<owl:Class rdf:about="&api4kp-ops;InterpretationTask">
		<rdfs:subClassOf rdf:resource="&api4kp-ops;LiftingTask"/>
		<rdfs:subClassOf>
			<owl:Restriction>
				<owl:onProperty rdf:resource="&api4kp-ops;involvesRole"/>
				<owl:someValuesFrom>
					<owl:Class>
						<owl:intersectionOf rdf:parseType="Collection">
							<rdf:Description rdf:about="&api4kp-ops;Input">
							</rdf:Description>
							<owl:Restriction>
								<owl:onProperty rdf:resource="&api4kp-ops;isFilledBy"/>
								<owl:someValuesFrom rdf:resource="&api4kp-lang;AbstractSyntaxTree"/>
							</owl:Restriction>
						</owl:intersectionOf>
					</owl:Class>
				</owl:someValuesFrom>
			</owl:Restriction>
		</rdfs:subClassOf>
		<rdfs:subClassOf>
			<owl:Restriction>
				<owl:onProperty rdf:resource="&api4kp-ops;involvesRole"/>
				<owl:someValuesFrom>
					<owl:Class>
						<owl:intersectionOf rdf:parseType="Collection">
							<rdf:Description rdf:about="&api4kp-ops;Product">
							</rdf:Description>
							<owl:Restriction>
								<owl:onProperty rdf:resource="&api4kp-ops;isFilledBy"/>
								<owl:someValuesFrom rdf:resource="&api4kp;WorkOfKnowledge"/>
							</owl:Restriction>
						</owl:intersectionOf>
					</owl:Class>
				</owl:someValuesFrom>
			</owl:Restriction>
		</rdfs:subClassOf>
		<rdfs:label>interpretation task</rdfs:label>
		<skos:altLabel>conceptualization task</skos:altLabel>
		<skos:definition>The act of extracting the information content expressed by a knowledge expression, by means of analyzing the AST of that expression</skos:definition>
	</owl:Class>
	
	<owl:Class rdf:about="&api4kp-ops;KnowledgeAnalyticTask">
		<rdfs:subClassOf rdf:resource="&api4kp-ops;SyntacticKnowledgeProcessingTask"/>
		<rdfs:label>knowledge analytic task</rdfs:label>
		<skos:definition>task whose objective is the determination of a quality of a knowledge expression (e.g. used language, complexity, etc.)</skos:definition>
	</owl:Class>
	
	<owl:Class rdf:about="&api4kp-ops;KnowledgeArtifactRegistrationTask">
		<rdfs:subClassOf rdf:resource="&api4kp-ops;KnowledgeAssetRepositoryTask"/>
		<rdfs:subClassOf>
			<owl:Restriction>
				<owl:onProperty rdf:resource="&api4kp-ops;involvesRole"/>
				<owl:someValuesFrom>
					<owl:Class>
						<owl:intersectionOf rdf:parseType="Collection">
							<rdf:Description rdf:about="&api4kp-ops;Input">
							</rdf:Description>
							<owl:Restriction>
								<owl:onProperty rdf:resource="&api4kp-ops;isFilledBy"/>
								<owl:someValuesFrom>
									<owl:Restriction>
										<owl:onProperty rdf:resource="&api4kp-ops;isCopyOf"/>
										<owl:someValuesFrom rdf:resource="&api4kp;KnowledgeArtifact"/>
									</owl:Restriction>
								</owl:someValuesFrom>
							</owl:Restriction>
						</owl:intersectionOf>
					</owl:Class>
				</owl:someValuesFrom>
			</owl:Restriction>
		</rdfs:subClassOf>
		<rdfs:label>knowledge artifact registration task</rdfs:label>
		<skos:definition>knowledge asset repository task that involves the association of a knowledge artifact (and/or surrogate) with a knowledge asset</skos:definition>
	</owl:Class>
	
	<owl:Class rdf:about="&api4kp-ops;KnowledgeArtifactRepositoryTask">
		<rdfs:subClassOf rdf:resource="&api4kp;KnowledgeProcessingTask"/>
		<rdfs:subClassOf>
			<owl:Restriction>
				<owl:onProperty rdf:resource="&api4kp-ops;involvesRole"/>
				<owl:someValuesFrom>
					<owl:Class>
						<owl:intersectionOf rdf:parseType="Collection">
							<rdf:Description rdf:about="&api4kp-ops;Input">
							</rdf:Description>
							<owl:Restriction>
								<owl:onProperty rdf:resource="&api4kp-ops;isFilledBy"/>
								<owl:someValuesFrom rdf:resource="&api4kp-series;VersionIdentifier"/>
							</owl:Restriction>
						</owl:intersectionOf>
					</owl:Class>
				</owl:someValuesFrom>
			</owl:Restriction>
		</rdfs:subClassOf>
		<rdfs:subClassOf>
			<owl:Restriction>
				<owl:onProperty rdf:resource="&api4kp-ops;involvesRole"/>
				<owl:someValuesFrom>
					<owl:Class>
						<owl:intersectionOf rdf:parseType="Collection">
							<rdf:Description rdf:about="&api4kp-ops;KnowledgeProcessingTaskRole">
							</rdf:Description>
							<owl:Restriction>
								<owl:onProperty rdf:resource="&api4kp-ops;isFilledBy"/>
								<owl:someValuesFrom rdf:resource="&api4kp;KnowledgeArtifact"/>
							</owl:Restriction>
						</owl:intersectionOf>
					</owl:Class>
				</owl:someValuesFrom>
			</owl:Restriction>
		</rdfs:subClassOf>
		<rdfs:label>knowledge artifact repository task</rdfs:label>
		<skos:definition>knowledge processing task focused on the storage, indexing and retrieval of specific versions of knowledge artifacts inside a repository&apos;s storage locations</skos:definition>
		<skos:note>Locations are logical entities, identified by a (location) identifier, regardless of the specific repository implementation, providing abstraction on a persistence layer.</skos:note>
	</owl:Class>
	
	<owl:Class rdf:about="&api4kp-ops;KnowledgeAssetRegistrationTask">
		<rdfs:subClassOf rdf:resource="&api4kp-ops;KnowledgeAssetRepositoryTask"/>
		<rdfs:subClassOf>
			<owl:Restriction>
				<owl:onProperty rdf:resource="&api4kp-ops;involvesRole"/>
				<owl:someValuesFrom>
					<owl:Class>
						<owl:intersectionOf rdf:parseType="Collection">
							<rdf:Description rdf:about="&api4kp-ops;Input">
							</rdf:Description>
							<owl:Restriction>
								<owl:onProperty rdf:resource="&api4kp-ops;isFilledBy"/>
								<owl:someValuesFrom>
									<owl:Restriction>
										<owl:onProperty rdf:resource="&api4kp-ops;isCopyOf"/>
										<owl:someValuesFrom rdf:resource="&api4kp;KnowledgeAssetSurrogate"/>
									</owl:Restriction>
								</owl:someValuesFrom>
							</owl:Restriction>
						</owl:intersectionOf>
					</owl:Class>
				</owl:someValuesFrom>
			</owl:Restriction>
		</rdfs:subClassOf>
		<rdfs:label>knowledge asset registration task</rdfs:label>
		<skos:definition>knowledge asset repository task that adds a Knowledge Asset to the repository, creating a Surrogate in the process</skos:definition>
	</owl:Class>
	
	<owl:Class rdf:about="&api4kp-ops;KnowledgeAssetRepositoryTask">
		<rdfs:subClassOf rdf:resource="&api4kp;KnowledgeProcessingTask"/>
		<rdfs:subClassOf>
			<owl:Restriction>
				<owl:onProperty rdf:resource="&api4kp-ops;involvesRole"/>
				<owl:someValuesFrom>
					<owl:Class>
						<owl:intersectionOf rdf:parseType="Collection">
							<rdf:Description rdf:about="&api4kp-ops;Substrate">
							</rdf:Description>
							<owl:Restriction>
								<owl:onProperty rdf:resource="&api4kp-ops;isFilledBy"/>
								<owl:someValuesFrom rdf:resource="&api4kp;KnowledgeAsset"/>
							</owl:Restriction>
						</owl:intersectionOf>
					</owl:Class>
				</owl:someValuesFrom>
			</owl:Restriction>
		</rdfs:subClassOf>
		<rdfs:label>knowledge asset repository task</rdfs:label>
		<skos:definition>knowledge processing task focused on the indexing, storage and retrieval of Knowledge Assets, manifested through their carriers and/or surrogates</skos:definition>
	</owl:Class>
	
	<owl:Class rdf:about="&api4kp-ops;KnowledgeBaseBuildingTask">
		<rdfs:subClassOf rdf:resource="&api4kp-ops;KnowledgeResourceAssemblyTask"/>
		<rdfs:subClassOf>
			<owl:Restriction>
				<owl:onProperty rdf:resource="&api4kp-ops;involvesRole"/>
				<owl:someValuesFrom>
					<owl:Class>
						<owl:intersectionOf rdf:parseType="Collection">
							<rdf:Description rdf:about="&api4kp-ops;Product">
							</rdf:Description>
							<owl:Restriction>
								<owl:onProperty rdf:resource="&api4kp-ops;isFilledBy"/>
								<owl:someValuesFrom rdf:resource="&api4kp-krr;KnowledgeBase"/>
							</owl:Restriction>
						</owl:intersectionOf>
					</owl:Class>
				</owl:someValuesFrom>
			</owl:Restriction>
		</rdfs:subClassOf>
		<rdfs:subClassOf>
			<owl:Restriction>
				<owl:onProperty rdf:resource="&api4kp-ops;involvesRole"/>
				<owl:someValuesFrom>
					<owl:Class>
						<owl:intersectionOf rdf:parseType="Collection">
							<rdf:Description rdf:about="&api4kp-ops;Substrate">
							</rdf:Description>
							<owl:Restriction>
								<owl:onProperty rdf:resource="&api4kp-ops;isFilledBy"/>
								<owl:someValuesFrom rdf:resource="&api4kp-krr;KnowledgeBase"/>
							</owl:Restriction>
						</owl:intersectionOf>
					</owl:Class>
				</owl:someValuesFrom>
			</owl:Restriction>
		</rdfs:subClassOf>
		<rdfs:label>knowledge base building task</rdfs:label>
		<skos:definition>incremental assembly task that operates on a knowledge base, to produce a new knowledge base that incorporates some additional knowledge resource</skos:definition>
	</owl:Class>
	
	<owl:Class rdf:about="&api4kp-ops;KnowledgeCarrierRetrievalTask">
		<rdfs:subClassOf rdf:resource="&api4kp-ops;KnowledgeAssetRepositoryTask"/>
		<rdfs:subClassOf>
			<owl:Restriction>
				<owl:onProperty rdf:resource="&api4kp-ops;involvesRole"/>
				<owl:someValuesFrom>
					<owl:Class>
						<owl:intersectionOf rdf:parseType="Collection">
							<rdf:Description rdf:about="&api4kp-ops;Input">
							</rdf:Description>
							<owl:Restriction>
								<owl:onProperty rdf:resource="&api4kp-ops;isFilledBy"/>
								<owl:someValuesFrom rdf:resource="&lcc-lr;Identifier"/>
							</owl:Restriction>
						</owl:intersectionOf>
					</owl:Class>
				</owl:someValuesFrom>
			</owl:Restriction>
		</rdfs:subClassOf>
		<rdfs:subClassOf>
			<owl:Restriction>
				<owl:onProperty rdf:resource="&api4kp-ops;involvesRole"/>
				<owl:someValuesFrom>
					<owl:Class>
						<owl:intersectionOf rdf:parseType="Collection">
							<rdf:Description rdf:about="&api4kp-ops;Product">
							</rdf:Description>
							<owl:Restriction>
								<owl:onProperty rdf:resource="&api4kp-ops;isFilledBy"/>
								<owl:someValuesFrom>
									<owl:Restriction>
										<owl:onProperty rdf:resource="&api4kp-ops;isCopyOf"/>
										<owl:someValuesFrom rdf:resource="&api4kp;KnowledgeArtifact"/>
									</owl:Restriction>
								</owl:someValuesFrom>
							</owl:Restriction>
						</owl:intersectionOf>
					</owl:Class>
				</owl:someValuesFrom>
			</owl:Restriction>
		</rdfs:subClassOf>
		<rdfs:label>knowledge carrier retrieval task</rdfs:label>
		<skos:definition>retrieves a knowledge artifact that is the carrier of (a given version of) a knowledge asset, possibly choosing between variant carriers using content negotiation</skos:definition>
	</owl:Class>
	
	<owl:Class rdf:about="&api4kp-ops;KnowledgeProcessingActivity">
		<rdfs:subClassOf rdf:resource="&api4kp;Activity"/>
		<rdfs:label>knowledge processing activity</rdfs:label>
		<skos:definition>(planned) activity that realizes a knowledge processing task, according to a method that specifies how to execute the task</skos:definition>
		<skos:note>knowledge processing activities involve knowledge resources, playing the role of inputs, outputs and substrates, and have reasoning agents as participants.</skos:note>
	</owl:Class>
	
	<owl:Class rdf:about="&api4kp-ops;KnowledgeProcessingTaskRole">
		<rdfs:subClassOf rdf:resource="&api4kp;DefinedConcept"/>
		<rdfs:label>knowledge processing task role</rdfs:label>
		<skos:definition>role type that is played by a resource in the context of a knowledge processing activity</skos:definition>
		<skos:editorialNote>Individual Task Roles allow to define specific roles tailored to specific Knowledge Processing Tasks, and those are the roles &apos;filled by&apos; the individual resources involved in individual activities</skos:editorialNote>
	</owl:Class>
	
	<owl:Class rdf:about="&api4kp-ops;KnowledgeReasoningTask">
		<rdfs:subClassOf rdf:resource="&api4kp;KnowledgeProcessingTask"/>
		<rdfs:subClassOf>
			<owl:Restriction>
				<owl:onProperty rdf:resource="&api4kp-ops;involvesRole"/>
				<owl:someValuesFrom>
					<owl:Restriction>
						<owl:onProperty rdf:resource="&api4kp-ops;isFilledBy"/>
						<owl:someValuesFrom rdf:resource="&api4kp-krr;KnowledgeBase"/>
					</owl:Restriction>
				</owl:someValuesFrom>
			</owl:Restriction>
		</rdfs:subClassOf>
		<rdfs:label>knowledge reasoning task</rdfs:label>
		<skos:definition>knowledge processing task involving an agent with reasoning capabilities, that derives new information leveraging the formal semantics of a working knowledge base</skos:definition>
	</owl:Class>
	
	<owl:Class rdf:about="&api4kp-ops;KnowledgeReshapingTask">
		<rdfs:subClassOf rdf:resource="&api4kp-ops;KnowledgeResourceStructuringTask"/>
		<rdfs:subClassOf>
			<owl:Restriction>
				<owl:onProperty rdf:resource="&api4kp-ops;involvesRole"/>
				<owl:someValuesFrom>
					<owl:Class>
						<owl:intersectionOf rdf:parseType="Collection">
							<rdf:Description rdf:about="&api4kp-ops;Input">
							</rdf:Description>
							<owl:Restriction>
								<owl:onProperty rdf:resource="&api4kp-ops;isFilledBy"/>
								<owl:someValuesFrom rdf:resource="&api4kp;KnowledgeExpression"/>
							</owl:Restriction>
						</owl:intersectionOf>
					</owl:Class>
				</owl:someValuesFrom>
			</owl:Restriction>
		</rdfs:subClassOf>
		<rdfs:subClassOf>
			<owl:Restriction>
				<owl:onProperty rdf:resource="&api4kp-ops;involvesRole"/>
				<owl:someValuesFrom>
					<owl:Class>
						<owl:intersectionOf rdf:parseType="Collection">
							<rdf:Description rdf:about="&api4kp-ops;Product">
							</rdf:Description>
							<owl:Restriction>
								<owl:onProperty rdf:resource="&api4kp-ops;isFilledBy"/>
								<owl:someValuesFrom rdf:resource="&api4kp;KnowledgeExpression"/>
							</owl:Restriction>
						</owl:intersectionOf>
					</owl:Class>
				</owl:someValuesFrom>
			</owl:Restriction>
		</rdfs:subClassOf>
		<rdfs:subClassOf>
			<owl:Restriction>
				<owl:onProperty rdf:resource="&api4kp-ops;involvesRole"/>
				<owl:someValuesFrom>
					<owl:Class>
						<owl:intersectionOf rdf:parseType="Collection">
							<rdf:Description rdf:about="&api4kp-ops;Substrate">
							</rdf:Description>
							<owl:Restriction>
								<owl:onProperty rdf:resource="&api4kp-ops;isFilledBy"/>
								<owl:someValuesFrom rdf:resource="&api4kp;KnowledgeFragment"/>
							</owl:Restriction>
						</owl:intersectionOf>
					</owl:Class>
				</owl:someValuesFrom>
			</owl:Restriction>
		</rdfs:subClassOf>
		<rdfs:subClassOf>
			<owl:Restriction>
				<owl:onProperty rdf:resource="&api4kp-ops;retains"/>
				<owl:someValuesFrom rdf:resource="&lcc-lr;Language"/>
			</owl:Restriction>
		</rdfs:subClassOf>
		<rdfs:label>knowledge reshaping task</rdfs:label>
		<skos:definition>structuring task that produces a knowledge expression, operating on knowledge fragments (and concepts thereof), preserving the language(s) of the input resources in the process</skos:definition>
	</owl:Class>
	
	<owl:Class rdf:about="&api4kp-ops;KnowledgeResourceAggregationTask">
		<rdfs:subClassOf rdf:resource="&api4kp-ops;KnowledgeResourceConstructionTask"/>
		<rdfs:label>knowledge resource aggregation task</rdfs:label>
		<skos:definition>task involving the construction of a set-oriented or other combined structure</skos:definition>
	</owl:Class>
	
	<owl:Class rdf:about="&api4kp-ops;KnowledgeResourceAssemblyTask">
		<rdfs:subClassOf rdf:resource="&api4kp-ops;KnowledgeResourceCompositionalTask"/>
		<rdfs:subClassOf>
			<owl:Restriction>
				<owl:onProperty rdf:resource="&api4kp-ops;involvesRole"/>
				<owl:someValuesFrom>
					<owl:Class>
						<owl:intersectionOf rdf:parseType="Collection">
							<rdf:Description rdf:about="&api4kp-ops;Input">
							</rdf:Description>
							<owl:Restriction>
								<owl:onProperty rdf:resource="&api4kp-ops;isFilledBy"/>
								<owl:someValuesFrom rdf:resource="&api4kp;KnowledgeResource"/>
							</owl:Restriction>
						</owl:intersectionOf>
					</owl:Class>
				</owl:someValuesFrom>
			</owl:Restriction>
		</rdfs:subClassOf>
		<rdfs:subClassOf>
			<owl:Restriction>
				<owl:onProperty rdf:resource="&api4kp-ops;involvesRole"/>
				<owl:someValuesFrom>
					<owl:Class>
						<owl:intersectionOf rdf:parseType="Collection">
							<rdf:Description rdf:about="&api4kp-ops;Input">
							</rdf:Description>
							<owl:Restriction>
								<owl:onProperty rdf:resource="&api4kp-ops;isFilledBy"/>
								<owl:someValuesFrom rdf:resource="&api4kp;StructuringKnowledgeExpression"/>
							</owl:Restriction>
						</owl:intersectionOf>
					</owl:Class>
				</owl:someValuesFrom>
			</owl:Restriction>
		</rdfs:subClassOf>
		<rdfs:subClassOf>
			<owl:Restriction>
				<owl:onProperty rdf:resource="&api4kp-ops;involvesRole"/>
				<owl:someValuesFrom>
					<owl:Class>
						<owl:intersectionOf rdf:parseType="Collection">
							<rdf:Description rdf:about="&api4kp-ops;Product">
							</rdf:Description>
							<owl:Restriction>
								<owl:onProperty rdf:resource="&api4kp-ops;isFilledBy"/>
								<owl:someValuesFrom rdf:resource="&api4kp;CompositeKnowledgeResource"/>
							</owl:Restriction>
						</owl:intersectionOf>
					</owl:Class>
				</owl:someValuesFrom>
			</owl:Restriction>
		</rdfs:subClassOf>
		<rdfs:label>knowledge resource assembly task</rdfs:label>
		<skos:note>compositional task that constructs a composite knowledge asset given a structure and the individual components</skos:note>
	</owl:Class>
	
	<owl:Class rdf:about="&api4kp-ops;KnowledgeResourceCompositionTask">
		<rdfs:subClassOf rdf:resource="&api4kp-ops;KnowledgeResourceConstructionTask"/>
		<rdfs:label>knowledge resource composition task</rdfs:label>
		<skos:definition>construction task resulting in a tree-oriented structure</skos:definition>
	</owl:Class>
	
	<owl:Class rdf:about="&api4kp-ops;KnowledgeResourceCompositionalTask">
		<rdfs:subClassOf rdf:resource="&api4kp-ops;KnowledgeResourceStructuringTask"/>
		<rdfs:subClassOf>
			<owl:Restriction>
				<owl:onProperty rdf:resource="&api4kp-ops;involvesRole"/>
				<owl:someValuesFrom>
					<owl:Restriction>
						<owl:onProperty rdf:resource="&api4kp-ops;isFilledBy"/>
						<owl:someValuesFrom rdf:resource="&api4kp;StructuringKnowledgeExpression"/>
					</owl:Restriction>
				</owl:someValuesFrom>
			</owl:Restriction>
		</rdfs:subClassOf>
		<rdfs:label>knowledge resource compositional task</rdfs:label>
		<skos:definition>task that operates on a composite knowledge resource, whose internal organization is manifested by a structuring knowledge resource</skos:definition>
	</owl:Class>
	
	<owl:Class rdf:about="&api4kp-ops;KnowledgeResourceConstructionTask">
		<rdfs:subClassOf rdf:resource="&api4kp-ops;KnowledgeResourceCompositionalTask"/>
		<rdfs:subClassOf>
			<owl:Restriction>
				<owl:onProperty rdf:resource="&api4kp-ops;involvesRole"/>
				<owl:someValuesFrom>
					<owl:Class>
						<owl:intersectionOf rdf:parseType="Collection">
							<rdf:Description rdf:about="&api4kp-ops;Input">
							</rdf:Description>
							<owl:Restriction>
								<owl:onProperty rdf:resource="&api4kp-ops;isFilledBy"/>
								<owl:someValuesFrom rdf:resource="&api4kp;KnowledgeResource"/>
							</owl:Restriction>
						</owl:intersectionOf>
					</owl:Class>
				</owl:someValuesFrom>
			</owl:Restriction>
		</rdfs:subClassOf>
		<rdfs:subClassOf>
			<owl:Restriction>
				<owl:onProperty rdf:resource="&api4kp-ops;involvesRole"/>
				<owl:someValuesFrom>
					<owl:Class>
						<owl:intersectionOf rdf:parseType="Collection">
							<rdf:Description rdf:about="&api4kp-ops;Product">
							</rdf:Description>
							<owl:Restriction>
								<owl:onProperty rdf:resource="&api4kp-ops;isFilledBy"/>
								<owl:someValuesFrom rdf:resource="&api4kp;StructuringKnowledgeExpression"/>
							</owl:Restriction>
						</owl:intersectionOf>
					</owl:Class>
				</owl:someValuesFrom>
			</owl:Restriction>
		</rdfs:subClassOf>
		<rdfs:label>knowledge resource construction task</rdfs:label>
		<skos:definition>compositional task that creates a structuring knowledge resource that has two or more knowledge resources as referenced components</skos:definition>
	</owl:Class>
	
	<owl:Class rdf:about="&api4kp-ops;KnowledgeResourceDecompositionTask">
		<rdfs:subClassOf rdf:resource="&api4kp-ops;KnowledgeResourceDeconstructionTask"/>
		<rdfs:label>knowledge resource decomposition task</rdfs:label>
		<skos:definition>deconstruction task that is limited to operating on tree-oriented structures</skos:definition>
	</owl:Class>
	
	<owl:Class rdf:about="&api4kp-ops;KnowledgeResourceDeconstructionTask">
		<rdfs:subClassOf rdf:resource="&api4kp-ops;KnowledgeResourceCompositionalTask"/>
		<rdfs:subClassOf>
			<owl:Restriction>
				<owl:onProperty rdf:resource="&api4kp-ops;involvesRole"/>
				<owl:someValuesFrom>
					<owl:Class>
						<owl:intersectionOf rdf:parseType="Collection">
							<rdf:Description rdf:about="&api4kp-ops;Input">
							</rdf:Description>
							<owl:Restriction>
								<owl:onProperty rdf:resource="&api4kp-ops;isFilledBy"/>
								<owl:someValuesFrom rdf:resource="&api4kp;KnowledgeResource"/>
							</owl:Restriction>
						</owl:intersectionOf>
					</owl:Class>
				</owl:someValuesFrom>
			</owl:Restriction>
		</rdfs:subClassOf>
		<rdfs:subClassOf>
			<owl:Restriction>
				<owl:onProperty rdf:resource="&api4kp-ops;involvesRole"/>
				<owl:someValuesFrom>
					<owl:Class>
						<owl:intersectionOf rdf:parseType="Collection">
							<rdf:Description rdf:about="&api4kp-ops;Product">
							</rdf:Description>
							<owl:Restriction>
								<owl:onProperty rdf:resource="&api4kp-ops;isFilledBy"/>
								<owl:someValuesFrom rdf:resource="&api4kp;StructuringKnowledgeExpression"/>
							</owl:Restriction>
						</owl:intersectionOf>
					</owl:Class>
				</owl:someValuesFrom>
			</owl:Restriction>
		</rdfs:subClassOf>
		<rdfs:label>knowledge resource deconstruction task</rdfs:label>
		<skos:definition>compositional task that creates a structuring knowledge resource from a single deconstructable resource, i.e. a resources that contains fragments which could be promoted to knowledge expressions</skos:definition>
	</owl:Class>
	
	<owl:Class rdf:about="&api4kp-ops;KnowledgeResourceDescriptionExtractionTask">
		<rdfs:subClassOf rdf:resource="&api4kp-ops;SemanticKnowledgeManagementTask"/>
		<rdfs:subClassOf>
			<owl:Restriction>
				<owl:onProperty rdf:resource="&api4kp-ops;involvesRole"/>
				<owl:someValuesFrom>
					<owl:Class>
						<owl:intersectionOf rdf:parseType="Collection">
							<rdf:Description rdf:about="&api4kp-ops;Input">
							</rdf:Description>
							<owl:Restriction>
								<owl:onProperty rdf:resource="&api4kp-ops;isFilledBy"/>
								<owl:someValuesFrom rdf:resource="&api4kp;KnowledgeExpression"/>
							</owl:Restriction>
						</owl:intersectionOf>
					</owl:Class>
				</owl:someValuesFrom>
			</owl:Restriction>
		</rdfs:subClassOf>
		<rdfs:subClassOf>
			<owl:Restriction>
				<owl:onProperty rdf:resource="&api4kp-ops;involvesRole"/>
				<owl:someValuesFrom>
					<owl:Class>
						<owl:intersectionOf rdf:parseType="Collection">
							<rdf:Description rdf:about="&api4kp-ops;Product">
							</rdf:Description>
							<owl:Restriction>
								<owl:onProperty rdf:resource="&api4kp-ops;isFilledBy"/>
								<owl:someValuesFrom rdf:resource="&api4kp;KnowledgeResourceDescription"/>
							</owl:Restriction>
						</owl:intersectionOf>
					</owl:Class>
				</owl:someValuesFrom>
			</owl:Restriction>
		</rdfs:subClassOf>
		<rdfs:label>knowledge resource description extraction task</rdfs:label>
		<skos:definition>Reasoning Task that infers a Knowledge Resource Description from a Knowledge Expression</skos:definition>
		<skos:note>The produced description is manifested as a Knowlege Asset Surrogate</skos:note>
	</owl:Class>
	
	<owl:Class rdf:about="&api4kp-ops;KnowledgeResourceDisaggregationTask">
		<rdfs:subClassOf rdf:resource="&api4kp-ops;KnowledgeResourceDeconstructionTask"/>
		<rdfs:label>knowledge resource disaggregation task</rdfs:label>
		<skos:definition>deconstruction task that is limited to set-oriented structures</skos:definition>
	</owl:Class>
	
	<owl:Class rdf:about="&api4kp-ops;KnowledgeResourceDisassemblyTask">
		<rdfs:subClassOf rdf:resource="&api4kp-ops;KnowledgeResourceCompositionalTask"/>
		<rdfs:subClassOf>
			<owl:Restriction>
				<owl:onProperty rdf:resource="&api4kp-ops;involvesRole"/>
				<owl:someValuesFrom>
					<owl:Class>
						<owl:intersectionOf rdf:parseType="Collection">
							<rdf:Description rdf:about="&api4kp-ops;Input">
							</rdf:Description>
							<owl:Restriction>
								<owl:onProperty rdf:resource="&api4kp-ops;isFilledBy"/>
								<owl:someValuesFrom rdf:resource="&api4kp;CompositeKnowledgeResource"/>
							</owl:Restriction>
						</owl:intersectionOf>
					</owl:Class>
				</owl:someValuesFrom>
			</owl:Restriction>
		</rdfs:subClassOf>
		<rdfs:subClassOf>
			<owl:Restriction>
				<owl:onProperty rdf:resource="&api4kp-ops;involvesRole"/>
				<owl:someValuesFrom>
					<owl:Class>
						<owl:intersectionOf rdf:parseType="Collection">
							<rdf:Description rdf:about="&api4kp-ops;Input">
							</rdf:Description>
							<owl:Restriction>
								<owl:onProperty rdf:resource="&api4kp-ops;isFilledBy"/>
								<owl:someValuesFrom rdf:resource="&api4kp;StructuringKnowledgeExpression"/>
							</owl:Restriction>
						</owl:intersectionOf>
					</owl:Class>
				</owl:someValuesFrom>
			</owl:Restriction>
		</rdfs:subClassOf>
		<rdfs:subClassOf>
			<owl:Restriction>
				<owl:onProperty rdf:resource="&api4kp-ops;involvesRole"/>
				<owl:someValuesFrom>
					<owl:Class>
						<owl:intersectionOf rdf:parseType="Collection">
							<rdf:Description rdf:about="&api4kp-ops;Product">
							</rdf:Description>
							<owl:Restriction>
								<owl:onProperty rdf:resource="&api4kp-ops;isFilledBy"/>
								<owl:someValuesFrom rdf:resource="&api4kp;KnowledgeResource"/>
							</owl:Restriction>
						</owl:intersectionOf>
					</owl:Class>
				</owl:someValuesFrom>
			</owl:Restriction>
		</rdfs:subClassOf>
		<rdfs:label>knowledge resource disassembly task</rdfs:label>
		<skos:definition>compositional task that consists in breaking apart a composite knowledge resources, to obtain the components as a product</skos:definition>
	</owl:Class>
	
	<owl:Class rdf:about="&api4kp-ops;KnowledgeResourceDiscoveryTask">
		<rdfs:subClassOf rdf:resource="&api4kp-ops;SemanticKnowledgeManagementTask"/>
		<rdfs:subClassOf>
			<owl:Restriction>
				<owl:onProperty rdf:resource="&api4kp-ops;hasSubtask"/>
				<owl:someValuesFrom rdf:resource="&api4kp-ops;QueryAnswerTask"/>
			</owl:Restriction>
		</rdfs:subClassOf>
		<rdfs:subClassOf>
			<owl:Restriction>
				<owl:onProperty rdf:resource="&api4kp-ops;involvesRole"/>
				<owl:someValuesFrom>
					<owl:Class>
						<owl:intersectionOf rdf:parseType="Collection">
							<rdf:Description rdf:about="&api4kp-ops;Input">
							</rdf:Description>
							<owl:Restriction>
								<owl:onProperty rdf:resource="&api4kp-ops;isFilledBy"/>
								<owl:someValuesFrom rdf:resource="&api4kp;KnowledgeResource"/>
							</owl:Restriction>
						</owl:intersectionOf>
					</owl:Class>
				</owl:someValuesFrom>
			</owl:Restriction>
		</rdfs:subClassOf>
		<rdfs:subClassOf>
			<owl:Restriction>
				<owl:onProperty rdf:resource="&api4kp-ops;involvesRole"/>
				<owl:someValuesFrom>
					<owl:Class>
						<owl:intersectionOf rdf:parseType="Collection">
							<rdf:Description rdf:about="&api4kp-ops;Product">
							</rdf:Description>
							<owl:Restriction>
								<owl:onProperty rdf:resource="&api4kp-ops;isFilledBy"/>
								<owl:someValuesFrom rdf:resource="&api4kp;KnowledgeResource"/>
							</owl:Restriction>
						</owl:intersectionOf>
					</owl:Class>
				</owl:someValuesFrom>
			</owl:Restriction>
		</rdfs:subClassOf>
		<rdfs:label>knowledge resource discovery task</rdfs:label>
		<skos:definition>knowledge management task that, given a knowledge asset repository, determines the knowledge resources that match some search/query criteria applied to the resources metadata</skos:definition>
	</owl:Class>
	
	<owl:Class rdf:about="&api4kp-ops;KnowledgeResourceFlatteningTask">
		<rdfs:subClassOf rdf:resource="&api4kp-ops;KnowledgeResourceCompositionalTask"/>
		<rdfs:subClassOf>
			<owl:Restriction>
				<owl:onProperty rdf:resource="&api4kp-ops;involvesRole"/>
				<owl:someValuesFrom>
					<owl:Restriction>
						<owl:onProperty rdf:resource="&api4kp-ops;isFilledBy"/>
						<owl:someValuesFrom rdf:resource="&api4kp;StructuringKnowledgeExpression"/>
					</owl:Restriction>
				</owl:someValuesFrom>
			</owl:Restriction>
		</rdfs:subClassOf>
		<rdfs:subClassOf>
			<owl:Restriction>
				<owl:onProperty rdf:resource="&api4kp-ops;involvesRole"/>
				<owl:someValuesFrom>
					<owl:Class>
						<owl:intersectionOf rdf:parseType="Collection">
							<rdf:Description rdf:about="&api4kp-ops;Input">
							</rdf:Description>
							<owl:Restriction>
								<owl:onProperty rdf:resource="&api4kp-ops;isFilledBy"/>
								<owl:someValuesFrom rdf:resource="&api4kp;CompositeKnowledgeResource"/>
							</owl:Restriction>
						</owl:intersectionOf>
					</owl:Class>
				</owl:someValuesFrom>
			</owl:Restriction>
		</rdfs:subClassOf>
		<rdfs:subClassOf>
			<owl:Restriction>
				<owl:onProperty rdf:resource="&api4kp-ops;involvesRole"/>
				<owl:someValuesFrom>
					<owl:Class>
						<owl:intersectionOf rdf:parseType="Collection">
							<rdf:Description rdf:about="&api4kp-ops;Product">
							</rdf:Description>
							<owl:Restriction>
								<owl:onProperty rdf:resource="&api4kp-ops;isFilledBy"/>
								<owl:someValuesFrom rdf:resource="&api4kp;KnowledgeResource"/>
							</owl:Restriction>
						</owl:intersectionOf>
					</owl:Class>
				</owl:someValuesFrom>
			</owl:Restriction>
		</rdfs:subClassOf>
		<rdfs:label>knowledge resource flattening task</rdfs:label>
		<skos:definition>compositional task that produces a single, flattened knowledge resource from a composite knowledge resource, respecting the composite&apos;s structure</skos:definition>
		<skos:note>The flattening may require some manipulation of the component resources before they can be merged</skos:note>
	</owl:Class>
	
	<owl:Class rdf:about="&api4kp-ops;KnowledgeResourceRearrangementTask">
		<rdfs:subClassOf rdf:resource="&api4kp-ops;KnowledgeResourceCompositionalTask"/>
		<rdfs:subClassOf>
			<owl:Restriction>
				<owl:onProperty rdf:resource="&api4kp-ops;involvesRole"/>
				<owl:someValuesFrom>
					<owl:Class>
						<owl:intersectionOf rdf:parseType="Collection">
							<rdf:Description rdf:about="&api4kp-ops;Input">
							</rdf:Description>
							<owl:Restriction>
								<owl:onProperty rdf:resource="&api4kp-ops;isFilledBy"/>
								<owl:someValuesFrom rdf:resource="&api4kp;StructuringKnowledgeExpression"/>
							</owl:Restriction>
						</owl:intersectionOf>
					</owl:Class>
				</owl:someValuesFrom>
			</owl:Restriction>
		</rdfs:subClassOf>
		<rdfs:subClassOf>
			<owl:Restriction>
				<owl:onProperty rdf:resource="&api4kp-ops;involvesRole"/>
				<owl:someValuesFrom>
					<owl:Class>
						<owl:intersectionOf rdf:parseType="Collection">
							<rdf:Description rdf:about="&api4kp-ops;Product">
							</rdf:Description>
							<owl:Restriction>
								<owl:onProperty rdf:resource="&api4kp-ops;isFilledBy"/>
								<owl:someValuesFrom rdf:resource="&api4kp;StructuringKnowledgeExpression"/>
							</owl:Restriction>
						</owl:intersectionOf>
					</owl:Class>
				</owl:someValuesFrom>
			</owl:Restriction>
		</rdfs:subClassOf>
		<rdfs:label>knowledge resource rearrangement task</rdfs:label>
		<skos:definition>compositional task that retains the identity and type of the components, but alters the mutual relationships</skos:definition>
		<skos:note>That is, the corresponding Composites have the same atomic components, but the underlying set-tree organization is different</skos:note>
		<skos:note>The operation generates a new structure, that is a versioned revision of the input structure</skos:note>
	</owl:Class>
	
	<owl:Class rdf:about="&api4kp-ops;KnowledgeResourceStructuringTask">
		<rdfs:subClassOf rdf:resource="&api4kp;KnowledgeProcessingTask"/>
		<rdfs:subClassOf>
			<owl:Class>
				<owl:complementOf>
					<owl:Restriction>
						<owl:onProperty rdf:resource="&api4kp-ops;retains"/>
						<owl:someValuesFrom rdf:resource="&api4kp;WorkOfKnowledge"/>
					</owl:Restriction>
				</owl:complementOf>
			</owl:Class>
		</rdfs:subClassOf>
		<rdfs:label>knowledge resource structuring task</rdfs:label>
		<skos:definition>task that produces a derivative knowledge resource that embodies a derivative work of knowledge</skos:definition>
		<skos:scopeNote>In API4KP a &apos;structure&apos; denotes, in a narrow sense, two or more resources organized into composite resources. In DOL, &apos;structuring&apos; is used in a broader sense, not only to cover the API4KP sense, but also the API4KP notion of &apos;(complex) manipulation&apos; - operations that are possibly, but not necessarily, used to prepare resources to become part of a structure.

To remain aligned, in API4KP &apos;structuring&apos; denotes manipulations other than &apos;horizontal&apos; and &apos;vertical&apos; manipulations which preserve the work of knowledge.  Hence, &apos;structuring&apos; tasks do not preserve the WoK. &apos;Structuring&apos; is then further partitioned into &apos;Composition&apos; - dealing with API4KP structures and composite resources - and &apos;Reshaping&apos; - dealing with non-WoK preserving transrepresentations.</skos:scopeNote>
	</owl:Class>
	
	<owl:Class rdf:about="&api4kp-ops;KnowledgeSurrogateRetrievalTask">
		<rdfs:subClassOf rdf:resource="&api4kp-ops;KnowledgeCarrierRetrievalTask"/>
		<rdfs:subClassOf>
			<owl:Restriction>
				<owl:onProperty rdf:resource="&api4kp-ops;involvesRole"/>
				<owl:someValuesFrom>
					<owl:Class>
						<owl:intersectionOf rdf:parseType="Collection">
							<rdf:Description rdf:about="&api4kp-ops;Product">
							</rdf:Description>
							<owl:Restriction>
								<owl:onProperty rdf:resource="&api4kp-ops;isFilledBy"/>
								<owl:allValuesFrom>
									<owl:Restriction>
										<owl:onProperty rdf:resource="&api4kp-ops;isCopyOf"/>
										<owl:someValuesFrom rdf:resource="&api4kp;KnowledgeAssetSurrogate"/>
									</owl:Restriction>
								</owl:allValuesFrom>
							</owl:Restriction>
						</owl:intersectionOf>
					</owl:Class>
				</owl:someValuesFrom>
			</owl:Restriction>
		</rdfs:subClassOf>
		<rdfs:label>knowledge surrogate retrieval task</rdfs:label>
		<skos:definition>knowledge carrier retrieval task that returns a surrogate</skos:definition>
	</owl:Class>
	
	<owl:Class rdf:about="&api4kp-ops;LanguageInformationDetectionTask">
		<rdfs:subClassOf rdf:resource="&api4kp-ops;KnowledgeAnalyticTask"/>
		<rdfs:subClassOf>
			<owl:Restriction>
				<owl:onProperty rdf:resource="&api4kp-ops;hasSubtask"/>
				<owl:someValuesFrom rdf:resource="&api4kp-ops;ParsingTask"/>
			</owl:Restriction>
		</rdfs:subClassOf>
		<rdfs:subClassOf>
			<owl:Restriction>
				<owl:onProperty rdf:resource="&api4kp-ops;involvesRole"/>
				<owl:someValuesFrom>
					<owl:Class>
						<owl:intersectionOf rdf:parseType="Collection">
							<rdf:Description rdf:about="&api4kp-ops;Product">
							</rdf:Description>
							<owl:Restriction>
								<owl:onProperty rdf:resource="&api4kp-ops;isFilledBy"/>
								<owl:someValuesFrom rdf:resource="&dol;Profile"/>
							</owl:Restriction>
						</owl:intersectionOf>
					</owl:Class>
				</owl:someValuesFrom>
			</owl:Restriction>
		</rdfs:subClassOf>
		<rdfs:subClassOf>
			<owl:Restriction>
				<owl:onProperty rdf:resource="&api4kp-ops;involvesRole"/>
				<owl:someValuesFrom>
					<owl:Class>
						<owl:intersectionOf rdf:parseType="Collection">
							<rdf:Description rdf:about="&api4kp-ops;Product">
							</rdf:Description>
							<owl:Restriction>
								<owl:onProperty rdf:resource="&api4kp-ops;isFilledBy"/>
								<owl:someValuesFrom rdf:resource="&api4kp-lang;Serialization"/>
							</owl:Restriction>
						</owl:intersectionOf>
					</owl:Class>
				</owl:someValuesFrom>
			</owl:Restriction>
		</rdfs:subClassOf>
		<rdfs:subClassOf>
			<owl:Restriction>
				<owl:onProperty rdf:resource="&api4kp-ops;involvesRole"/>
				<owl:someValuesFrom>
					<owl:Class>
						<owl:intersectionOf rdf:parseType="Collection">
							<rdf:Description rdf:about="&api4kp-ops;Product">
							</rdf:Description>
							<owl:Restriction>
								<owl:onProperty rdf:resource="&api4kp-ops;isFilledBy"/>
								<owl:someValuesFrom rdf:resource="&lcc-lr;Language"/>
							</owl:Restriction>
						</owl:intersectionOf>
					</owl:Class>
				</owl:someValuesFrom>
			</owl:Restriction>
		</rdfs:subClassOf>
		<rdfs:label>language information detection task</rdfs:label>
		<skos:definition>analytic task that detects the language, profile and/or concrete syntax used in a knowledge expression</skos:definition>
	</owl:Class>
	
	<owl:Class rdf:about="&api4kp-ops;LiftingTask">
		<rdfs:subClassOf rdf:resource="&api4kp-ops;VerticalKnowledgeProcessingTask"/>
		<rdfs:label>lifting task</rdfs:label>
		<skos:definition>vertical knowledge processing task that produces a resource at a higher level of abstraction that its input</skos:definition>
	</owl:Class>
	
	<owl:Class rdf:about="&api4kp-ops;LogicBasedReasoningTask">
		<rdfs:subClassOf rdf:resource="&api4kp-ops;KnowledgeReasoningTask"/>
		<rdfs:label>logic-based reasoning task</rdfs:label>
		<skos:definition>knowledge reasoning task based on the semantics and pragmatics of some underlying logic, based on symbolic methods, suitable to be peformed by &apos;reasoners&apos;</skos:definition>
	</owl:Class>
	
	<owl:Class rdf:about="&api4kp-ops;LogicDetectionTask">
		<rdfs:subClassOf rdf:resource="&api4kp-ops;KnowledgeAnalyticTask"/>
		<rdfs:subClassOf>
			<owl:Restriction>
				<owl:onProperty rdf:resource="&api4kp-ops;involvesRole"/>
				<owl:someValuesFrom>
					<owl:Class>
						<owl:intersectionOf rdf:parseType="Collection">
							<rdf:Description rdf:about="&api4kp-ops;Product">
							</rdf:Description>
							<owl:Restriction>
								<owl:onProperty rdf:resource="&api4kp-ops;isFilledBy"/>
								<owl:someValuesFrom rdf:resource="&dol;Logic"/>
							</owl:Restriction>
						</owl:intersectionOf>
					</owl:Class>
				</owl:someValuesFrom>
			</owl:Restriction>
		</rdfs:subClassOf>
		<rdfs:label>logic detection task</rdfs:label>
		<skos:definition>Analytic task that detects the (simplest) logic that is expressive enough to formalize the given Knowledge Expression.</skos:definition>
	</owl:Class>
	
	<owl:Class rdf:about="&api4kp-ops;LoweringTask">
		<rdfs:subClassOf rdf:resource="&api4kp-ops;VerticalKnowledgeProcessingTask"/>
		<rdfs:label>lowering task</rdfs:label>
		<skos:definition>vertical knowledge processing task that produces a resource at a lower level of abstraction that its input</skos:definition>
		<skos:note>with respect to a lowering, there is usually a 1:N relationship between the resource at the higher level and the resource(s) at the lower level</skos:note>
	</owl:Class>
	
	<owl:Class rdf:about="&api4kp-ops;ParaphraseTask">
		<rdfs:subClassOf rdf:resource="&api4kp-ops;HorizontalKnowledgeProcessingTask"/>
		<rdfs:subClassOf>
			<owl:Restriction>
				<owl:onProperty rdf:resource="&api4kp-ops;involvesRole"/>
				<owl:someValuesFrom>
					<owl:Class>
						<owl:intersectionOf rdf:parseType="Collection">
							<rdf:Description rdf:about="&api4kp-ops;Input">
							</rdf:Description>
							<owl:Restriction>
								<owl:onProperty rdf:resource="&api4kp-ops;isFilledBy"/>
								<owl:someValuesFrom rdf:resource="&api4kp;KnowledgeExpression"/>
							</owl:Restriction>
						</owl:intersectionOf>
					</owl:Class>
				</owl:someValuesFrom>
			</owl:Restriction>
		</rdfs:subClassOf>
		<rdfs:subClassOf>
			<owl:Restriction>
				<owl:onProperty rdf:resource="&api4kp-ops;involvesRole"/>
				<owl:someValuesFrom>
					<owl:Class>
						<owl:intersectionOf rdf:parseType="Collection">
							<rdf:Description rdf:about="&api4kp-ops;Product">
							</rdf:Description>
							<owl:Restriction>
								<owl:onProperty rdf:resource="&api4kp-ops;isFilledBy"/>
								<owl:someValuesFrom rdf:resource="&api4kp;KnowledgeExpression"/>
							</owl:Restriction>
						</owl:intersectionOf>
					</owl:Class>
				</owl:someValuesFrom>
			</owl:Restriction>
		</rdfs:subClassOf>
		<rdfs:subClassOf>
			<owl:Restriction>
				<owl:onProperty rdf:resource="&api4kp-ops;retains"/>
				<owl:someValuesFrom rdf:resource="&lcc-lr;Language"/>
			</owl:Restriction>
		</rdfs:subClassOf>
		<rdfs:label>paraphrase task</rdfs:label>
		<skos:definition>horizontal translation task that creates an alternative expression (concrete or abstract) that carries the same meaning, but uses different fragments (sentences and/or linguistic elements).</skos:definition>
		<skos:note>Meaning (work of knowledge), language and format are preserved, but not the internal structure of an expression.</skos:note>
		<skos:note>Paraphrase is only admissible in languages that are redundant, i.e. allow alternative, different expressions of the same meaning</skos:note>
		<skos:scopeNote>Interesting &apos;paraphrases&apos; are the ones that cast an expression, in a given language, within the boundaries of a profile of that language</skos:scopeNote>
	</owl:Class>
	
	<owl:Class rdf:about="&api4kp-ops;ParsingTask">
		<rdfs:subClassOf rdf:resource="&api4kp-ops;LiftingTask"/>
		<rdfs:subClassOf>
			<owl:Restriction>
				<owl:onProperty rdf:resource="&api4kp-ops;involvesRole"/>
				<owl:someValuesFrom>
					<owl:Class>
						<owl:intersectionOf rdf:parseType="Collection">
							<rdf:Description rdf:about="&api4kp-ops;Input">
							</rdf:Description>
							<owl:Restriction>
								<owl:onProperty rdf:resource="&api4kp-ops;isFilledBy"/>
								<owl:someValuesFrom rdf:resource="&api4kp;ConcreteKnowledgeExpression"/>
							</owl:Restriction>
						</owl:intersectionOf>
					</owl:Class>
				</owl:someValuesFrom>
			</owl:Restriction>
		</rdfs:subClassOf>
		<rdfs:subClassOf>
			<owl:Restriction>
				<owl:onProperty rdf:resource="&api4kp-ops;involvesRole"/>
				<owl:someValuesFrom>
					<owl:Class>
						<owl:intersectionOf rdf:parseType="Collection">
							<rdf:Description rdf:about="&api4kp-ops;Product">
							</rdf:Description>
							<owl:Restriction>
								<owl:onProperty rdf:resource="&api4kp-ops;isFilledBy"/>
								<owl:someValuesFrom rdf:resource="&api4kp;AbstractKnowledgeExpression"/>
							</owl:Restriction>
						</owl:intersectionOf>
					</owl:Class>
				</owl:someValuesFrom>
			</owl:Restriction>
		</rdfs:subClassOf>
		<rdfs:label>parsing task</rdfs:label>
		<skos:definition>the act of creating an AST (of an abstract knowldge expression) from a concrete knowledge expression</skos:definition>
	</owl:Class>
	
	<owl:Class rdf:about="&api4kp-ops;PartitionTask">
		<rdfs:subClassOf rdf:resource="&api4kp-ops;SeparationTask"/>
		<rdfs:label>partition task</rdfs:label>
		<skos:definition>A separation based on a set-oriented deconstruction</skos:definition>
	</owl:Class>
	
	<owl:Class rdf:about="&api4kp-ops;Product">
		<rdfs:subClassOf rdf:resource="&api4kp-ops;KnowledgeProcessingTaskRole"/>
		<rdfs:label>product</rdfs:label>
		<skos:definition>role played by a resource that is used in an activity, and comes into being as a consequence of the successful completion of the activity</skos:definition>
	</owl:Class>
	
	<owl:Class rdf:about="&api4kp-ops;ProofGenerationTask">
		<rdfs:subClassOf rdf:resource="&api4kp-ops;LogicBasedReasoningTask"/>
		<rdfs:subClassOf>
			<owl:Restriction>
				<owl:onProperty rdf:resource="&api4kp-ops;involvesRole"/>
				<owl:someValuesFrom>
					<owl:Class>
						<owl:intersectionOf rdf:parseType="Collection">
							<rdf:Description rdf:about="&api4kp-ops;Explanation">
							</rdf:Description>
							<rdf:Description rdf:about="&api4kp-ops;Product">
							</rdf:Description>
						</owl:intersectionOf>
					</owl:Class>
				</owl:someValuesFrom>
			</owl:Restriction>
		</rdfs:subClassOf>
		<rdfs:label>proof generation task</rdfs:label>
		<skos:definition>Reasoning Tasks that produces a proof, i.e. an Explanation of how a Knowledge Base is entailed by another Knowledge Base</skos:definition>
	</owl:Class>
	
	<owl:Class rdf:about="&api4kp-ops;QueryAnswerTask">
		<rdfs:subClassOf rdf:resource="&api4kp-ops;LogicBasedReasoningTask"/>
		<rdfs:subClassOf>
			<owl:Restriction>
				<owl:onProperty rdf:resource="&api4kp-ops;involvesRole"/>
				<owl:someValuesFrom>
					<owl:Class>
						<owl:intersectionOf rdf:parseType="Collection">
							<rdf:Description rdf:about="&api4kp-ops;Input">
							</rdf:Description>
							<owl:Restriction>
								<owl:onProperty rdf:resource="&api4kp-ops;isFilledBy"/>
								<owl:someValuesFrom rdf:resource="&dol;Query"/>
							</owl:Restriction>
						</owl:intersectionOf>
					</owl:Class>
				</owl:someValuesFrom>
			</owl:Restriction>
		</rdfs:subClassOf>
		<rdfs:subClassOf>
			<owl:Restriction>
				<owl:onProperty rdf:resource="&api4kp-ops;involvesRole"/>
				<owl:someValuesFrom>
					<owl:Class>
						<owl:intersectionOf rdf:parseType="Collection">
							<rdf:Description rdf:about="&api4kp-ops;Product">
							</rdf:Description>
							<owl:Restriction>
								<owl:onProperty rdf:resource="&api4kp-ops;isFilledBy"/>
								<owl:someValuesFrom rdf:resource="&api4kp;KnowledgeExpression"/>
							</owl:Restriction>
						</owl:intersectionOf>
					</owl:Class>
				</owl:someValuesFrom>
			</owl:Restriction>
		</rdfs:subClassOf>
		<rdfs:label>query answering task</rdfs:label>
		<skos:definition>Reasoning Task that, given a Working Knowledge Base and a Query, (expressed by means of a proper knowledge expression that contains variables), returns an &apos;answer&apos; in terms of bindings of those variables with respect to the contents of the Knowledge Base</skos:definition>
	</owl:Class>
	
	<owl:Class rdf:about="&api4kp-ops;ReadTask">
		<rdfs:subClassOf rdf:resource="&api4kp-ops;LiftingTask"/>
		<rdfs:subClassOf>
			<owl:Restriction>
				<owl:onProperty rdf:resource="&api4kp-ops;involvesRole"/>
				<owl:someValuesFrom>
					<owl:Class>
						<owl:intersectionOf rdf:parseType="Collection">
							<rdf:Description rdf:about="&api4kp-ops;Input">
							</rdf:Description>
							<owl:Restriction>
								<owl:onProperty rdf:resource="&api4kp-ops;isFilledBy"/>
								<owl:someValuesFrom rdf:resource="&api4kp;ExternalizedKnowledgeExpression"/>
							</owl:Restriction>
						</owl:intersectionOf>
					</owl:Class>
				</owl:someValuesFrom>
			</owl:Restriction>
		</rdfs:subClassOf>
		<rdfs:subClassOf>
			<owl:Restriction>
				<owl:onProperty rdf:resource="&api4kp-ops;involvesRole"/>
				<owl:someValuesFrom>
					<owl:Class>
						<owl:intersectionOf rdf:parseType="Collection">
							<rdf:Description rdf:about="&api4kp-ops;Product">
							</rdf:Description>
							<owl:Restriction>
								<owl:onProperty rdf:resource="&api4kp-ops;isFilledBy"/>
								<owl:someValuesFrom rdf:resource="&api4kp;EncodedKnowledgeExpression"/>
							</owl:Restriction>
						</owl:intersectionOf>
					</owl:Class>
				</owl:someValuesFrom>
			</owl:Restriction>
		</rdfs:subClassOf>
		<rdfs:subClassOf>
			<owl:Restriction>
				<owl:onProperty rdf:resource="&api4kp-ops;involvesRole"/>
				<owl:someValuesFrom>
					<owl:Class>
						<owl:intersectionOf rdf:parseType="Collection">
							<rdf:Description rdf:about="&api4kp-ops;Substrate">
							</rdf:Description>
							<owl:Restriction>
								<owl:onProperty rdf:resource="&api4kp-ops;isFilledBy"/>
								<owl:someValuesFrom rdf:resource="&api4kp;KnowledgeArtifact"/>
							</owl:Restriction>
						</owl:intersectionOf>
					</owl:Class>
				</owl:someValuesFrom>
			</owl:Restriction>
		</rdfs:subClassOf>
		<rdfs:label>I/O read task</rdfs:label>
		<skos:altLabel>extraction task</skos:altLabel>
		<skos:definition>A task that extracts an encoded knowledge expression from a carrier</skos:definition>
		<skos:example>opening a file and reading the stream of Unicode-encoded characters</skos:example>
	</owl:Class>
	
	<owl:Class rdf:about="&api4kp-ops;RedactionTask">
		<rdfs:subClassOf rdf:resource="&api4kp-ops;SimplificationTask"/>
		<rdfs:label>syntactic redaction task</rdfs:label>
		<skos:definition>simplification that removes concepts by means of removing the entire fragments that evoke them</skos:definition>
	</owl:Class>
	
	<owl:Class rdf:about="&api4kp-ops;ReductionTask">
		<rdfs:subClassOf rdf:resource="&api4kp-ops;SimplificationTask"/>
		<rdfs:label>reduction task</rdfs:label>
		<skos:definition>Simplification that removes one or more classes of concepts</skos:definition>
		<skos:note>reductions can be performed in preparation of a translation or a profile projection, removing concepts that would not be expressible in the target language</skos:note>
	</owl:Class>
	
	<owl:Class rdf:about="&api4kp-ops;RemovalTask">
		<rdfs:subClassOf rdf:resource="&api4kp-ops;SeparationTask"/>
		<rdfs:label>removal task</rdfs:label>
		<skos:definition>separation based on a tree-oriented deconstruction, where the Resources that are part of a subtree of the underlying Structure are discarded.</skos:definition>
	</owl:Class>
	
	<owl:Class rdf:about="&api4kp-ops;ReplicationTask">
		<rdfs:subClassOf rdf:resource="&api4kp-ops;HorizontalKnowledgeProcessingTask"/>
		<rdfs:label>replication task</rdfs:label>
		<skos:definition>horizontal translation task that creates a new, equal, copy of the input resource.</skos:definition>
	</owl:Class>
	
	<owl:Class rdf:about="&api4kp-ops;RetrieveArtifactFromRepositoryLocationTask">
		<rdfs:subClassOf rdf:resource="&api4kp-ops;KnowledgeArtifactRepositoryTask"/>
		<rdfs:label>retrieve artifact from location task</rdfs:label>
		<skos:definition>returns (a copy of) an artifact stored at a given location</skos:definition>
	</owl:Class>
	
	<owl:Class rdf:about="&api4kp-ops;SatisfiabilityCheckTask">
		<rdfs:subClassOf rdf:resource="&api4kp-ops;LogicBasedReasoningTask"/>
		<rdfs:label>satisfiability check task</rdfs:label>
		<rdfs:seeAlso>https://en.wikipedia.org/wiki/Satisfiability</rdfs:seeAlso>
		<skos:definition>Reasoning Tasks that determines whether a knowledge base with open variables is satisfiable or not, i.e. there is at least one binding of those variables that is not inconsistent</skos:definition>
	</owl:Class>
	
	<owl:Class rdf:about="&api4kp-ops;SelectionTask">
		<rdfs:subClassOf rdf:resource="&api4kp-ops;KnowledgeReshapingTask"/>
		<rdfs:label>selection task</rdfs:label>
		<skos:definition>reshaping task that results in (the expression of) a Work of Knowledge that uses a subset of the concepts used by the original Knowledge Resource, where the subset is defined by inclusion</skos:definition>
		<skos:note>Selection is additive (to the target WoK), whereas simplification is subtractive (to the source WoK)</skos:note>
	</owl:Class>
	
	<owl:Class rdf:about="&api4kp-ops;SemanticKnowledgeManagementTask">
		<rdfs:subClassOf rdf:resource="&api4kp-ops;KnowledgeAssetRepositoryTask"/>
		<rdfs:subClassOf>
			<owl:Restriction>
				<owl:onProperty rdf:resource="&api4kp-ops;hasSubtask"/>
				<owl:someValuesFrom rdf:resource="&api4kp-ops;KnowledgeReasoningTask"/>
			</owl:Restriction>
		</rdfs:subClassOf>
		<rdfs:subClassOf>
			<owl:Restriction>
				<owl:onProperty rdf:resource="&api4kp-ops;involvesRole"/>
				<owl:someValuesFrom>
					<owl:Restriction>
						<owl:onProperty rdf:resource="&api4kp-ops;isFilledBy"/>
						<owl:someValuesFrom rdf:resource="&api4kp;KnowledgeResourceDescription"/>
					</owl:Restriction>
				</owl:someValuesFrom>
			</owl:Restriction>
		</rdfs:subClassOf>
		<rdfs:label>semantic knowledge management task</rdfs:label>
		<skos:definition>Knowledge Asset Repository Task that is a Reasoning Task applied to the Knowledge Base constituted by the Surrogates managed in the Repository</skos:definition>
	</owl:Class>
	
	<owl:Class rdf:about="&api4kp-ops;SemanticTranslationTask">
		<rdfs:subClassOf rdf:resource="&api4kp-ops;TranslationTask"/>
		<rdfs:subClassOf>
			<owl:Class>
				<owl:intersectionOf rdf:parseType="Collection">
					<owl:Restriction>
						<owl:onProperty rdf:resource="&api4kp-ops;hasSubtask"/>
						<owl:someValuesFrom rdf:resource="&api4kp-ops;ExpressionTask"/>
					</owl:Restriction>
					<owl:Restriction>
						<owl:onProperty rdf:resource="&api4kp-ops;hasSubtask"/>
						<owl:someValuesFrom rdf:resource="&api4kp-ops;InterpretationTask"/>
					</owl:Restriction>
				</owl:intersectionOf>
			</owl:Class>
		</rdfs:subClassOf>
		<rdfs:label>semantic translation task</rdfs:label>
		<skos:definition>translation task leverages the interpretation of the input expression</skos:definition>
	</owl:Class>
	
	<owl:Class rdf:about="&api4kp-ops;SeparationTask">
		<rdfs:subClassOf rdf:resource="&api4kp-ops;KnowledgeReshapingTask"/>
		<rdfs:label>separation task</rdfs:label>
		<skos:definition>reshaping task that breaks a knowledge resource into components, which are returned as individual resources</skos:definition>
		<skos:note>Conceptually equivalent to a deconstruction followed by a disassembly</skos:note>
		<skos:note>deconstructable knowledge resources are perfectly separable, i.e. the resulting resources carry, globally, the same information as the source one</skos:note>
	</owl:Class>
	
	<owl:Class rdf:about="&api4kp-ops;SerializationTask">
		<rdfs:subClassOf rdf:resource="&api4kp-ops;LoweringTask"/>
		<rdfs:subClassOf>
			<owl:Restriction>
				<owl:onProperty rdf:resource="&api4kp-ops;involvesRole"/>
				<owl:someValuesFrom>
					<owl:Class>
						<owl:intersectionOf rdf:parseType="Collection">
							<rdf:Description rdf:about="&api4kp-ops;Input">
							</rdf:Description>
							<owl:Restriction>
								<owl:onProperty rdf:resource="&api4kp-ops;isFilledBy"/>
								<owl:someValuesFrom rdf:resource="&api4kp-lang;Serialization"/>
							</owl:Restriction>
						</owl:intersectionOf>
					</owl:Class>
				</owl:someValuesFrom>
			</owl:Restriction>
		</rdfs:subClassOf>
		<rdfs:subClassOf>
			<owl:Restriction>
				<owl:onProperty rdf:resource="&api4kp-ops;involvesRole"/>
				<owl:someValuesFrom>
					<owl:Class>
						<owl:intersectionOf rdf:parseType="Collection">
							<rdf:Description rdf:about="&api4kp-ops;Input">
							</rdf:Description>
							<owl:Restriction>
								<owl:onProperty rdf:resource="&api4kp-ops;isFilledBy"/>
								<owl:someValuesFrom rdf:resource="&api4kp;AbstractKnowledgeExpression"/>
							</owl:Restriction>
						</owl:intersectionOf>
					</owl:Class>
				</owl:someValuesFrom>
			</owl:Restriction>
		</rdfs:subClassOf>
		<rdfs:subClassOf>
			<owl:Restriction>
				<owl:onProperty rdf:resource="&api4kp-ops;involvesRole"/>
				<owl:someValuesFrom>
					<owl:Class>
						<owl:intersectionOf rdf:parseType="Collection">
							<rdf:Description rdf:about="&api4kp-ops;Product">
							</rdf:Description>
							<owl:Restriction>
								<owl:onProperty rdf:resource="&api4kp-ops;isFilledBy"/>
								<owl:someValuesFrom rdf:resource="&api4kp;ConcreteKnowledgeExpression"/>
							</owl:Restriction>
						</owl:intersectionOf>
					</owl:Class>
				</owl:someValuesFrom>
			</owl:Restriction>
		</rdfs:subClassOf>
		<rdfs:label>serialization task</rdfs:label>
		<skos:definition>lowering task that serializes an abstract expression, using one of the concrete syntaxes supported by the langauge</skos:definition>
	</owl:Class>
	
	<owl:Class rdf:about="&api4kp-ops;SignatureDetectionTask">
		<rdfs:subClassOf rdf:resource="&api4kp-ops;KnowledgeAnalyticTask"/>
		<rdfs:subClassOf>
			<owl:Restriction>
				<owl:onProperty rdf:resource="&api4kp-ops;involvesRole"/>
				<owl:someValuesFrom>
					<owl:Class>
						<owl:intersectionOf rdf:parseType="Collection">
							<rdf:Description rdf:about="&api4kp-ops;Product">
							</rdf:Description>
							<owl:Restriction>
								<owl:onProperty rdf:resource="&api4kp-ops;isFilledBy"/>
								<owl:someValuesFrom rdf:resource="&api4kp-lang;Lexicon"/>
							</owl:Restriction>
						</owl:intersectionOf>
					</owl:Class>
				</owl:someValuesFrom>
			</owl:Restriction>
		</rdfs:subClassOf>
		<rdfs:label>signature detection task</rdfs:label>
		<skos:definition>Analytic task that detects the non-logical symbols (aka &quot;terms&quot; - concretizations of linguistic elements that express domain concepts) used in an expression, identifying the lexicon they have been extracted from</skos:definition>
	</owl:Class>
	
	<owl:Class rdf:about="&api4kp-ops;SimplificationTask">
		<rdfs:subClassOf rdf:resource="&api4kp-ops;KnowledgeReshapingTask"/>
		<rdfs:label>simplification task</rdfs:label>
		<skos:definition>reshaping task that results in (the expression of) a Work of Knowledge that uses a subset of the concepts used by the original Knowledge Resource, where the subset is defined by elimination</skos:definition>
	</owl:Class>
	
	<owl:Class rdf:about="&api4kp-ops;StoreArtifactAtRepositoryLocationTask">
		<rdfs:subClassOf rdf:resource="&api4kp-ops;KnowledgeArtifactRepositoryTask"/>
		<rdfs:subClassOf>
			<owl:Restriction>
				<owl:onProperty rdf:resource="&api4kp-ops;involvesRole"/>
				<owl:someValuesFrom>
					<owl:Class>
						<owl:intersectionOf rdf:parseType="Collection">
							<rdf:Description rdf:about="&api4kp-ops;Input">
							</rdf:Description>
							<owl:Restriction>
								<owl:onProperty rdf:resource="&api4kp-ops;isFilledBy"/>
								<owl:someValuesFrom rdf:resource="&api4kp;KnowledgeArtifact"/>
							</owl:Restriction>
						</owl:intersectionOf>
					</owl:Class>
				</owl:someValuesFrom>
			</owl:Restriction>
		</rdfs:subClassOf>
		<rdfs:label>store artifact at location task</rdfs:label>
		<skos:definition>ensures that an artifact is available at a given location</skos:definition>
	</owl:Class>
	
	<owl:Class rdf:about="&api4kp-ops;Substrate">
		<rdfs:subClassOf rdf:resource="&api4kp-ops;KnowledgeProcessingTaskRole"/>
		<rdfs:label>substrate</rdfs:label>
		<skos:altLabel>input/output</skos:altLabel>
		<skos:definition>role played by a resource that is used in an activity of a given type, exists before the activity is started, and is available to the agent executing the activity before the activity is started</skos:definition>
	</owl:Class>
	
	<owl:Class rdf:about="&api4kp-ops;SubsumptionTask">
		<rdfs:subClassOf rdf:resource="&api4kp-ops;LogicBasedReasoningTask"/>
		<rdfs:label>subsumption task</rdfs:label>
		<skos:note>Reasoning Task that, given two concepts (classes), determines whether one is necessarily broader than (a subclass of) the other</skos:note>
	</owl:Class>
	
	<owl:Class rdf:about="&api4kp-ops;SummarizationTask">
		<rdfs:subClassOf rdf:resource="&api4kp-ops;SimplificationTask"/>
		<rdfs:label>summarization task</rdfs:label>
		<skos:definition>simplification that removes concepts which are redundant, i.e. whose elimination produces a minimal loss of information</skos:definition>
	</owl:Class>
	
	<owl:Class rdf:about="&api4kp-ops;SyntacticAnalysisTask">
		<rdfs:subClassOf rdf:resource="&api4kp-ops;LiftingTask"/>
		<rdfs:subClassOf>
			<owl:Restriction>
				<owl:onProperty rdf:resource="&api4kp-ops;involvesRole"/>
				<owl:someValuesFrom>
					<owl:Class>
						<owl:intersectionOf rdf:parseType="Collection">
							<rdf:Description rdf:about="&api4kp-ops;Input">
							</rdf:Description>
							<owl:Restriction>
								<owl:onProperty rdf:resource="&api4kp-ops;isFilledBy"/>
								<owl:someValuesFrom rdf:resource="&api4kp-lang;ConcreteSyntaxTree"/>
							</owl:Restriction>
						</owl:intersectionOf>
					</owl:Class>
				</owl:someValuesFrom>
			</owl:Restriction>
		</rdfs:subClassOf>
		<rdfs:subClassOf>
			<owl:Restriction>
				<owl:onProperty rdf:resource="&api4kp-ops;involvesRole"/>
				<owl:someValuesFrom>
					<owl:Class>
						<owl:intersectionOf rdf:parseType="Collection">
							<rdf:Description rdf:about="&api4kp-ops;Product">
							</rdf:Description>
							<owl:Restriction>
								<owl:onProperty rdf:resource="&api4kp-ops;isFilledBy"/>
								<owl:someValuesFrom rdf:resource="&api4kp-lang;AbstractSyntaxTree"/>
							</owl:Restriction>
						</owl:intersectionOf>
					</owl:Class>
				</owl:someValuesFrom>
			</owl:Restriction>
		</rdfs:subClassOf>
		<rdfs:label>syntactic analysis task</rdfs:label>
		<skos:definition>the act of deriving an AST from a parse tree</skos:definition>
	</owl:Class>
	
	<owl:Class rdf:about="&api4kp-ops;SyntacticKnowledgeProcessingTask">
		<rdfs:subClassOf rdf:resource="&api4kp;KnowledgeProcessingTask"/>
		<rdfs:subClassOf>
			<owl:Restriction>
				<owl:onProperty rdf:resource="&api4kp-ops;involvesRole"/>
				<owl:someValuesFrom>
					<owl:Class>
						<owl:intersectionOf rdf:parseType="Collection">
							<rdf:Description rdf:about="&api4kp-ops;Input">
							</rdf:Description>
							<owl:Restriction>
								<owl:onProperty rdf:resource="&api4kp-ops;isFilledBy"/>
								<owl:someValuesFrom rdf:resource="&api4kp;KnowledgeExpression"/>
							</owl:Restriction>
						</owl:intersectionOf>
					</owl:Class>
				</owl:someValuesFrom>
			</owl:Restriction>
		</rdfs:subClassOf>
		<rdfs:label>syntactic knowledge processing task</rdfs:label>
		<skos:definition>Knowledge Processing Task that leverages the syntactic aspects of a Knowledge Expression, as determined by the grammar of the language(s) used in the Expression, without impacting the Knowledge Content of the Resource.</skos:definition>
	</owl:Class>
	
	<owl:Class rdf:about="&api4kp-ops;SyntacticParsingTask">
		<rdfs:subClassOf rdf:resource="&api4kp-ops;LiftingTask"/>
		<rdfs:subClassOf>
			<owl:Restriction>
				<owl:onProperty rdf:resource="&api4kp-ops;involvesRole"/>
				<owl:someValuesFrom>
					<owl:Class>
						<owl:intersectionOf rdf:parseType="Collection">
							<rdf:Description rdf:about="&api4kp-ops;Input">
							</rdf:Description>
							<owl:Restriction>
								<owl:onProperty rdf:resource="&api4kp-ops;isFilledBy"/>
								<owl:someValuesFrom rdf:resource="&api4kp;ConcreteKnowledgeExpression"/>
							</owl:Restriction>
						</owl:intersectionOf>
					</owl:Class>
				</owl:someValuesFrom>
			</owl:Restriction>
		</rdfs:subClassOf>
		<rdfs:subClassOf>
			<owl:Restriction>
				<owl:onProperty rdf:resource="&api4kp-ops;involvesRole"/>
				<owl:someValuesFrom>
					<owl:Class>
						<owl:intersectionOf rdf:parseType="Collection">
							<rdf:Description rdf:about="&api4kp-ops;Product">
							</rdf:Description>
							<owl:Restriction>
								<owl:onProperty rdf:resource="&api4kp-ops;isFilledBy"/>
								<owl:someValuesFrom rdf:resource="&api4kp-lang;ConcreteSyntaxTree"/>
							</owl:Restriction>
						</owl:intersectionOf>
					</owl:Class>
				</owl:someValuesFrom>
			</owl:Restriction>
		</rdfs:subClassOf>
		<rdfs:label>syntactic parsing task</rdfs:label>
		<skos:definition>the act of creating a parse tree from a concrete knowledge expression. scanning and tokenization are considered sub-atomic parts of this task</skos:definition>
	</owl:Class>
	
	<owl:Class rdf:about="&api4kp-ops;TranscreationTask">
		<rdfs:subClassOf rdf:resource="&api4kp-ops;KnowledgeResourceStructuringTask"/>
		<rdfs:subClassOf>
			<owl:Restriction>
				<owl:onProperty rdf:resource="&api4kp-ops;involvesRole"/>
				<owl:someValuesFrom>
					<owl:Class>
						<owl:intersectionOf rdf:parseType="Collection">
							<rdf:Description rdf:about="&api4kp-ops;Input">
							</rdf:Description>
							<owl:Restriction>
								<owl:onProperty rdf:resource="&api4kp-ops;isFilledBy"/>
								<owl:someValuesFrom rdf:resource="&api4kp;KnowledgeResource"/>
							</owl:Restriction>
						</owl:intersectionOf>
					</owl:Class>
				</owl:someValuesFrom>
			</owl:Restriction>
		</rdfs:subClassOf>
		<rdfs:subClassOf>
			<owl:Restriction>
				<owl:onProperty rdf:resource="&api4kp-ops;involvesRole"/>
				<owl:someValuesFrom>
					<owl:Class>
						<owl:intersectionOf rdf:parseType="Collection">
							<rdf:Description rdf:about="&api4kp-ops;Product">
							</rdf:Description>
							<owl:Restriction>
								<owl:onProperty rdf:resource="&api4kp-ops;isFilledBy"/>
								<owl:someValuesFrom>
									<owl:Class>
										<owl:intersectionOf rdf:parseType="Collection">
											<rdf:Description rdf:about="&api4kp;KnowledgeResource">
											</rdf:Description>
											<owl:Restriction>
												<owl:onProperty rdf:resource="&api4kp;isDerivedFrom"/>
												<owl:someValuesFrom rdf:resource="&api4kp;KnowledgeResource"/>
											</owl:Restriction>
										</owl:intersectionOf>
									</owl:Class>
								</owl:someValuesFrom>
							</owl:Restriction>
						</owl:intersectionOf>
					</owl:Class>
				</owl:someValuesFrom>
			</owl:Restriction>
		</rdfs:subClassOf>
		<rdfs:label>transcreation task</rdfs:label>
		<skos:definition>complex transformation that can alter the language and/or semantics of an input resource</skos:definition>
	</owl:Class>
	
	<owl:Class rdf:about="&api4kp-ops;TranscriptionTask">
		<rdfs:subClassOf rdf:resource="&api4kp-ops;HorizontalKnowledgeProcessingTask"/>
		<rdfs:subClassOf>
			<owl:Restriction>
				<owl:onProperty rdf:resource="&api4kp-ops;involvesRole"/>
				<owl:someValuesFrom>
					<owl:Class>
						<owl:intersectionOf rdf:parseType="Collection">
							<rdf:Description rdf:about="&api4kp-ops;Input">
							</rdf:Description>
							<owl:Restriction>
								<owl:onProperty rdf:resource="&api4kp-ops;isFilledBy"/>
								<owl:someValuesFrom rdf:resource="&api4kp-lang;Serialization"/>
							</owl:Restriction>
						</owl:intersectionOf>
					</owl:Class>
				</owl:someValuesFrom>
			</owl:Restriction>
		</rdfs:subClassOf>
		<rdfs:subClassOf>
			<owl:Restriction>
				<owl:onProperty rdf:resource="&api4kp-ops;involvesRole"/>
				<owl:someValuesFrom>
					<owl:Class>
						<owl:intersectionOf rdf:parseType="Collection">
							<rdf:Description rdf:about="&api4kp-ops;Input">
							</rdf:Description>
							<owl:Restriction>
								<owl:onProperty rdf:resource="&api4kp-ops;isFilledBy"/>
								<owl:someValuesFrom rdf:resource="&api4kp;KnowledgeExpression"/>
							</owl:Restriction>
						</owl:intersectionOf>
					</owl:Class>
				</owl:someValuesFrom>
			</owl:Restriction>
		</rdfs:subClassOf>
		<rdfs:subClassOf>
			<owl:Restriction>
				<owl:onProperty rdf:resource="&api4kp-ops;involvesRole"/>
				<owl:someValuesFrom>
					<owl:Class>
						<owl:intersectionOf rdf:parseType="Collection">
							<rdf:Description rdf:about="&api4kp-ops;Product">
							</rdf:Description>
							<owl:Restriction>
								<owl:onProperty rdf:resource="&api4kp-ops;isFilledBy"/>
								<owl:someValuesFrom rdf:resource="&api4kp;KnowledgeExpression"/>
							</owl:Restriction>
						</owl:intersectionOf>
					</owl:Class>
				</owl:someValuesFrom>
			</owl:Restriction>
		</rdfs:subClassOf>
		<rdfs:subClassOf>
			<owl:Restriction>
				<owl:onProperty rdf:resource="&api4kp-ops;retains"/>
				<owl:someValuesFrom rdf:resource="&lcc-lr;Language"/>
			</owl:Restriction>
		</rdfs:subClassOf>
		<rdfs:label>syntactic transcription task</rdfs:label>
		<skos:definition>horizontal translation task that maps an expression in the concrete syntax of a given language to an expression in a different concrete syntax of the same language</skos:definition>
	</owl:Class>
	
	<owl:Class rdf:about="&api4kp-ops;TranslationTask">
		<rdfs:subClassOf rdf:resource="&api4kp-ops;HorizontalKnowledgeProcessingTask"/>
		<rdfs:subClassOf>
			<owl:Restriction>
				<owl:onProperty rdf:resource="&api4kp-ops;involvesRole"/>
				<owl:someValuesFrom>
					<owl:Class>
						<owl:intersectionOf rdf:parseType="Collection">
							<rdf:Description rdf:about="&api4kp-ops;Input">
							</rdf:Description>
							<owl:Restriction>
								<owl:onProperty rdf:resource="&api4kp-ops;isFilledBy"/>
								<owl:someValuesFrom rdf:resource="&api4kp;KnowledgeExpression"/>
							</owl:Restriction>
						</owl:intersectionOf>
					</owl:Class>
				</owl:someValuesFrom>
			</owl:Restriction>
		</rdfs:subClassOf>
		<rdfs:subClassOf>
			<owl:Restriction>
				<owl:onProperty rdf:resource="&api4kp-ops;involvesRole"/>
				<owl:someValuesFrom>
					<owl:Class>
						<owl:intersectionOf rdf:parseType="Collection">
							<rdf:Description rdf:about="&api4kp-ops;Input">
							</rdf:Description>
							<owl:Restriction>
								<owl:onProperty rdf:resource="&api4kp-ops;isFilledBy"/>
								<owl:someValuesFrom rdf:resource="&lcc-lr;Language"/>
							</owl:Restriction>
						</owl:intersectionOf>
					</owl:Class>
				</owl:someValuesFrom>
			</owl:Restriction>
		</rdfs:subClassOf>
		<rdfs:subClassOf>
			<owl:Restriction>
				<owl:onProperty rdf:resource="&api4kp-ops;involvesRole"/>
				<owl:someValuesFrom>
					<owl:Class>
						<owl:intersectionOf rdf:parseType="Collection">
							<rdf:Description rdf:about="&api4kp-ops;Product">
							</rdf:Description>
							<owl:Restriction>
								<owl:onProperty rdf:resource="&api4kp-ops;isFilledBy"/>
								<owl:someValuesFrom rdf:resource="&api4kp;KnowledgeExpression"/>
							</owl:Restriction>
						</owl:intersectionOf>
					</owl:Class>
				</owl:someValuesFrom>
			</owl:Restriction>
		</rdfs:subClassOf>
		<rdfs:label>syntactic translation task</rdfs:label>
		<skos:definition>horizontal translation task that maps an expression in a given language to an expression of the same knowledge in a target language</skos:definition>
	</owl:Class>
	
	<owl:Class rdf:about="&api4kp-ops;UnionTask">
		<rdfs:subClassOf rdf:resource="&api4kp-ops;FusionTask"/>
		<rdfs:label>union task</rdfs:label>
		<skos:definition>Fusion in terms of a set-oriented implicit structure</skos:definition>
	</owl:Class>
	
	<owl:Class rdf:about="&api4kp-ops;VerticalKnowledgeProcessingTask">
		<rdfs:subClassOf rdf:resource="&api4kp-ops;SyntacticKnowledgeProcessingTask"/>
		<rdfs:subClassOf>
			<owl:Restriction>
				<owl:onProperty rdf:resource="&api4kp-ops;involvesRole"/>
				<owl:someValuesFrom>
					<owl:Class>
						<owl:intersectionOf rdf:parseType="Collection">
							<rdf:Description rdf:about="&api4kp-ops;Input">
							</rdf:Description>
							<owl:Restriction>
								<owl:onProperty rdf:resource="&api4kp-ops;isFilledBy"/>
								<owl:someValuesFrom rdf:resource="&api4kp;KnowledgeResource"/>
							</owl:Restriction>
						</owl:intersectionOf>
					</owl:Class>
				</owl:someValuesFrom>
			</owl:Restriction>
		</rdfs:subClassOf>
		<rdfs:subClassOf>
			<owl:Restriction>
				<owl:onProperty rdf:resource="&api4kp-ops;involvesRole"/>
				<owl:someValuesFrom>
					<owl:Class>
						<owl:intersectionOf rdf:parseType="Collection">
							<rdf:Description rdf:about="&api4kp-ops;Product">
							</rdf:Description>
							<owl:Restriction>
								<owl:onProperty rdf:resource="&api4kp-ops;isFilledBy"/>
								<owl:someValuesFrom rdf:resource="&api4kp;KnowledgeResource"/>
							</owl:Restriction>
						</owl:intersectionOf>
					</owl:Class>
				</owl:someValuesFrom>
			</owl:Restriction>
		</rdfs:subClassOf>
		<rdfs:subClassOf>
			<owl:Restriction>
				<owl:onProperty rdf:resource="&api4kp-ops;retains"/>
				<owl:someValuesFrom rdf:resource="&api4kp;WorkOfKnowledge"/>
			</owl:Restriction>
		</rdfs:subClassOf>
		<rdfs:label>vertical knowledge processing task</rdfs:label>
		<skos:definition>syntactic knowledge processing task that produces Knowledge Resources at higher or lower level of abstraction along the &quot;artifact - asset&quot; chain</skos:definition>
	</owl:Class>
	
	<owl:Class rdf:about="&api4kp-ops;WeavingTask">
		<rdfs:subClassOf rdf:resource="&api4kp-ops;KnowledgeReshapingTask"/>
		<rdfs:label>weaving task</rdfs:label>
		<skos:definition>a reshaping such that fragments of one or more expressions are embedded in a target expression</skos:definition>
	</owl:Class>
	
	<owl:Class rdf:about="&api4kp-ops;WellFormednessCheckTask">
		<rdfs:subClassOf rdf:resource="&api4kp-ops;KnowledgeAnalyticTask"/>
		<rdfs:subClassOf>
			<owl:Restriction>
				<owl:onProperty rdf:resource="&api4kp-ops;involvesRole"/>
				<owl:someValuesFrom>
					<owl:Class>
						<owl:intersectionOf rdf:parseType="Collection">
							<rdf:Description rdf:about="&api4kp-ops;Input">
							</rdf:Description>
							<owl:Restriction>
								<owl:onProperty rdf:resource="&api4kp-ops;isFilledBy"/>
								<owl:someValuesFrom rdf:resource="&lcc-lr;Language"/>
							</owl:Restriction>
						</owl:intersectionOf>
					</owl:Class>
				</owl:someValuesFrom>
			</owl:Restriction>
		</rdfs:subClassOf>
		<rdfs:label>well-formedness check task</rdfs:label>
		<skos:definition>Analytic task that detects whether a Knowledge Expression is a valid sentence according to the syntax - abstract and/or concrete - of some language, or profile thereof.</skos:definition>
	</owl:Class>
	
	<owl:Class rdf:about="&api4kp-ops;WorkingKnowledgeBaseCreationTask">
		<rdfs:subClassOf rdf:resource="&api4kp-ops;KnowledgeResourceAssemblyTask"/>
		<rdfs:subClassOf>
			<owl:Restriction>
				<owl:onProperty rdf:resource="&api4kp-ops;involvesRole"/>
				<owl:someValuesFrom>
					<owl:Class>
						<owl:intersectionOf rdf:parseType="Collection">
							<rdf:Description rdf:about="&api4kp-ops;Product">
							</rdf:Description>
							<owl:Restriction>
								<owl:onProperty rdf:resource="&api4kp-ops;isFilledBy"/>
								<owl:someValuesFrom rdf:resource="&api4kp-krr;KnowledgeBase"/>
							</owl:Restriction>
						</owl:intersectionOf>
					</owl:Class>
				</owl:someValuesFrom>
			</owl:Restriction>
		</rdfs:subClassOf>
		<rdfs:label>create working knowledge base task</rdfs:label>
		<skos:definition>assembly task that initializes a working knowledge base, possibly using a knowledge resource as initial content</skos:definition>
	</owl:Class>
	
	<owl:Class rdf:about="&api4kp-ops;WriteTask">
		<rdfs:subClassOf rdf:resource="&api4kp-ops;LoweringTask"/>
		<rdfs:subClassOf>
			<owl:Restriction>
				<owl:onProperty rdf:resource="&api4kp-ops;involvesRole"/>
				<owl:someValuesFrom>
					<owl:Class>
						<owl:intersectionOf rdf:parseType="Collection">
							<rdf:Description rdf:about="&api4kp-ops;Input">
							</rdf:Description>
							<owl:Restriction>
								<owl:onProperty rdf:resource="&api4kp-ops;isFilledBy"/>
								<owl:someValuesFrom rdf:resource="&api4kp;EncodedKnowledgeExpression"/>
							</owl:Restriction>
						</owl:intersectionOf>
					</owl:Class>
				</owl:someValuesFrom>
			</owl:Restriction>
		</rdfs:subClassOf>
		<rdfs:subClassOf>
			<owl:Restriction>
				<owl:onProperty rdf:resource="&api4kp-ops;involvesRole"/>
				<owl:someValuesFrom>
					<owl:Class>
						<owl:intersectionOf rdf:parseType="Collection">
							<rdf:Description rdf:about="&api4kp-ops;Product">
							</rdf:Description>
							<owl:Restriction>
								<owl:onProperty rdf:resource="&api4kp-ops;isFilledBy"/>
								<owl:someValuesFrom rdf:resource="&api4kp;ExternalizedKnowledgeExpression"/>
							</owl:Restriction>
						</owl:intersectionOf>
					</owl:Class>
				</owl:someValuesFrom>
			</owl:Restriction>
		</rdfs:subClassOf>
		<rdfs:subClassOf>
			<owl:Restriction>
				<owl:onProperty rdf:resource="&api4kp-ops;involvesRole"/>
				<owl:someValuesFrom>
					<owl:Class>
						<owl:intersectionOf rdf:parseType="Collection">
							<rdf:Description rdf:about="&api4kp-ops;Substrate">
							</rdf:Description>
							<owl:Restriction>
								<owl:onProperty rdf:resource="&api4kp-ops;isFilledBy"/>
								<owl:someValuesFrom rdf:resource="&api4kp;KnowledgeArtifact"/>
							</owl:Restriction>
						</owl:intersectionOf>
					</owl:Class>
				</owl:someValuesFrom>
			</owl:Restriction>
		</rdfs:subClassOf>
		<rdfs:label>I/O write task</rdfs:label>
		<skos:altLabel>engraving task</skos:altLabel>
		<skos:definition>lowering task that imprints an encoded expression on a carrier artifact</skos:definition>
		<skos:example>writing a stream of ASCII characters to a (text) file</skos:example>
	</owl:Class>
	
	<owl:ObjectProperty rdf:about="&api4kp-ops;hasSubtask">
		<rdfs:subPropertyOf rdf:resource="&api4kp;hasProperPart"/>
		<rdfs:label>has subTask</rdfs:label>
		<rdfs:domain rdf:resource="&api4kp;KnowledgeProcessingTask"/>
		<rdfs:range rdf:resource="&api4kp;KnowledgeProcessingTask"/>
		<skos:definition>the relationship between a task T and a task S, such that an activity of kind T will have an activity of type S as a sub-activity, i.e. as a (temporal) proper process part</skos:definition>
	</owl:ObjectProperty>
	
	<owl:ObjectProperty rdf:about="&api4kp-ops;involvesRole">
		<rdfs:subPropertyOf rdf:resource="&api4kp;hasProperPart"/>
		<rdfs:label>has role</rdfs:label>
		<rdfs:domain rdf:resource="&api4kp;KnowledgeProcessingTask"/>
		<rdfs:range rdf:resource="&api4kp-ops;KnowledgeProcessingTaskRole"/>
		<skos:definition>has a definition, part of which is the given role</skos:definition>
		<skos:note>tasks (activity definitions) involve roles, and roles are filled by entities that participate in the activities of the given type</skos:note>
	</owl:ObjectProperty>
	
	<owl:ObjectProperty rdf:about="&api4kp-ops;isCopyOf">
		<rdfs:label>is copy of</rdfs:label>
		<skos:definition>distinct individual that, at creation time, replicates all the qualities/characteristics of</skos:definition>
	</owl:ObjectProperty>
	
	<owl:ObjectProperty rdf:about="&api4kp-ops;isFilledBy">
		<rdfs:subPropertyOf rdf:resource="&api4kp;archetypes"/>
		<rdfs:label>is filled by</rdfs:label>
		<rdfs:domain rdf:resource="&api4kp-ops;KnowledgeProcessingTaskRole"/>
		<skos:definition>abstracts the characteristics of, with respect to the participation in a knowledge processing activity of a given type</skos:definition>
	</owl:ObjectProperty>
	
	<owl:ObjectProperty rdf:about="&api4kp-ops;retains">
		<rdfs:label>retains</rdfs:label>
		<rdfs:domain rdf:resource="&api4kp;KnowledgeProcessingTask"/>
		<skos:definition>does not impact an (invariant) characteristic shared by its inputs and outputs</skos:definition>
	</owl:ObjectProperty>
	
	<owl:Class rdf:about="&api4kp;KnowledgeProcessingTask">
		<rdfs:subClassOf rdf:resource="&api4kp;DefinedConcept"/>
		<rdfs:subClassOf>
			<owl:Restriction>
				<owl:onProperty rdf:resource="&api4kp-ops;involvesRole"/>
				<owl:someValuesFrom>
					<owl:Class>
						<owl:intersectionOf rdf:parseType="Collection">
							<rdf:Description rdf:about="&api4kp-ops;KnowledgeProcessingTaskRole">
							</rdf:Description>
							<owl:Restriction>
								<owl:onProperty rdf:resource="&api4kp-ops;isFilledBy"/>
								<owl:someValuesFrom rdf:resource="&api4kp;KnowledgeResource"/>
							</owl:Restriction>
						</owl:intersectionOf>
					</owl:Class>
				</owl:someValuesFrom>
			</owl:Restriction>
		</rdfs:subClassOf>
		<rdfs:subClassOf>
			<owl:Restriction>
				<owl:onProperty rdf:resource="&api4kp;archetypes"/>
				<owl:someValuesFrom rdf:resource="&api4kp-ops;KnowledgeProcessingActivity"/>
			</owl:Restriction>
		</rdfs:subClassOf>
		<rdfs:label>knowledge processing task</rdfs:label>
		<skos:definition>archetypical abstraction of a class of knowledge processing activities that are executed according to a common method, and involve resources of the same nature</skos:definition>
		<skos:editorialNote>The notion of &apos;task&apos;, &apos;activity&apos;, and &apos;method&apos; is informed by the DOLCE DnS ontology</skos:editorialNote>
		<skos:note>A Knowledge Processing Task abstracts, defining it, the role that different types of Knowledge Resources play in a Knowledge Processing Activity</skos:note>
		<skos:note>A Knowledge Processing Task includes a Goal, i.e. a formal description of the expected situation that is the outcome of the execution of an Activity of the type defined by the Task.
When the outcome matches the Goal - i.e. the description of the outcome is subsumed by the Goal - the activity is considered to be successful. Otherwise, it is considered to be failed.</skos:note>
		<skos:note>Knowledge Processing Tasks are associated to Constructive Definitions that are (Knowledge Processing) Methods which specify how to execute the Task.</skos:note>
		<skos:note>Knowledge Processing Tasks executed according to a method that has some degrees of freedom, can be configured using Parameters</skos:note>
		<skos:note>The execution of a Knowledge Processing Task may involve the generation of an &apos;explanation&apos;</skos:note>
	</owl:Class>

</rdf:RDF>