<?xml version="1.0" encoding="UTF-8"?>
<!DOCTYPE rdf:RDF [
	<!ENTITY api4kp "https://www.omg.org/spec/API4KP/api4kp/">
	<!ENTITY api4kp-series "https://www.omg.org/spec/API4KP/api4kp-series/">
	<!ENTITY dct "http://purl.org/dc/terms/">
	<!ENTITY dol "http://www.omg.org/spec/DOL/DOL-terms/">
	<!ENTITY lcc-lr "https://www.omg.org/spec/LCC/Languages/LanguageRepresentation/">
	<!ENTITY owl "http://www.w3.org/2002/07/owl#">
	<!ENTITY rdf "http://www.w3.org/1999/02/22-rdf-syntax-ns#">
	<!ENTITY rdfs "http://www.w3.org/2000/01/rdf-schema#">
	<!ENTITY skos "http://www.w3.org/2004/02/skos/core#">
	<!ENTITY sm "http://www.omg.org/techprocess/ab/SpecificationMetadata/">
	<!ENTITY xsd "http://www.w3.org/2001/XMLSchema#">
]>
<rdf:RDF xml:base="https://www.omg.org/spec/API4KP/api4kp-series/"
	xmlns:api4kp="https://www.omg.org/spec/API4KP/api4kp/"
	xmlns:api4kp-series="https://www.omg.org/spec/API4KP/api4kp-series/"
	xmlns:dct="http://purl.org/dc/terms/"
	xmlns:dol="http://www.omg.org/spec/DOL/DOL-terms/"
	xmlns:lcc-lr="https://www.omg.org/spec/LCC/Languages/LanguageRepresentation/"
	xmlns:owl="http://www.w3.org/2002/07/owl#"
	xmlns:rdf="http://www.w3.org/1999/02/22-rdf-syntax-ns#"
	xmlns:rdfs="http://www.w3.org/2000/01/rdf-schema#"
	xmlns:skos="http://www.w3.org/2004/02/skos/core#"
	xmlns:sm="http://www.omg.org/techprocess/ab/SpecificationMetadata/"
	xmlns:xsd="http://www.w3.org/2001/XMLSchema#">
	
	<owl:Ontology rdf:about="https://www.omg.org/spec/API4KP/api4kp-series/">
		<rdfs:label>API4KP Ontology of Series</rdfs:label>
		<dct:abstract>This ontology extends the core API4KP ontology to incorporate notions of     20210401s and versions of knowledge artifacts as they change over time.</dct:abstract>
		<dct:contributor>Elisa Kendall (ekendall at thematix.com)</dct:contributor>
		<dct:creator>Davide Sottara (sottara.davide at mayo.edu)</dct:creator>
		<dct:license rdf:datatype="&xsd;anyURI">http://opensource.org/licenses/MIT</dct:license>
		<sm:contentLanguage rdf:datatype="&xsd;anyURI">https://www.w3.org/TR/owl2-quick-reference/</sm:contentLanguage>
		<sm:copyright>Copyright (c) 2014-2021 Athan Services</sm:copyright>
		<sm:copyright>Copyright (c) 2014-2021 Fraunhofer Gesellschaft</sm:copyright>
		<sm:copyright>Copyright (c) 2014-2021 Freie Universität Berlin</sm:copyright>
		<sm:copyright>Copyright (c) 2014-2021 Mayo Foundation for Medical Education and Research (MFMER)</sm:copyright>
		<sm:copyright>Copyright (c) 2014-2021 Thematix Partners LLC</sm:copyright>
		<sm:copyright>Copyright (c) 2015-2021 Object Management Group, Inc.</sm:copyright>
		<sm:copyright>Copyright (c) 2019-2021 Universität Leipzig</sm:copyright>
		<sm:copyright>Copyright (c) 2020-2021 Micro Focus</sm:copyright>
		<sm:dependsOn rdf:datatype="&xsd;anyURI">https://www.omg.org/spec/API4KP/api4kp/</sm:dependsOn>
		<sm:dependsOn rdf:datatype="&xsd;anyURI">https://www.omg.org/spec/DOL/</sm:dependsOn>
		<sm:dependsOn rdf:datatype="&xsd;anyURI">https://www.omg.org/spec/LCC/</sm:dependsOn>
		<sm:fileAbbreviation>api4kp-series</sm:fileAbbreviation>
		<sm:filename>api4kp-series.rdf</sm:filename>
		<owl:imports rdf:resource="http://www.omg.org/techprocess/ab/SpecificationMetadata/"/>
		<owl:imports rdf:resource="https://www.omg.org/spec/API4KP/api4kp/"/>
		<owl:imports rdf:resource="https://www.omg.org/spec/DOL/DOL-terms/"/>
		<owl:imports rdf:resource="https://www.omg.org/spec/LCC/Languages/LanguageRepresentation/"/>
		<owl:versionIRI rdf:resource="https://www.omg.org/spec/API4KP/20210401/api4kp-series/"/>
	</owl:Ontology>
	
	<rdfs:Datatype rdf:about="&api4kp-series;CombinedDateTime">
		<rdfs:label>combined date time</rdfs:label>
		<owl:equivalentClass>
			<rdfs:Datatype>
				<owl:unionOf rdf:parseType="Collection">
					<rdf:Description rdf:about="&xsd;string">
					</rdf:Description>
					<rdf:Description rdf:about="&xsd;dateTime">
					</rdf:Description>
					<rdf:Description rdf:about="&xsd;dateTimeStamp">
					</rdf:Description>
				</owl:unionOf>
			</rdfs:Datatype>
		</owl:equivalentClass>
		<skos:definition>datatype that maps to several base types for dates and times</skos:definition>
		<skos:note>Valid values must use the ISO 8601 representation for a date, or the corresponding XML Schema Datatypes representation for a date and time, or date and time including the time zone.</skos:note>
		<skos:scopeNote>There are many cases where the representation of a date may or may not include a time, and where the underlying data representation varies.  This composite datatype should only be used in cases where a standard representation using one of the options in the union for date or date and time value specification does not work, for example, when resolution beyond microseconds is needed.</skos:scopeNote>
	</rdfs:Datatype>
	
	<owl:Class rdf:about="&api4kp-series;ImmutableEntity">
		<rdfs:label>immutable</rdfs:label>
		<owl:disjointWith rdf:resource="&api4kp-series;MutableEntity"/>
		<skos:definition>entity whose state does not, or cannot, change over time without preserving the identity of the entity</skos:definition>
	</owl:Class>
	
	<owl:Class rdf:about="&api4kp-series;MutableEntity">
		<rdfs:label>mutable</rdfs:label>
		<skos:definition>continuant entity whose state, determined by the configuration of its qualia, changes over time while maintaining a principle of identity</skos:definition>
	</owl:Class>
	
	<owl:Class rdf:about="&api4kp-series;Series">
		<rdfs:subClassOf rdf:resource="&api4kp-series;MutableEntity"/>
		<rdfs:subClassOf rdf:resource="&lcc-lr;Collection"/>
		<rdfs:subClassOf>
			<owl:Restriction>
				<owl:onProperty rdf:resource="&dol;hasPart"/>
				<owl:someValuesFrom rdf:resource="&lcc-lr;IdentificationScheme"/>
			</owl:Restriction>
		</rdfs:subClassOf>
		<rdfs:subClassOf>
			<owl:Restriction>
				<owl:onProperty rdf:resource="&api4kp-series;isSeriesOf"/>
				<owl:someValuesFrom rdf:resource="&api4kp-series;MutableEntity"/>
			</owl:Restriction>
		</rdfs:subClassOf>
		<rdfs:subClassOf>
			<owl:Restriction>
				<owl:onProperty rdf:resource="&lcc-lr;hasMember"/>
				<owl:someValuesFrom rdf:resource="&api4kp-series;Version"/>
			</owl:Restriction>
		</rdfs:subClassOf>
		<rdfs:label>series</rdfs:label>
		<skos:definition>set of all versions of the same entity</skos:definition>
		<skos:note>The set is implicitly equipped with a total order determined by the points in time at which the     20210401s were taken, as well as an identification scheme that supports version identifiers.</skos:note>
	</owl:Class>
	
	<owl:Class rdf:about="&api4kp-series;    20210401">
		<rdfs:subClassOf rdf:resource="&api4kp-series;ImmutableEntity"/>
		<rdfs:label>    20210401</rdfs:label>
		<rdfs:seeAlso>https://en.wikipedia.org/wiki/20210401_(computer_storage)</rdfs:seeAlso>
		<skos:definition>immutable entity that reflects and maintains the state of a mutable entity at a particular point in time</skos:definition>
	</owl:Class>
	
	<owl:Class rdf:about="&api4kp-series;Version">
		<rdfs:subClassOf rdf:resource="&api4kp-series;    20210401"/>
		<rdfs:label>version</rdfs:label>
		<owl:equivalentClass>
			<owl:Class>
				<owl:intersectionOf rdf:parseType="Collection">
					<rdf:Description rdf:about="&api4kp-series;    20210401">
					</rdf:Description>
					<owl:Restriction>
						<owl:onProperty rdf:resource="&lcc-lr;isIdentifiedBy"/>
						<owl:someValuesFrom rdf:resource="&lcc-lr;Identifier"/>
					</owl:Restriction>
					<owl:Restriction>
						<owl:onProperty rdf:resource="&api4kp-series;hasObservedDateTime"/>
						<owl:someValuesFrom rdf:resource="&api4kp-series;CombinedDateTime"/>
					</owl:Restriction>
				</owl:intersectionOf>
			</owl:Class>
		</owl:equivalentClass>
		<skos:definition>    20210401 was observed at some point in time and that is assigned an identifier in some context</skos:definition>
	</owl:Class>
	
	<owl:Class rdf:about="&api4kp-series;VersionIdentifier">
		<rdfs:subClassOf rdf:resource="&lcc-lr;Identifier"/>
		<rdfs:subClassOf>
			<owl:Restriction>
				<owl:onProperty rdf:resource="&dol;hasPart"/>
				<owl:someValuesFrom>
					<owl:Restriction>
						<owl:onProperty rdf:resource="&lcc-lr;identifies"/>
						<owl:someValuesFrom rdf:resource="&api4kp-series;MutableEntity"/>
					</owl:Restriction>
				</owl:someValuesFrom>
			</owl:Restriction>
		</rdfs:subClassOf>
		<rdfs:subClassOf>
			<owl:Restriction>
				<owl:onProperty rdf:resource="&lcc-lr;identifies"/>
				<owl:someValuesFrom rdf:resource="&api4kp-series;Version"/>
			</owl:Restriction>
		</rdfs:subClassOf>
		<rdfs:label>version identifier</rdfs:label>
		<skos:altLabel>version-aware identifier</skos:altLabel>
		<skos:definition>identifier of a particular version of an entity, and has a part that identifies the entity (series) itself</skos:definition>
		<skos:example>the IRI / versionIRI pair used to identify versions of an OWL ontology</skos:example>
	</owl:Class>
	
	<owl:ObjectProperty rdf:about="&api4kp-series;hasLatest">
		<rdfs:subPropertyOf rdf:resource="&lcc-lr;hasMember"/>
		<rdfs:label>has latest</rdfs:label>
		<rdfs:domain rdf:resource="&api4kp-series;Series"/>
		<rdfs:range rdf:resource="&api4kp-series;Version"/>
		<skos:definition>has member version that is the successor of every other member of the series, and does not have any successor itself</skos:definition>
		<skos:note>this property is mutable as the series mutates over time</skos:note>
	</owl:ObjectProperty>
	
	<owl:ObjectProperty rdf:about="&api4kp-series;hasNextVersion">
		<rdfs:subPropertyOf rdf:resource="&api4kp-series;hasSuccesorVersion"/>
		<rdfs:label>has next version</rdfs:label>
		<owl:inverseOf rdf:resource="&api4kp-series;hasPreviousVersion"/>
		<skos:altLabel>has next immediate version</skos:altLabel>
		<skos:definition>is a version V1 that has successor version V2, and there is no other distinct version that is successor of V1 and predecessor of V2</skos:definition>
	</owl:ObjectProperty>
	
	<owl:DatatypeProperty rdf:about="&api4kp-series;hasObservedDateTime">
		<rdf:type rdf:resource="&owl;FunctionalProperty"/>
		<rdfs:label>has observed date and time</rdfs:label>
		<rdfs:range rdf:resource="&api4kp-series;CombinedDateTime"/>
		<skos:definition>indicates a date and time for an event, measurement,     20210401 or other observation</skos:definition>
	</owl:DatatypeProperty>
	
	<owl:ObjectProperty rdf:about="&api4kp-series;hasOriginal">
		<rdfs:subPropertyOf rdf:resource="&lcc-lr;hasMember"/>
		<rdfs:label>has original</rdfs:label>
		<rdfs:domain rdf:resource="&api4kp-series;Series"/>
		<rdfs:range rdf:resource="&api4kp-series;Version"/>
		<skos:definition>has member version that is the predecessor of every other member of the series, and it is not possible for it to have any predecessor itself</skos:definition>
	</owl:ObjectProperty>
	
	<owl:ObjectProperty rdf:about="&api4kp-series;hasPredecessorVersion">
		<rdfs:subPropertyOf rdf:resource="&api4kp-series;isInSeriesWith"/>
		<rdfs:label>has predecessor version</rdfs:label>
		<rdfs:domain rdf:resource="&api4kp-series;Version"/>
		<rdfs:range rdf:resource="&api4kp-series;Version"/>
		<owl:inverseOf rdf:resource="&api4kp-series;hasSuccesorVersion"/>
		<skos:altLabel>has prior version</skos:altLabel>
		<skos:definition>is in the same series with a version whose timestamp is before the timestamp of this version</skos:definition>
	</owl:ObjectProperty>
	
	<owl:ObjectProperty rdf:about="&api4kp-series;hasPreviousVersion">
		<rdfs:subPropertyOf rdf:resource="&api4kp-series;hasPredecessorVersion"/>
		<rdfs:label>has previous version</rdfs:label>
		<skos:altLabel>has previous immediate version</skos:altLabel>
		<skos:definition>is a version V1 that has predecessor version V2, and there is no other distinct version that is predecessor of V1 and successor of V2</skos:definition>
	</owl:ObjectProperty>
	
	<owl:ObjectProperty rdf:about="&api4kp-series;has    20210401">
		<rdfs:label>has     20210401</rdfs:label>
		<rdfs:domain rdf:resource="&api4kp-series;MutableEntity"/>
		<rdfs:range rdf:resource="&api4kp-series;    20210401"/>
		<owl:inverseOf rdf:resource="&api4kp-series;is    20210401Of"/>
		<skos:definition>had a state at some point in time that is reflected by the target immutable entity</skos:definition>
	</owl:ObjectProperty>
	
	<owl:ObjectProperty rdf:about="&api4kp-series;hasSuccesorVersion">
		<rdfs:subPropertyOf rdf:resource="&api4kp-series;isInSeriesWith"/>
		<rdfs:label>has successor version</rdfs:label>
		<skos:definition>is in the same series with a version whose timestamp is after the timestamp of this version</skos:definition>
	</owl:ObjectProperty>
	
	<owl:ObjectProperty rdf:about="&api4kp-series;hasVersion">
		<rdfs:subPropertyOf rdf:resource="&api4kp-series;has    20210401"/>
		<rdfs:label>has version</rdfs:label>
		<rdfs:domain rdf:resource="&api4kp-series;MutableEntity"/>
		<rdfs:range rdf:resource="&api4kp-series;Version"/>
		<owl:inverseOf rdf:resource="&api4kp-series;isVersionOf"/>
		<skos:definition>has a     20210401 that is explicitly identified</skos:definition>
	</owl:ObjectProperty>
	
	<owl:ObjectProperty rdf:about="&api4kp-series;isInSeriesWith">
		<rdf:type rdf:resource="&owl;SymmetricProperty"/>
		<rdfs:label>is in series with</rdfs:label>
		<rdfs:domain rdf:resource="&api4kp-series;    20210401"/>
		<rdfs:range rdf:resource="&api4kp-series;    20210401"/>
		<skos:definition>is a different     20210401 of the same entity</skos:definition>
	</owl:ObjectProperty>
	
	<owl:ObjectProperty rdf:about="&api4kp-series;isSeriesOf">
		<rdfs:label>is series of</rdfs:label>
		<rdfs:domain rdf:resource="&api4kp-series;Series"/>
		<rdfs:range rdf:resource="&api4kp-series;MutableEntity"/>
		<skos:definition>is the set of all versions of the same mutable entity</skos:definition>
	</owl:ObjectProperty>
	
	<owl:ObjectProperty rdf:about="&api4kp-series;is    20210401Of">
		<rdfs:label>is     20210401 of</rdfs:label>
		<rdfs:domain rdf:resource="&api4kp-series;    20210401"/>
		<rdfs:range rdf:resource="&api4kp-series;MutableEntity"/>
		<skos:definition>reflects the state of, at a particular point in time</skos:definition>
	</owl:ObjectProperty>
	
	<owl:ObjectProperty rdf:about="&api4kp-series;isVersionOf">
		<rdfs:subPropertyOf rdf:resource="&api4kp-series;is    20210401Of"/>
		<rdfs:label>is version of</rdfs:label>
		<rdfs:domain rdf:resource="&api4kp-series;Version"/>
		<rdfs:range rdf:resource="&api4kp-series;MutableEntity"/>
		<skos:definition>is an explicitly identified     20210401 of the target entity</skos:definition>
	</owl:ObjectProperty>
	
	<owl:Class rdf:about="&api4kp;KnowledgeResource">
		<rdfs:subClassOf rdf:resource="&api4kp-series;Version"/>
	</owl:Class>
	
	<owl:Class rdf:about="&lcc-lr;CodeElement">
		<rdfs:subClassOf rdf:resource="&api4kp-series;ImmutableEntity"/>
	</owl:Class>
	
	<owl:Class rdf:about="&lcc-lr;Identifier">
		<rdfs:subClassOf rdf:resource="&api4kp-series;ImmutableEntity"/>
	</owl:Class>
	
	<owl:Class rdf:about="&lcc-lr;Language">
		<rdfs:subClassOf>
			<owl:Class>
				<owl:intersectionOf rdf:parseType="Collection">
					<rdf:Description rdf:about="&api4kp-series;MutableEntity">
					</rdf:Description>
					<rdf:Description rdf:about="&api4kp;Knowledge">
					</rdf:Description>
				</owl:intersectionOf>
			</owl:Class>
		</rdfs:subClassOf>
	</owl:Class>

</rdf:RDF>