<?xml version="1.0" encoding="UTF-8"?>
<!DOCTYPE rdf:RDF [
	<!ENTITY api4kp "https://www.omg.org/spec/API4KP/api4kp/">
	<!ENTITY api4kp-ckao "https://www.omg.org/spec/API4KP/api4kp-ckao/">
	<!ENTITY api4kp-kao "https://www.omg.org/spec/API4KP/api4kp-kao/">
	<!ENTITY api4kp-lang "https://www.omg.org/spec/API4KP/api4kp-lang/">
	<!ENTITY dct "http://purl.org/dc/terms/">
	<!ENTITY owl "http://www.w3.org/2002/07/owl#">
	<!ENTITY rdf "http://www.w3.org/1999/02/22-rdf-syntax-ns#">
	<!ENTITY rdfs "http://www.w3.org/2000/01/rdf-schema#">
	<!ENTITY skos "http://www.w3.org/2004/02/skos/core#">
	<!ENTITY sm "http://www.omg.org/techprocess/ab/SpecificationMetadata/">
	<!ENTITY xsd "http://www.w3.org/2001/XMLSchema#">
]>
<rdf:RDF xml:base="https://www.omg.org/spec/API4KP/api4kp-ckao/"
	xmlns:api4kp="https://www.omg.org/spec/API4KP/api4kp/"
	xmlns:api4kp-ckao="https://www.omg.org/spec/API4KP/api4kp-ckao/"
	xmlns:api4kp-kao="https://www.omg.org/spec/API4KP/api4kp-kao/"
	xmlns:api4kp-lang="https://www.omg.org/spec/API4KP/api4kp-lang/"
	xmlns:dct="http://purl.org/dc/terms/"
	xmlns:owl="http://www.w3.org/2002/07/owl#"
	xmlns:rdf="http://www.w3.org/1999/02/22-rdf-syntax-ns#"
	xmlns:rdfs="http://www.w3.org/2000/01/rdf-schema#"
	xmlns:skos="http://www.w3.org/2004/02/skos/core#"
	xmlns:sm="http://www.omg.org/techprocess/ab/SpecificationMetadata/"
	xmlns:xsd="http://www.w3.org/2001/XMLSchema#">
	
	<owl:Ontology rdf:about="https://www.omg.org/spec/API4KP/api4kp-ckao/">
		<rdfs:label>API4KP Clinical Knowledge Assets Ontology</rdfs:label>
		<dct:abstract>TODO</dct:abstract>
		<dct:contributor>Elisa Kendall (ekendall at thematix.com)</dct:contributor>
		<dct:creator>Davide Sottara (sottara.davide at mayo.edu)</dct:creator>
		<dct:license rdf:datatype="&xsd;anyURI">http://opensource.org/licenses/MIT</dct:license>
		<sm:contentLanguage rdf:datatype="&xsd;anyURI">https://www.w3.org/TR/owl2-quick-reference/</sm:contentLanguage>
		<sm:copyright>Copyright (c) 2014-2021 Athan Services</sm:copyright>
		<sm:copyright>Copyright (c) 2014-2021 Fraunhofer Gesellschaft</sm:copyright>
		<sm:copyright>Copyright (c) 2014-2021 Freie Universität Berlin</sm:copyright>
		<sm:copyright>Copyright (c) 2014-2021 Mayo Foundation for Medical Education and Research (MFMER)</sm:copyright>
		<sm:copyright>Copyright (c) 2014-2021 Thematix Partners LLC</sm:copyright>
		<sm:copyright>Copyright (c) 2015-2021 Object Management Group, Inc.</sm:copyright>
		<sm:copyright>Copyright (c) 2019-2021 Universität Leipzig</sm:copyright>
		<sm:copyright>Copyright (c) 2020-2021 Micro Focus</sm:copyright>
		<sm:dependsOn rdf:datatype="&xsd;anyURI">https://www.omg.org/spec/API4KP/api4kp-kao/</sm:dependsOn>
		<sm:dependsOn rdf:datatype="&xsd;anyURI">https://www.omg.org/spec/API4KP/api4kp/</sm:dependsOn>
		<sm:fileAbbreviation>api4kp-ckao</sm:fileAbbreviation>
		<sm:filename>api4kp-ckao.rdf</sm:filename>
		<owl:imports rdf:resource="http://www.omg.org/spec/DOL/DOL-terms/"/>
		<owl:imports rdf:resource="http://www.omg.org/techprocess/ab/SpecificationMetadata/"/>
		<owl:imports rdf:resource="https://www.omg.org/spec/API4KP/api4kp-kao/"/>
		<owl:versionIRI rdf:resource="https://www.omg.org/spec/API4KP/20210401/api4kp-ckao/"/>
	</owl:Ontology>

	<owl:Class rdf:about="&api4kp-kao;DomainSpecificKnowledgeAsset">
		<rdfs:subClassOf rdf:resource="&api4kp;KnowledgeAsset"/>
		<rdfs:label>domain-specific knowledge asset</rdfs:label>
	</owl:Class>

	<owl:Class rdf:about="&api4kp-ckao;ClinicalKnowledgeAsset">
		<rdfs:subClassOf rdf:resource="&api4kp-ckao;DomainSpecificKnowledgeAsset"/>
		<rdfs:label>clinical knowledge asset</rdfs:label>
		<skos:definition>domain-specific knowledge asset that uses primarily concepts from the clinical business domain</skos:definition>
	</owl:Class>

  <owl:Class rdf:about="&api4kp-kao;CategorizedKnowledgeAsset">
    <rdfs:subClassOf rdf:resource="&api4kp;KnowledgeAsset"/>
    <rdfs:label>categorized knowledge asset</rdfs:label>
  </owl:Class>

  <owl:Class rdf:about="&api4kp-kao;ImperativeAsset">
    <rdfs:subClassOf rdf:resource="&api4kp-kao;CategorizedKnowledgeAsset"/>
    <dct:identifier>7db1af1f-1703-356f-bddc-8cb0a81a442c</dct:identifier>
    <skos:prefLabel>Rules, Policies and Guidelines</skos:prefLabel>
  </owl:Class>

  <owl:Class rdf:about="&api4kp-kao;InferenceAsset">
    <rdfs:subClassOf rdf:resource="&api4kp-kao;CategorizedKnowledgeAsset"/>
    <dct:identifier>d4b0e868-60c8-387d-a139-e3c35427bfb6</dct:identifier>
    <skos:prefLabel xml:lang="en">Assessment, Predictive and Inferential Models</skos:prefLabel>
  </owl:Class>

  <owl:Class rdf:about="&api4kp-kao;InformationAsset">
    <rdfs:subClassOf rdf:resource="&api4kp-kao;CategorizedKnowledgeAsset"/>
    <dct:identifier>3f55a496-5ff3-3989-bf0a-15a61da8b09c</dct:identifier>
    <skos:prefLabel>Structured Information and Data Capture Models</skos:prefLabel>
  </owl:Class>

  <owl:Class rdf:about="&api4kp-kao;SemioticAsset">
    <rdfs:subClassOf rdf:resource="&api4kp-kao;CategorizedKnowledgeAsset"/>
    <dct:identifier>64719ac1-415f-3747-843c-e1e8949071ff</dct:identifier>
    <skos:prefLabel>Terminology, Ontology and Assertional KBs</skos:prefLabel>
  </owl:Class>

  <owl:Class rdf:about="&api4kp-kao;MetricAsset">
    <rdfs:subClassOf rdf:resource="&api4kp-kao;CategorizedKnowledgeAsset"/>
    <dct:identifier>2d705e5a-22d4-3368-98a6-e5ea7d52fd05</dct:identifier>
    <skos:prefLabel>KPIs, Measurements and Metrics</skos:prefLabel>
  </owl:Class>

  <owl:Class rdf:about="&api4kp-kao;ProcessAsset">
    <rdfs:subClassOf rdf:resource="&api4kp-kao;CategorizedKnowledgeAsset"/>
    <dct:identifier>f9e2a69d-0f6e-3a2b-94c4-beaf6fdadaea</dct:identifier>
    <skos:prefLabel>Plans, Processes, Pathways and Protocol Definitions</skos:prefLabel>
  </owl:Class>

  <owl:Class rdf:about="&api4kp-kao;OperationalConceptDefinition">
    <rdfs:subClassOf rdf:resource="&api4kp;ConstructiveDefinition"/>
    <rdfs:subClassOf rdf:resource="&api4kp-kao;ExplicitRoleKnowledgeAsset"/>
    <rdfs:subClassOf>
      <owl:Restriction>
        <owl:onProperty rdf:resource="&api4kp;defines"/>
        <owl:someValuesFrom rdf:resource="&api4kp;ResolvableConcept"/>
      </owl:Restriction>
    </rdfs:subClassOf>
    <rdfs:comment>Constructive Definition of a (resolvable) Concept that specifies how to resolve that Concept in some context or situation.
Some definitions have conditional applicability, limiting the class of situations in which they can be used</rdfs:comment>
    <rdfs:label>operational concept definition</rdfs:label>
  </owl:Class>

  <owl:Class rdf:about="&api4kp-kao;AssessmentModel">
    <rdfs:subClassOf rdf:resource="&api4kp-kao;InferenceAsset"/>
    <rdfs:comment>knowledge that allows to infer an otherwise unknown or not directly observable state or situation</rdfs:comment>
    <rdfs:label>assessment model</rdfs:label>
  </owl:Class>

  <owl:Class rdf:about="&api4kp-kao;CognitiveProcessModel">
    <rdfs:subClassOf rdf:resource="&api4kp-kao;ProcessAsset"/>
    <rdfs:subClassOf>
      <owl:Restriction>
        <owl:onProperty rdf:resource="&api4kp;has-part"/>
        <owl:someValuesFrom rdf:resource="&api4kp-kao;DecisionModel"/>
      </owl:Restriction>
    </rdfs:subClassOf>
    <rdfs:comment>Knowledge Asset that captures how information is processed internally by an intelligent agent</rdfs:comment>
    <rdfs:label>cognitive process model</rdfs:label>
  </owl:Class>

  <owl:Class rdf:about="&api4kp-ckao;PatientCohortDefinition">
    <rdfs:subClassOf rdf:resource="&api4kp-kao;InferenceAsset"/>
		<rdfs:subClassOf rdf:resource="&api4kp-ckao;ClinicalKnowledgeAsset"/>
    <rdfs:comment>Definition used to classify patients into classes defined by some common characteristic</rdfs:comment>
    <rdfs:label>patient cohort definition</rdfs:label>
  </owl:Class>

  <owl:Class rdf:about="&api4kp-kao;ComputableDecisionModel">
    <rdfs:subClassOf rdf:resource="&api4kp-kao;DecisionModel"/>
    <rdfs:comment>Decision Model that includes an explicit specification of its decision making logic, suitable to be faithfully expressed in a computable language</rdfs:comment>
    <rdfs:label>computable decision model</rdfs:label>
  </owl:Class>

  <owl:Class rdf:about="&api4kp-ckao;ClinicalDecisionModel">
    <rdfs:subClassOf rdf:resource="&api4kp-kao;DecisionModel"/>
    <rdfs:subClassOf rdf:resource="&api4kp-ckao;ClinicalKnowledgeAsset"/>
    <rdfs:comment>decision model capturing the knowledge used in the assessment of a patient's health status, or choice of intervention</rdfs:comment>
    <rdfs:label>clinical decision model</rdfs:label>
  </owl:Class>

  <owl:Class rdf:about="&api4kp-kao;NaturalisticDecisionModel">
    <rdfs:subClassOf rdf:resource="&api4kp-kao;DecisionModel"/>
    <rdfs:comment>decision model capturing how people make decisions in real life</rdfs:comment>
    <rdfs:label>naturalistic decision model</rdfs:label>
  </owl:Class>

  <owl:Class rdf:about="&api4kp-kao;ConceptualModel">
    <rdfs:subClassOf rdf:resource="&api4kp-kao;SemioticAsset"/>
    <rdfs:comment>Abstraction of the structure and/or behavior of the entities in a given domain</rdfs:comment>
    <rdfs:label>Conceptual (Domain) Model</rdfs:label>
    <skos:altLabel>domain conceptualization</skos:altLabel>
  </owl:Class>


  <owl:Class rdf:about="&api4kp-kao;AssertionalKnowledge">
    <rdfs:subClassOf rdf:resource="&api4kp-kao;SemioticAsset"/>
    <rdfs:comment>Knowledge that is held to be a faithful description of the state of affairs in a given domain by all agents that share (and understand) it.</rdfs:comment>
    <rdfs:label>assertional knowledge</rdfs:label>
  </owl:Class>

  <owl:Class rdf:about="&api4kp-kao;ContextualizableKnowledge">
    <rdfs:subClassOf rdf:resource="&api4kp-kao;AssertionalKnowledge"/>
    <rdfs:comment>Assertional knowledge that is not completely ground, and can be specialized or adapted to a particular context</rdfs:comment>
    <rdfs:label>contextualizable knowledge</rdfs:label>
  </owl:Class>

  <owl:Class rdf:about="&api4kp-kao;GroundedKnowledge">
    <rdfs:subClassOf rdf:resource="&api4kp-kao;AssertionalKnowledge"/>
    <rdfs:comment>Assertional knowledge about specific individuals, entities and concepts</rdfs:comment>
    <rdfs:label>grounded knowledge</rdfs:label>
  </owl:Class>

  <owl:Class rdf:about="&api4kp-kao;DecisionModel">
    <rdfs:subClassOf rdf:resource="&api4kp-kao;AssessmentModel"/>
    <rdfs:comment>Assessment that can be abstracted by means of a question, which requires to select one out of a set of admissible options</rdfs:comment>
    <rdfs:label>decision model</rdfs:label>
  </owl:Class>

  <owl:Class rdf:about="&api4kp-kao;CaseManagementModel">
    <rdfs:subClassOf rdf:resource="&api4kp-kao;ProcessAsset"/>
    <rdfs:comment>specification of how to handle a case</rdfs:comment>
    <rdfs:label>case management model</rdfs:label>
  </owl:Class>

  <owl:Class rdf:about="&api4kp-kao;DecisionTaskModel">
    <rdfs:subClassOf rdf:resource="&api4kp-kao;CognitiveProcessModel"/>
    <rdfs:subClassOf>
      <owl:Restriction>
        <owl:onProperty rdf:resource="&api4kp;part-of"/>
        <owl:someValuesFrom rdf:resource="&api4kp-kao;CognitiveProcessModel"/>
      </owl:Restriction>
    </rdfs:subClassOf>
    <rdfs:comment>Model of who, when, where and why a Decision is made, usually as part of a broader process. Also known as Decision Making Process Model, usually includes a Decision Model that specifies how to actually choose the optimal option</rdfs:comment>
    <rdfs:label>decision task model</rdfs:label>
  </owl:Class>

  <owl:Class rdf:about="&api4kp-kao;DocumentationTemplate">
    <rdfs:subClassOf rdf:resource="&api4kp-kao;InformationAsset"/>
    <rdfs:comment>An organized collection of determinable concepts, possibly associated to questions, which are meant to be resolved in a particular context</rdfs:comment>
    <rdfs:label>documentation template</rdfs:label>
    <skos:scopeNote>more general than questionnaires, whose questions are meant to be answered by a human agent (possibly with computer aid), documentation templates can be used  by software agents as well</skos:scopeNote>
  </owl:Class>


  <owl:Class rdf:about="&api4kp-kao;InteractiveDocumentationTemplate">
    <rdfs:subClassOf rdf:resource="&api4kp-kao;DocumentationTemplate"/>
    <rdfs:comment>Documentation template designed for human computer interaction, where the human fills a questionnaire, and a computer processes the gathered information to provide further insight to the human</rdfs:comment>
    <rdfs:label>interactive documentation template</rdfs:label>
  </owl:Class>

  <owl:Class rdf:about="&api4kp-kao;Equation">
    <rdfs:subClassOf rdf:resource="&api4kp-kao;FunctionalExpression"/>
    <rdfs:comment>A functional expression, defined in terms of two functional expressions connected by means of the well known equality operator.</rdfs:comment>
    <rdfs:label>equation</rdfs:label>
  </owl:Class>


  <owl:Class rdf:about="&api4kp-kao;FormalOntology">
    <rdfs:subClassOf rdf:resource="&api4kp-kao;ConceptualModel"/>
    <rdfs:comment>conceptual model that is based on formal principles, such as that allow to make inferences and/or verify the consistency of the model</rdfs:comment>
    <rdfs:label>formal ontology</rdfs:label>
  </owl:Class>

  <owl:Class rdf:about="&api4kp-kao;FunctionalExpression">
    <rdfs:subClassOf rdf:resource="&api4kp-kao;AssessmentModel"/>
    <rdfs:comment>Knowledge about the application of well-known information processing methods, possibly chained together, which are stateless, functional and idempotent in nature.</rdfs:comment>
    <rdfs:label>functional expression</rdfs:label>
    <skos:example>&apos;mass&apos; times the square of the speed of light</skos:example>
  </owl:Class>

  <owl:Class rdf:about="&api4kp-kao;InformationModel">
    <rdfs:subClassOf rdf:resource="&api4kp-kao;InformationAsset"/>
    <rdfs:comment>(Meta) model that defines which information should be captured about some kind of domain</rdfs:comment>
    <rdfs:label>information model</rdfs:label>
    <skos:altLabel>logical data model</skos:altLabel>
  </owl:Class>

  <owl:Class rdf:about="&api4kp-kao;InquirySpecification">
    <rdfs:subClassOf rdf:resource="&api4kp-kao;ProcessAsset"/>
    <rdfs:comment>The definition of how (and possibly when and where) to ask a question, following some kind of protocol, for the purpose of receiving a specific answer, with the goal of gaining information in the process</rdfs:comment>
    <rdfs:label>inquiry specification</rdfs:label>
  </owl:Class>

  <owl:Class rdf:about="&api4kp-kao;MultiAgentDecisionTaskModel">
    <rdfs:subClassOf rdf:resource="&api4kp-kao;DecisionTaskModel"/>
    <rdfs:comment>Decision Task Model that requires the participation of two or more agents</rdfs:comment>
    <rdfs:label>multi-agent decision task model</rdfs:label>
  </owl:Class>

  <owl:Class rdf:about="&api4kp-kao;PredictiveModel">
    <rdfs:subClassOf rdf:resource="&api4kp-kao;AssessmentModel"/>
    <rdfs:comment>assessment of some state that is unobservable due to being in the future</rdfs:comment>
    <rdfs:label>predictive model</rdfs:label>
  </owl:Class>

  <owl:Class rdf:about="&api4kp-kao;Protocol">
    <rdfs:subClassOf rdf:resource="&api4kp-kao;ProcessAsset"/>
    <rdfs:comment>A shared, endorsed, justified, imperative specification of the expected behavior of one or more agents in a specific situation</rdfs:comment>
    <rdfs:isDefinedBy rdf:resource="http://ontology.mayo.edu/ontology/KAO"/>
    <rdfs:label>protocol</rdfs:label>
  </owl:Class>

  <owl:Class rdf:about="&api4kp-kao;Questionnaire">
    <rdfs:subClassOf rdf:resource="&api4kp-kao;DocumentationTemplate"/>
    <rdfs:comment xml:lang="en">An organized collection of questions intended to solicit information from patients, providers or other individuals in the healthcare domain</rdfs:comment>
    <rdfs:isDefinedBy rdf:resource="http://ontology.mayo.edu/ontology/KAO"/>
    <rdfs:label xml:lang="en">questionnaire</rdfs:label>
    <skos:example xml:lang="en">First Visit Questionnaire</skos:example>
  </owl:Class>

  <owl:Class rdf:about="&api4kp-kao;SemanticDecisionModel">
    <rdfs:subClassOf rdf:resource="&api4kp-kao;DecisionModel"/>
    <rdfs:comment>Decision Model that includes an unambiguous definition of every concept involved</rdfs:comment>
    <rdfs:label>semantic decision model</rdfs:label>
  </owl:Class>

  <owl:Class rdf:about="&api4kp-kao;SemanticInformationModel">
    <rdfs:subClassOf rdf:resource="&api4kp-kao;InformationModel"/>
    <rdfs:subClassOf>
      <owl:Restriction>
        <owl:onProperty rdf:resource="&api4kp;has-part"/>
        <owl:someValuesFrom rdf:resource="&api4kp-kao;SemanticInformationModel"/>
      </owl:Restriction>
    </rdfs:subClassOf>
    <rdfs:comment>Information Model designed such that instances have one and only one interpretation</rdfs:comment>
    <rdfs:label>semantic information model</rdfs:label>
  </owl:Class>

  <owl:Class rdf:about="&api4kp-kao;ServiceDescription">
    <rdfs:subClassOf rdf:resource="&api4kp-kao;ProcessAsset"/>
    <rdfs:label>service description</rdfs:label>
  </owl:Class>

  <owl:Class rdf:about="&api4kp-kao;ServiceProfile">
    <rdfs:subClassOf rdf:resource="&api4kp-kao;ServiceDescription"/>
    <rdfs:comment>Service Description that refines (by constraint), and thus depends on, some Service Description</rdfs:comment>
    <rdfs:label>service profile</rdfs:label>
  </owl:Class>

  <owl:Class rdf:about="&api4kp-kao;ServiceSpecification">
    <rdfs:subClassOf rdf:resource="&api4kp-kao;ServiceDescription"/>
    <rdfs:comment>Formal Service Description</rdfs:comment>
    <rdfs:label>service specification</rdfs:label>
  </owl:Class>

  <owl:Class rdf:about="&api4kp-kao;RESTfulServiceSpecification">
    <rdfs:subClassOf rdf:resource="&api4kp-kao;ServiceSpecification"/>
    <rdfs:comment>Specification of a ReSTful service, i.e. one which exposes resources at endpoints</rdfs:comment>
    <rdfs:label>ReSTful service specification</rdfs:label>
  </owl:Class>

  <owl:Class rdf:about="&api4kp-kao;OperationOrientedServiceSpecification">
    <rdfs:subClassOf rdf:resource="&api4kp-kao;ServiceSpecification"/>
    <rdfs:comment>Specification of a Operation-oriented service, i.e. one which exposes operations at endpoints</rdfs:comment>
    <rdfs:label>operation oriented service specification</rdfs:label>
  </owl:Class>


  <owl:Class rdf:about="&api4kp-kao;ValueSet">
    <rdfs:subClassOf rdf:resource="&api4kp-kao;SemioticAsset"/>
    <rdfs:comment xml:lang="en">A set of pairs of &quot;codes&quot;, drawn from one or more code systems, and human-readable terms that represent clinical concepts (e.g. &quot;diabetes type II&quot;)</rdfs:comment>
    <rdfs:isDefinedBy rdf:resource="http://ontology.mayo.edu/ontology/KAO"/>
    <rdfs:label xml:lang="en">value set</rdfs:label>
    <skos:example xml:lang="en">The Asthma Value Set</skos:example>
  </owl:Class>

	<owl:Class rdf:about="&api4kp-ckao;CareProcessModel">
		<rdfs:subClassOf rdf:resource="&api4kp-ckao;ClinicalKnowledgeAsset"/>
		<rdfs:subClassOf rdf:resource="&api4kp-kao;ProcessAsset"/>
		<rdfs:label xml:lang="en">care process model</rdfs:label>
		<skos:altLabel xml:lang="en">CPM</skos:altLabel>
		<skos:definition>adaptive specification of how to perform (complex) clinical activities, properly orchestrated over time, so to achieve certain objectives and goals</skos:definition>
		<skos:example xml:lang="en">The Mayo Clinic Rectal Adenocarcinoma CPM</skos:example>
		<skos:scopeNote xml:lang="en">Includes AME Care Process Models (CPM)</skos:scopeNote>
	</owl:Class>
	
	<owl:Class rdf:about="&api4kp-ckao;CaseEnrichmentRule">
		<rdfs:subClassOf rdf:resource="&api4kp-ckao;ClinicalRule"/>
		<rdfs:label>case enrichment rule</rdfs:label>
		<skos:definition>clinical rule, or set thereof, that uses summarization, inference, guidance and contextualization logic to augment a patient&apos;s case, with respect to a disorder that the case is centered on</skos:definition>
	</owl:Class>
	
	<owl:Class rdf:about="&api4kp-ckao;CaseSummarizationRule">
		<rdfs:subClassOf rdf:resource="&api4kp-ckao;CaseEnrichmentRule"/>
		<rdfs:label>case summarization rule</rdfs:label>
		<skos:definition>clinical rule, or set thereof, that extracts salient &apos;features&apos; from a patient case</skos:definition>
		<skos:scopeNote>A summarization rule does not generate new information, but rather selects information that is already present.</skos:scopeNote>
	</owl:Class>
	
	<owl:Class rdf:about="&api4kp-ckao;ClinicalCalculationRule">
		<rdfs:subClassOf rdf:resource="&api4kp-ckao;ClinicalInferenceRule"/>
		<rdfs:label>clinical calculation rule</rdfs:label>
		<skos:definition>clinical inference rule that determines a single, derived, &apos;observed&apos; value</skos:definition>
	</owl:Class>
	
	<owl:Class rdf:about="&api4kp-ckao;ClinicalContextualizationRule">
		<rdfs:subClassOf rdf:resource="&api4kp-ckao;ClinicalInferenceRule"/>
		<rdfs:label>clinical contextualization rule</rdfs:label>
		<skos:definition>clinical inference rule that &quot;projects&quot; the patient&apos;s state around a set of (usually related) concepts, effectively creating a focused context</skos:definition>
	</owl:Class>
	
	<owl:Class rdf:about="&api4kp-ckao;ClinicalEligibilityRule">
		<rdfs:subClassOf rdf:resource="&api4kp-ckao;ClinicalRule"/>
		<rdfs:label>clinical eligibility rule</rdfs:label>
		<skos:definition>clinical rule that determines whether a treatment, or study thereof, is potentially administrable to a patient (cohort), based on the patient&apos;s characteristics</skos:definition>
	</owl:Class>
	
	<owl:Class rdf:about="&api4kp-ckao;ClinicalEnrollmentRule">
		<rdfs:subClassOf rdf:resource="&api4kp-ckao;ClinicalRule"/>
		<rdfs:label>clinical enrollment rule</rdfs:label>
		<skos:definition>clinical rule that determines whether a patient will be administered care, as specified by a care process, pathway or protocol</skos:definition>
	</owl:Class>
	
	<owl:Class rdf:about="&api4kp-ckao;ClinicalGuidanceRule">
		<rdfs:subClassOf rdf:resource="&api4kp-ckao;CaseEnrichmentRule"/>
		<rdfs:label>clinical guidance rule</rdfs:label>
		<skos:definition>clinical rule, or set thereof, that uses a patient&apos;s (possibly summarized) case, to produce a recommendation, (i.e. a proposed strategy) to address a gap between the current and desired state</skos:definition>
		<skos:scopeNote>The information generated by guidance rules is generally meant to be a (partial) intervention plan, and thus drive an agent&apos;s action.</skos:scopeNote>
	</owl:Class>
	
	<owl:Class rdf:about="&api4kp-ckao;ClinicalInferenceRule">
		<rdfs:subClassOf rdf:resource="&api4kp-ckao;CaseEnrichmentRule"/>
		<rdfs:label>clinical inference rule</rdfs:label>
		<skos:definition>clinical rule, or set thereof, that uses a patient&apos;s (possibly summarized) case, to assess the patient&apos;s state, predict the case&apos;s course, and/or determine (contra)indicated intervention options</skos:definition>
		<skos:scopeNote>Inference rules generate new information based on the current state, and knowledge that dictates how to interpret that state. Inference rules, however, do not drive actions/interventions directly.</skos:scopeNote>
	</owl:Class>

	<owl:Class rdf:about="&api4kp-ckao;ClinicalPracticeGuideline">
		<rdfs:subClassOf rdf:resource="&api4kp-ckao;ClinicalKnowledgeAsset"/>
		<rdfs:subClassOf rdf:resource="&api4kp-kao;ImperativeAsset"/>
		<rdfs:label xml:lang="en">clinical practice guideline</rdfs:label>
		<rdfs:seeAlso rdf:resource="http://mayoweb.mayo.edu/pmr/documents/PracticeGuidelineTemplateSternotomy.pdf"/>
		<skos:altLabel xml:lang="en">clinical practice guideline</skos:altLabel>
		<skos:definition xml:lang="en">systematically developed statement(s) that assist provider decisions about appropriate healthcare for specific clinical situations</skos:definition>
		<skos:example xml:lang="en">The Mayo Clinic Sternotomy Guideline</skos:example>
	</owl:Class>
	
	<owl:Class rdf:about="&api4kp-ckao;ClinicalProtocol">
		<rdfs:subClassOf rdf:resource="&api4kp-kao;Protocol"/>
		<rdfs:subClassOf rdf:resource="&api4kp-ckao;ClinicalKnowledgeAsset"/>
		<rdfs:label>clinical protocol</rdfs:label>
		<skos:definition>protocol applicable in a clinical situation, such that it directs the behavior of patients and/or providers</skos:definition>
	</owl:Class>
	
	<owl:Class rdf:about="&api4kp-ckao;ClinicalRule">
		<rdfs:subClassOf rdf:resource="&api4kp-ckao;ClinicalKnowledgeAsset"/>
		<rdfs:subClassOf rdf:resource="&api4kp-kao;ImperativeAsset"/>
		<rdfs:label xml:lang="en">clinical rule</rdfs:label>
		<rdfs:seeAlso rdf:resource="https://clinicalknowledgemanagement.mayo.edu/mayo-clinic-rules-catalog/asset/km-asset/KAT-20323041"/>
		<skos:definition xml:lang="en">computational logic to direct clinical interventions that are typically expressed as if/then statements but may also be represented by a diagram, decision table or other representation language</skos:definition>
		<skos:example xml:lang="en">The &apos;HGB value prior to RBC transfusion&apos; Recommendation Rule</skos:example>
	</owl:Class>
	
	<owl:Class rdf:about="&api4kp-ckao;ClinicalTrialProtocol">
		<rdfs:subClassOf rdf:resource="&api4kp-ckao;ClinicalProtocol"/>
		<rdfs:label>clinical trial protocol</rdfs:label>
		<rdfs:isDefinedBy>https://www.ncbi.nlm.nih.gov/pubmed/20815294</rdfs:isDefinedBy>
		<skos:definition>descriptions of the objectives, design, methodology, statistical considerations and aspects related to the organization of clinical trials</skos:definition>
		<skos:note>Trial protocols provide the background and rationale for conducting a study, highlighting specific research questions that are addressed, and taking into consideration ethical issues. Trial protocols must meet a standard that adheres to the principles of Good Clinical Practice, and are used to obtain ethics approval by local Ethics Committees or Institutional Review Boards.</skos:note>
	</owl:Class>
	
	<owl:Class rdf:about="&api4kp-ckao;CognitiveCareProcessModel">
		<rdfs:subClassOf rdf:resource="&api4kp-ckao;CareProcessModel"/>
		<rdfs:subClassOf rdf:resource="&api4kp-ckao;CognitiveProcessModel"/>
		<rdfs:label>cognitive care process model</rdfs:label>
		<skos:definition>knowledge whose primary subject covers the cognitive aspects of a care process</skos:definition>
	</owl:Class>

	<owl:Class rdf:about="&api4kp-ckao;ClinicalPathway">
		<rdfs:subClassOf rdf:resource="&api4kp-ckao;CareProcessModel"/>
		<rdfs:label>clinical pathway</rdfs:label>
		<skos:definition>specification of a possible, ideal course of action for the diagnosis or treatment of a condition</skos:definition>
	</owl:Class>

	<owl:Class rdf:about="&api4kp-ckao;ClinicalCaseManagementModel">
	  <rdfs:subClassOf rdf:resource="&api4kp-ckao;ClinicalKnowledgeAsset"/>
		<rdfs:subClassOf rdf:resource="&api4kp-kao;CaseManagementModel"/>
		<rdfs:label>clinical case management model</rdfs:label>
		<skos:definition>knowledge of how to manage a person's diagnosis of a clinical condition</skos:definition>
	</owl:Class>

	
	<owl:Class rdf:about="&api4kp-ckao;ClinicalDecisionSupportInteraction">
		<rdfs:subClassOf rdf:resource="&api4kp-kao;Protocol"/>
		<rdfs:subClassOf rdf:resource="&api4kp-ckao;ClinicalKnowledgeAsset"/>
		<rdfs:label>clinical decision support interaction</rdfs:label>
		<skos:definition>decision support interaction that delivers an alert, a reminder or a recommendation</skos:definition>
	</owl:Class>

	
	<owl:Class rdf:about="&api4kp-ckao;NursingProtocol">
		<rdfs:subClassOf rdf:resource="&api4kp-ckao;ClinicalProtocol"/>
		<rdfs:label>nursing protocol</rdfs:label>
		<skos:definition>protocol that directs the behavior of nurses</skos:definition>
	</owl:Class>
	
	<owl:Class rdf:about="&api4kp-ckao;OrderSet">
		<rdfs:subClassOf rdf:resource="&api4kp-ckao;ClinicalKnowledgeAsset"/>
		<rdfs:subClassOf rdf:resource="&api4kp-kao;ProcessAsset"/>
		<rdfs:label xml:lang="en">order set</rdfs:label>
		<skos:definition xml:lang="en">a standardized list of orders for a specific diagnosis</skos:definition>
		<skos:editorialNote xml:lang="en">Verify the defintion that restricts the order sets to be developed by OSPAG, vs produced or endorsed</skos:editorialNote>
		<skos:example xml:lang="en">The Heart Failure Medication Titration Order Set</skos:example>
	</owl:Class>

	<owl:Class rdf:about="&api4kp-ckao;TherapyPlan">
		<rdfs:subClassOf rdf:resource="&api4kp-ckao;ClinicalKnowledgeAsset"/>
		<rdfs:subClassOf rdf:resource="&api4kp-kao;ProcessAsset"/>
		<rdfs:label xml:lang="en">therapy plan</rdfs:label>
		<skos:definition xml:lang="en">TODO composite orderset ? that spans over multiple encounters, aimed at the treatment of a specific disorder</skos:definition>
	</owl:Class>

	<owl:Class rdf:about="&api4kp-kao;QualityMeasure">
		<rdfs:subClassOf rdf:resource="&api4kp-kao;MetricAsset"/>
		<rdfs:label xml:lang="en">quality measure</rdfs:label>
		<skos:definition>tool that helps measure or quantify healthcare processes, outcomes, patient perceptions and organizational structure and/or systems that are associated with the ability to provide high-quality healthcare and/or that relate to one or more quality goals</skos:definition>
	</owl:Class>

	<owl:Class rdf:about="&api4kp-ckao;ClinicalQualityMeasure">
		<rdfs:subClassOf rdf:resource="&api4kp-kao;QualityMeasure"/>
		<rdfs:subClassOf rdf:resource="&api4kp-ckao;ClinicalKnowledgeAsset"/>
		<rdfs:label xml:lang="en">clinical quality measure</rdfs:label>
		<skos:definition>quality measure applied to patient cohorts</skos:definition>
	</owl:Class>

  <owl:Class rdf:about="&api4kp-kao;Lexicon">
    <rdfs:subClassOf rdf:resource="&api4kp-kao;SemioticAsset"/>
    <rdfs:subClassOf rdf:resource="&api4kp;Lexicon"/>
    <rdfs:label xml:lang="en">lexicon</rdfs:label>
  </owl:Class>

  <owl:Class rdf:about="&api4kp-kao;GrammarSpecification">
    <rdfs:subClassOf rdf:resource="&api4kp-kao;InformationAsset"/>
    <rdfs:subClassOf rdf:resource="&api4kp-lang;Grammar"/>
    <rdfs:label xml:lang="en">grammar specification</rdfs:label>
  </owl:Class>

  <owl:Class rdf:about="&api4kp;ConstructiveDefinition">
  </owl:Class>

    <owl:Class rdf:about="&api4kp;Definition">
  		<rdfs:subClassOf rdf:resource="&api4kp-kao;SemioticAsset"/>
	 </owl:Class>>

  <owl:Class rdf:about="&api4kp-kao;ExplicitRoleKnowledgeAsset">
  		<rdfs:subClassOf rdf:resource="&api4kp;KnowledgeAsset"/>
  		<rdfs:label>explicit role knowledge asset</rdfs:label>
	</owl:Class>

	<owl:Class rdf:about="&api4kp-kao;CompositeKnowledgeAsset">
  		<rdfs:subClassOf rdf:resource="&api4kp-kao;ExplicitRoleKnowledgeAsset"/>
	</owl:Class>

	<owl:Class rdf:about="&api4kp-kao;ComponentKnowledgeAsset">
  		<rdfs:subClassOf rdf:resource="&api4kp-kao;ExplicitRoleKnowledgeAsset"/>
	</owl:Class>

  <owl:Class rdf:about="&api4kp;KnowledgeAsset">
  </owl:Class>

  <owl:Class rdf:about="&api4kp;ResolvableConcept">
  </owl:Class>

</rdf:RDF>