<?xml version="1.0" encoding="UTF-8"?>
<!DOCTYPE rdf:RDF [
	<!ENTITY api4kp "https://www.omg.org/spec/API4KP/api4kp/">
	<!ENTITY kp "https://www.omg.org/spec/API4KP/api4kp-kp/">
	<!ENTITY dct "http://purl.org/dc/terms/">
	<!ENTITY lcc-lr "https://www.omg.org/spec/LCC/Languages/LanguageRepresentation/">
	<!ENTITY rdf "http://www.w3.org/1999/02/22-rdf-syntax-ns#">
	<!ENTITY rdfs "http://www.w3.org/2000/01/rdf-schema#">
	<!ENTITY owl "http://www.w3.org/2002/07/owl#">
	<!ENTITY skos "http://www.w3.org/2004/02/skos/core#">
	<!ENTITY sm "http://www.omg.org/techprocess/ab/SpecificationMetadata/">
	<!ENTITY xsd "http://www.w3.org/2001/XMLSchema#">
]>

<rdf:RDF xml:base="https://www.omg.org/spec/API4KP/api4kp-kp/"
	xmlns:dct="http://purl.org/dc/terms/"
    xmlns:api4kp="https://www.omg.org/spec/API4KP/api4kp/"
	xmlns:kp="https://www.omg.org/spec/API4KP/api4kp-kp/"
    xmlns:lcc-lr="https://www.omg.org/spec/LCC/Languages/LanguageRepresentation/"
	xmlns:owl="http://www.w3.org/2002/07/owl#"
	xmlns:rdf="http://www.w3.org/1999/02/22-rdf-syntax-ns#"
	xmlns:rdfs="http://www.w3.org/2000/01/rdf-schema#"
	xmlns:skos="http://www.w3.org/2004/02/skos/core#"
	xmlns:sm="http://www.omg.org/techprocess/ab/SpecificationMetadata/"
	xmlns:xsd="http://www.w3.org/2001/XMLSchema#">
	
	<owl:Ontology rdf:about="https://www.omg.org/spec/API4KP/api4kp-kp/">
		<rdfs:label>API4KP Ontology of Knowledge Platforms</rdfs:label>
        <dct:abstract>This ontology formalizes the notion of a Knowledge Platform.</dct:abstract>
        <dct:creator>Davide Sottara (sottara.davide@mayo.edu)</dct:creator>
		<dct:license rdf:datatype="&xsd;anyURI">http://opensource.org/licenses/MIT</dct:license>
        <sm:copyright>Copyright (c) 2014-2020 88 Solutions</sm:copyright>
		<sm:copyright>Copyright (c) 2014-2020 Adaptive</sm:copyright>
        <sm:copyright>Copyright (c) 2014-2020 Athan Services</sm:copyright>
        <sm:copyright>Copyright (c) 2014-2020 Arizona State University</sm:copyright>
	    <sm:copyright>Copyright (c) 2014-2020 Fraunhofer FOKUS</sm:copyright>
        <sm:copyright>Copyright (c) 2014-2020 Freie Universitat Berlin</sm:copyright>
		<sm:copyright>Copyright (c) 2014-2020 Mayo Clinic</sm:copyright>
	    <sm:copyright>Copyright (c) 2019-2020 Micro Focus</sm:copyright>
		<sm:copyright>Copyright (c) 2014-2020 Model Driven Solutions</sm:copyright>
		<sm:copyright>Copyright (c) 2014-2020 Thematix Partners LLC</sm:copyright>
		<sm:copyright>Copyright (c) 2015-2020 Object Management Group, Inc.</sm:copyright>
		<sm:contentLanguage rdf:datatype="&xsd;anyURI">http://www.w3.org/standards/techs/owl#w3c_all</sm:contentLanguage>
		<sm:dependsOn rdf:datatype="&xsd;anyURI">https://www.omg.org/spec/LCC/</sm:dependsOn>
		<sm:dependsOn rdf:datatype="&xsd;anyURI">https://www.omg.org/spec/API4KP/api4kp/</sm:dependsOn>
		<sm:filename>api4kp-kp.rdf</sm:filename>
		<sm:fileAbbreviation>kp</sm:fileAbbreviation>
        <owl:imports rdf:resource="http://www.omg.org/techprocess/ab/SpecificationMetadata/"/>
        <owl:imports rdf:resource="https://www.omg.org/spec/LCC/Languages/LanguageRepresentation/"/>
        <owl:imports rdf:resource="https://www.omg.org/spec/API4KP/api4kp/"/>
        <owl:versionIRI rdf:resource="https://www.omg.org/spec/API4KP/SNAPSHOT/api4kp-kp/"/>
   </owl:Ontology>


    <!-- 
    ///////////////////////////////////////////////////////////////////////////////////////
    //
    // Object Properties
    //
    ///////////////////////////////////////////////////////////////////////////////////////
     -->

    <owl:ObjectProperty rdf:about="&kp;deployment-of">
        <rdfs:domain rdf:resource="&kp;DeployedSoftware"/>
        <rdfs:range rdf:resource="&api4kp;Software"/>
        <rdfs:label>deployment of</rdfs:label>
    </owl:ObjectProperty>

    <owl:ObjectProperty rdf:about="&kp;executes">
        <rdfs:domain rdf:resource="&kp;ExecutionEnvironment"/>
        <rdfs:range rdf:resource="&kp;SoftwareExecution"/>
        <rdfs:label>executes</rdfs:label>
        <skos:definition>The relationship between an environment that provides the computational resources (e.g. CPU, memory, I/O) which enable the act of executing the instructions specified by some software, and that act.</skos:definition>
    </owl:ObjectProperty>

    <owl:ObjectProperty rdf:about="&kp;hosts">
        <rdfs:domain rdf:resource="&kp;ExecutionEnvironment"/>
        <rdfs:range rdf:resource="&kp;DeployedSoftware"/>
        <owl:propertyChainAxiom rdf:parseType="Collection">
            <rdf:Description rdf:about="&kp;executes"/>
            <rdf:Description rdf:about="&kp;sustains"/>
        </owl:propertyChainAxiom>
        <skos:definition>The relationship between an execution environment, and a software that has been launched and/or deployed in that environment</skos:definition>
    </owl:ObjectProperty>

    <owl:ObjectProperty rdf:about="&kp;instantiation-of">
        <rdfs:domain rdf:resource="&kp;SoftwareExecution"/>
        <rdfs:range rdf:resource="&api4kp;Software"/>
        <owl:propertyChainAxiom rdf:parseType="Collection">
            <rdf:Description rdf:about="&kp;sustains"/>
            <rdf:Description rdf:about="&kp;deployment-of"/>
        </owl:propertyChainAxiom>
        <rdfs:comment>The relationship between a Software Execution, and the Software that was run during that execution</rdfs:comment>
        <rdfs:label>instantiation of</rdfs:label>
    </owl:ObjectProperty>
    
    <owl:ObjectProperty rdf:about="&kp;runs">
        <rdfs:domain rdf:resource="&kp;ExecutionEnvironment"/>
        <rdfs:range rdf:resource="&api4kp;Software"/>
        <owl:propertyChainAxiom rdf:parseType="Collection">
            <rdf:Description rdf:about="&kp;executes"/>
            <rdf:Description rdf:about="&kp;instantiation-of"/>
        </owl:propertyChainAxiom>
        <owl:propertyChainAxiom rdf:parseType="Collection">
            <rdf:Description rdf:about="&kp;executes"/>
            <rdf:Description rdf:about="&kp;sustains"/>
            <rdf:Description rdf:about="&kp;deployment-of"/>
        </owl:propertyChainAxiom>
        <owl:propertyChainAxiom rdf:parseType="Collection">
            <rdf:Description rdf:about="&kp;hosts"/>
            <rdf:Description rdf:about="&kp;deployment-of"/>
        </owl:propertyChainAxiom>
        <skos:definition>The relationship that holds between an execution environment, and any software (code) that is being run on that environment at a given point in time.

More specifically, an environment runs a software if there is an execution activity in progress that uses computational resources of that environment to execute a program, as specified by the instructions in the software source code.</skos:definition>
    </owl:ObjectProperty>

    <owl:ObjectProperty rdf:about="&kp;sustains">
        <rdfs:domain rdf:resource="&kp;SoftwareExecution"/>
        <rdfs:range rdf:resource="&kp;DeployedSoftware"/>
        <rdfs:comment>The relationship between the execution of a software by a (virtual) machine, and its &quot;phenotypical&quot; manifestation</rdfs:comment>
    </owl:ObjectProperty>

    <owl:ObjectProperty rdf:about="&api4kp;internally-represents">
        <rdfs:domain rdf:resource="&kp;DeployedSoftware"/>
    </owl:ObjectProperty>
    
 
    <!-- 
    ///////////////////////////////////////////////////////////////////////////////////////
    //
    // Classes
    //
    ///////////////////////////////////////////////////////////////////////////////////////
     -->

    <owl:Class rdf:about="&kp;AgentiveRole"/>

    <owl:Class rdf:about="&kp;DLReasoner">
        <rdfs:subClassOf rdf:resource="&kp;Reasoner"/>
        <rdfs:label>description logic reasoner</rdfs:label>
        <skos:definition>reasoner that supports reasoning operations with expressions that use a language that supports some of, and only, the aspects of description logics</skos:definition>
    </owl:Class>

    <owl:Class rdf:about="&kp;DeployedSoftware">
        <rdfs:subClassOf rdf:resource="&api4kp;KnowledgeArtifact"/>
        <rdfs:subClassOf>
            <owl:Restriction>
                <owl:onProperty rdf:resource="&kp;deployment-of"/>
                <owl:someValuesFrom rdf:resource="&api4kp;Software"/>
            </owl:Restriction>
        </rdfs:subClassOf>
        <rdfs:comment>test</rdfs:comment>
        <rdfs:label>Deployed Software</rdfs:label>
        <rdfs:label>Deployed Software Module</rdfs:label>
        <skos:definition>A packaged copy of a Software, which has been deployed (installed) on some Execution Environment</skos:definition>
    </owl:Class>
    
    <owl:Class rdf:about="&kp;ExecutionEnvironment">
        <rdfs:subClassOf>
            <owl:Restriction>
                <owl:onProperty rdf:resource="&kp;hosts"/>
                <owl:someValuesFrom rdf:resource="&kp;DeployedSoftware"/>
            </owl:Restriction>
        </rdfs:subClassOf>
        <rdfs:subClassOf>
            <owl:Restriction>
                <owl:onProperty rdf:resource="&kp;runs"/>
                <owl:someValuesFrom rdf:resource="&api4kp;Software"/>
            </owl:Restriction>
        </rdfs:subClassOf>
        <rdfs:label>Execution Environment</rdfs:label>
        <skos:definition>General concept that abstracts hardware, OS, Virtual Machines, Containers, or combinations thereof</skos:definition>
    </owl:Class>

    <owl:Class rdf:about="&kp;KnowledgePlatform">
        <owl:equivalentClass>
            <owl:Class>
                <owl:intersectionOf rdf:parseType="Collection">
                    <rdf:Description rdf:about="&kp;ExecutionEnvironment"/>
                    <owl:Restriction>
                        <owl:onProperty rdf:resource="&kp;hosts"/>
                        <owl:someValuesFrom>
                            <owl:Class>
                                <owl:intersectionOf rdf:parseType="Collection">
                                    <rdf:Description rdf:about="&kp;KnowledgePlatformModule"/>
                                    <owl:Restriction>
                                        <owl:onProperty rdf:resource="&api4kp;performs"/>
                                        <owl:someValuesFrom rdf:resource="&api4kp;KnowledgeActivity"/>
                                    </owl:Restriction>
                                </owl:intersectionOf>
                            </owl:Class>
                        </owl:someValuesFrom>
                    </owl:Restriction>
                </owl:intersectionOf>
            </owl:Class>
        </owl:equivalentClass>
        <rdfs:subClassOf rdf:resource="&kp;ExecutionEnvironment"/>
        <rdfs:label>Knowledge Platform</rdfs:label>
    </owl:Class>

    <owl:Class rdf:about="&kp;KnowledgePlatformModule">
        <rdfs:subClassOf rdf:resource="&kp;Server"/>
        <rdfs:subClassOf rdf:resource="&api4kp;Agent"/>
        <rdfs:subClassOf>
            <owl:Restriction>
                <owl:onProperty rdf:resource="&api4kp;internally-represents"/>
                <owl:someValuesFrom rdf:resource="&api4kp;KnowledgeResource"/>
            </owl:Restriction>
        </rdfs:subClassOf>
        <rdfs:subClassOf>
            <owl:Restriction>
                <owl:onProperty rdf:resource="&api4kp;part-of"/>
                <owl:someValuesFrom rdf:resource="&kp;KnowledgePlatform"/>
            </owl:Restriction>
        </rdfs:subClassOf>
        <rdfs:subClassOf>
            <owl:Restriction>
                <owl:onProperty rdf:resource="&api4kp;performs"/>
                <owl:someValuesFrom rdf:resource="&api4kp;KnowledgeActivity"/>
            </owl:Restriction>
        </rdfs:subClassOf>
        <rdfs:label>Knowledge Platform Component</rdfs:label>
        <rdfs:label>Knowledge Platform Module</rdfs:label>
    </owl:Class>

    <owl:Class rdf:about="&kp;ProductionRuleEngine">
        <rdfs:subClassOf rdf:resource="&kp;RuleEngine"/>
        <rdfs:label>production rule engine</rdfs:label>
        <skos:definition>rule engine optimized for production (condition-action) rules</skos:definition>
    </owl:Class>

    <owl:Class rdf:about="&kp;Reasoner">
        <rdfs:subClassOf rdf:resource="&api4kp;Software"/>
        <rdfs:comment>software that has the capability of performing reasoning operations</rdfs:comment>
        <rdfs:label>reasoner</rdfs:label>
        <skos:altLabel>engine</skos:altLabel>
    </owl:Class>

    <owl:Class rdf:about="&kp;RuleEngine">
        <rdfs:subClassOf rdf:resource="&kp;Reasoner"/>
        <rdfs:label>rule engine</rdfs:label>
        <skos:definition>reasoner that supports reasoning operations performed on rule bases - structured knowldege bases whose elements are expressed in some rule language that supports logic aspects commonly used to construct &apos;if-then&apos; rules</skos:definition>
    </owl:Class>

    <owl:Class rdf:about="&kp;Server">
        <rdfs:subClassOf rdf:resource="&kp;AgentiveRole"/>
        <rdfs:subClassOf rdf:resource="&kp;DeployedSoftware"/>
        <rdfs:subClassOf>
            <owl:Class>
                <owl:intersectionOf rdf:parseType="Collection">
                    <rdf:Description rdf:about="&kp;AgentiveRole"/>
                    <owl:Restriction>
                        <owl:onProperty rdf:resource="&api4kp;archetypes"/>
                        <owl:someValuesFrom rdf:resource="&api4kp;Software"/>
                    </owl:Restriction>
                </owl:intersectionOf>
            </owl:Class>
        </rdfs:subClassOf>
        <rdfs:label>TODO server</rdfs:label>
    </owl:Class>

    <owl:Class rdf:about="&kp;SoftwareExecution">
        <rdfs:subClassOf rdf:resource="&api4kp;Activity"/>
        <rdfs:subClassOf>
            <owl:Restriction>
                <owl:onProperty rdf:resource="&kp;sustains"/>
                <owl:someValuesFrom rdf:resource="&kp;DeployedSoftware"/>
            </owl:Restriction>
        </rdfs:subClassOf>
        <rdfs:comment>The process by which a (virtual) machine interpretes and executes the instructions that are fragments of a Software.</rdfs:comment>
        <rdfs:label>Software Execution</rdfs:label>
    </owl:Class>
    
</rdf:RDF>
