<?xml version="1.0"?>
<rdf:RDF xmlns="https://www.omg.org/spec/API4KP/api4kp-kao/"
     xml:base="https://www.omg.org/spec/API4KP/api4kp-kao/"
     xmlns:sm="http://www.omg.org/techprocess/ab/SpecificationMetadata/"
     xmlns:dct="http://purl.org/dc/terms/"
     xmlns:kao="https://www.omg.org/spec/API4KP/api4kp-kao/"
     xmlns:owl="http://www.w3.org/2002/07/owl#"
     xmlns:rdf="http://www.w3.org/1999/02/22-rdf-syntax-ns#"
     xmlns:xml="http://www.w3.org/XML/1998/namespace"
     xmlns:xsd="http://www.w3.org/2001/XMLSchema#"
     xmlns:rdfs="http://www.w3.org/2000/01/rdf-schema#"
     xmlns:skos="http://www.w3.org/2004/02/skos/core#"
     xmlns:api4kp="https://www.omg.org/spec/API4KP/api4kp/"
     xmlns:lcc-lr="https://www.omg.org/spec/LCC/Languages/LanguageRepresentation/">
    <owl:Ontology rdf:about="https://www.omg.org/spec/API4KP/api4kp-kao/">
        <owl:versionIRI rdf:resource="https://www.omg.org/spec/API4KP/SNAPSHOT/api4kp-kao/"/>
        <owl:imports rdf:resource="http://www.omg.org/techprocess/ab/SpecificationMetadata/"/>
        <owl:imports rdf:resource="https://www.omg.org/spec/API4KP/api4kp/"/>
        <owl:imports rdf:resource="https://www.omg.org/spec/LCC/Languages/LanguageRepresentation/"/>
        <dct:abstract>This ontology formalizes the notion of types of Knowledge Assets along two dimensions: (i) the underlying logical and mathematical aspects, which influence what kind of reasoning capabilities are required to process the knowledge, and determine the kind of actions that can be empowered by that knowledge; (ii) the compatibility relationship with languages that are expressive enough to capture assets of that type, i.e. have adequate language aspects to express the underlying logical/mathematical aspects.</dct:abstract>
        <dct:creator>Davide Sottara (sottara.davide@mayo.edu)</dct:creator>
        <dct:license rdf:datatype="http://www.w3.org/2001/XMLSchema#anyURI">http://opensource.org/licenses/MIT</dct:license>
        <sm:contentLanguage rdf:datatype="http://www.w3.org/2001/XMLSchema#anyURI">http://www.w3.org/standards/techs/owl#w3c_all</sm:contentLanguage>
        <sm:copyright>Copyright (c) 2014-2020 88 Solutions</sm:copyright>
        <sm:copyright>Copyright (c) 2014-2020 Adaptive</sm:copyright>
        <sm:copyright>Copyright (c) 2014-2020 Arizona State University</sm:copyright>
        <sm:copyright>Copyright (c) 2014-2020 Athan Services</sm:copyright>
        <sm:copyright>Copyright (c) 2014-2020 Fraunhofer FOKUS</sm:copyright>
        <sm:copyright>Copyright (c) 2014-2020 Freie Universitat Berlin</sm:copyright>
        <sm:copyright>Copyright (c) 2014-2020 Mayo Clinic</sm:copyright>
        <sm:copyright>Copyright (c) 2014-2020 Model Driven Solutions</sm:copyright>
        <sm:copyright>Copyright (c) 2014-2020 Thematix Partners LLC</sm:copyright>
        <sm:copyright>Copyright (c) 2015-2020 Object Management Group, Inc.</sm:copyright>
        <sm:copyright>Copyright (c) 2019-2020 Micro Focus</sm:copyright>
        <sm:dependsOn rdf:datatype="http://www.w3.org/2001/XMLSchema#anyURI">https://www.omg.org/spec/API4KP/api4kp/</sm:dependsOn>
        <sm:dependsOn rdf:datatype="http://www.w3.org/2001/XMLSchema#anyURI">https://www.omg.org/spec/LCC/</sm:dependsOn>
        <sm:fileAbbreviation>kao</sm:fileAbbreviation>
        <sm:filename>api4kp-kao.rdf</sm:filename>
        <rdfs:label>API4KP Knowledge Asset Type Ontology</rdfs:label>
    </owl:Ontology>
    


    <!-- 
    ///////////////////////////////////////////////////////////////////////////////////////
    //
    // Classes
    //
    ///////////////////////////////////////////////////////////////////////////////////////
     -->

    


    <!-- https://www.omg.org/spec/API4KP/api4kp-kao/AssessmentModel -->

    <owl:Class rdf:about="https://www.omg.org/spec/API4KP/api4kp-kao/AssessmentModel">
        <rdfs:subClassOf rdf:resource="https://www.omg.org/spec/API4KP/api4kp-kao/InferentialAsset"/>
        <rdfs:comment>knowledge that allows to infer an otherwise unknown or not directly observable state or situation</rdfs:comment>
        <rdfs:label>Assessment Model</rdfs:label>
    </owl:Class>
    


    <!-- https://www.omg.org/spec/API4KP/api4kp-kao/BusinessRuleAsset -->

    <owl:Class rdf:about="https://www.omg.org/spec/API4KP/api4kp-kao/BusinessRuleAsset">
        <rdfs:subClassOf rdf:resource="https://www.omg.org/spec/API4KP/api4kp-kao/CategorizedKnowledgeAsset"/>
        <rdfs:comment>Assets in this category describe or specify how to limit an agent&apos;s degree of freedom, to prevent undesirable behaviors, in favor of more desirable ones.</rdfs:comment>
        <rdfs:comment>At its essence, knowledge of this kind is expressed using &quot;IF..DO..&quot; rules, usually by means of constraint-oriented languages with ECA and/or deontic aspects</rdfs:comment>
        <rdfs:label>Rule-Oriented Knowledge Asset</rdfs:label>
        <skos:definition>Knowledge about the social, organizational and behavioral aspects of how business is (not) required, expected or permitted to be conducted, as determined by some party that has jurisdiction over an environment.</skos:definition>
        <skos:prefLabel>Rules, Policies and Guidelines</skos:prefLabel>
        <skos:scopeNote>Business rules are deontic in nature, whereas alethic rules are considered inferential models.</skos:scopeNote>
    </owl:Class>
    


    <!-- https://www.omg.org/spec/API4KP/api4kp-kao/CategorizedKnowledgeAsset -->

    <owl:Class rdf:about="https://www.omg.org/spec/API4KP/api4kp-kao/CategorizedKnowledgeAsset">
        <rdfs:subClassOf rdf:resource="https://www.omg.org/spec/API4KP/api4kp/KnowledgeAsset"/>
        <skos:definition>knowledge asset that is classified according to the logical and mathematical aspects that classify the concepts used in the asset</skos:definition>
        <skos:prefLabel>formally categorized knowledge asset</skos:prefLabel>
    </owl:Class>
    


    <!-- https://www.omg.org/spec/API4KP/api4kp-kao/CognitiveProcessModel -->

    <owl:Class rdf:about="https://www.omg.org/spec/API4KP/api4kp-kao/CognitiveProcessModel">
        <rdfs:subClassOf rdf:resource="https://www.omg.org/spec/API4KP/api4kp-kao/ProcessAsset"/>
        <rdfs:subClassOf>
            <owl:Restriction>
                <owl:onProperty rdf:resource="https://www.omg.org/spec/API4KP/api4kp/has-part"/>
                <owl:someValuesFrom rdf:resource="https://www.omg.org/spec/API4KP/api4kp-kao/DecisionModel"/>
            </owl:Restriction>
        </rdfs:subClassOf>
        <rdfs:comment>Knowledge Asset that captures how information is processed internally by an intelligent agent</rdfs:comment>
        <rdfs:label>Cognitive Process Model</rdfs:label>
    </owl:Class>
    


    <!-- https://www.omg.org/spec/API4KP/api4kp-kao/CohortDefinition -->

    <owl:Class rdf:about="https://www.omg.org/spec/API4KP/api4kp-kao/CohortDefinition">
        <rdfs:subClassOf rdf:resource="https://www.omg.org/spec/API4KP/api4kp-kao/InferentialAsset"/>
        <rdfs:comment>Definition used to classify persons into classes defined by some common characteristic</rdfs:comment>
        <rdfs:label>Cohort Definition</rdfs:label>
    </owl:Class>
    


    <!-- https://www.omg.org/spec/API4KP/api4kp-kao/ComponentKnowledgeAsset -->

    <owl:Class rdf:about="https://www.omg.org/spec/API4KP/api4kp-kao/ComponentKnowledgeAsset">
        <rdfs:subClassOf rdf:resource="https://www.omg.org/spec/API4KP/api4kp-kao/ExplicitRoleKnowledgeAsset"/>
        <rdfs:comment>a component asset is likely to play more specific roles based on its function and the type of the composite</rdfs:comment>
        <skos:definition>knowledge asset that is proper part of some other (composite) knowledge asset.</skos:definition>
        <skos:prefLabel>component knowledge asset</skos:prefLabel>
    </owl:Class>
    


    <!-- https://www.omg.org/spec/API4KP/api4kp-kao/CompositeKnowledgeAsset -->

    <owl:Class rdf:about="https://www.omg.org/spec/API4KP/api4kp-kao/CompositeKnowledgeAsset">
        <rdfs:subClassOf rdf:resource="https://www.omg.org/spec/API4KP/api4kp-kao/ExplicitRoleKnowledgeAsset"/>
        <rdfs:subClassOf rdf:resource="https://www.omg.org/spec/API4KP/api4kp/CompositeKnowledgeResource"/>
        <rdfs:comment>both composite and components are distinct individuals (i.e. with different IDs)</rdfs:comment>
        <skos:definition>knowledge asset that has other knowledge assets as proper parts</skos:definition>
        <skos:prefLabel>composite knowledge asset</skos:prefLabel>
    </owl:Class>
    


    <!-- https://www.omg.org/spec/API4KP/api4kp-kao/ComputableDecisionModel -->

    <owl:Class rdf:about="https://www.omg.org/spec/API4KP/api4kp-kao/ComputableDecisionModel">
        <rdfs:subClassOf rdf:resource="https://www.omg.org/spec/API4KP/api4kp-kao/DecisionModel"/>
        <rdfs:comment>Decision Model that includes an explicit specification of its decision making logic, suitable to be faithfully expressed in a computable language</rdfs:comment>
        <rdfs:label>Computable Decision Model</rdfs:label>
    </owl:Class>
    


    <!-- https://www.omg.org/spec/API4KP/api4kp-kao/ComputationalTechnique -->

    <owl:Class rdf:about="https://www.omg.org/spec/API4KP/api4kp-kao/ComputationalTechnique">
        <rdfs:subClassOf rdf:resource="https://www.omg.org/spec/API4KP/api4kp/KnowledgeProcessingTechnique"/>
        <owl:disjointWith rdf:resource="https://www.omg.org/spec/API4KP/api4kp-kao/NaturalisticTechnique"/>
        <rdfs:label>computational technique</rdfs:label>
        <skos:definition>Technique used in some knowledge processing task method specification that can be faithfully expressed in some machine-computable language</skos:definition>
    </owl:Class>
    


    <!-- https://www.omg.org/spec/API4KP/api4kp-kao/ConceptualModel -->

    <owl:Class rdf:about="https://www.omg.org/spec/API4KP/api4kp-kao/ConceptualModel">
        <rdfs:subClassOf rdf:resource="https://www.omg.org/spec/API4KP/api4kp-kao/SemanticAsset"/>
        <rdfs:comment>Abstraction of the structure and/or behavior of the entities in a given domain</rdfs:comment>
        <rdfs:label>Conceptual (Domain) Model</rdfs:label>
        <skos:altLabel>domain conceptualization</skos:altLabel>
    </owl:Class>
    


    <!-- https://www.omg.org/spec/API4KP/api4kp-kao/ContextualizabledKnowledge -->

    <owl:Class rdf:about="https://www.omg.org/spec/API4KP/api4kp-kao/ContextualizabledKnowledge">
        <rdfs:subClassOf rdf:resource="https://www.omg.org/spec/API4KP/api4kp-kao/ConceptualModel"/>
        <rdfs:comment>Conceptual Work of Knowledge that has been adapted for a given context</rdfs:comment>
        <rdfs:label>Contextualizable Knowledge</rdfs:label>
    </owl:Class>
    


    <!-- https://www.omg.org/spec/API4KP/api4kp-kao/DecisionMakingTask -->

    <owl:Class rdf:about="https://www.omg.org/spec/API4KP/api4kp-kao/DecisionMakingTask">
        <rdfs:subClassOf rdf:resource="https://www.omg.org/spec/API4KP/api4kp/InformationProcessingTask"/>
        <rdfs:label>decision making task</rdfs:label>
    </owl:Class>
    


    <!-- https://www.omg.org/spec/API4KP/api4kp-kao/DecisionModel -->

    <owl:Class rdf:about="https://www.omg.org/spec/API4KP/api4kp-kao/DecisionModel">
        <rdfs:subClassOf rdf:resource="https://www.omg.org/spec/API4KP/api4kp-kao/AssessmentModel"/>
        <rdfs:comment>Assessment that can be abstracted by means of a question, which requires to select one out of a set of admissible options</rdfs:comment>
        <rdfs:label>Decision Model</rdfs:label>
    </owl:Class>
    


    <!-- https://www.omg.org/spec/API4KP/api4kp-kao/DecisionTaskModel -->

    <owl:Class rdf:about="https://www.omg.org/spec/API4KP/api4kp-kao/DecisionTaskModel">
        <rdfs:subClassOf rdf:resource="https://www.omg.org/spec/API4KP/api4kp-kao/CognitiveProcessModel"/>
        <rdfs:subClassOf>
            <owl:Restriction>
                <owl:onProperty rdf:resource="https://www.omg.org/spec/API4KP/api4kp/defines"/>
                <owl:someValuesFrom rdf:resource="https://www.omg.org/spec/API4KP/api4kp-kao/DecisionMakingTask"/>
            </owl:Restriction>
        </rdfs:subClassOf>
        <rdfs:subClassOf>
            <owl:Restriction>
                <owl:onProperty rdf:resource="https://www.omg.org/spec/API4KP/api4kp/part-of"/>
                <owl:someValuesFrom rdf:resource="https://www.omg.org/spec/API4KP/api4kp-kao/CognitiveProcessModel"/>
            </owl:Restriction>
        </rdfs:subClassOf>
        <rdfs:comment>Model of who, when, where and why a Decision is made, usually as part of a broader process. Also known as Decision Making Process Model, usually includes a Decision Model that specifies how to actually choose the optimal option</rdfs:comment>
        <rdfs:label>Decision Task Model</rdfs:label>
    </owl:Class>
    


    <!-- https://www.omg.org/spec/API4KP/api4kp-kao/DocumentationTemplate -->

    <owl:Class rdf:about="https://www.omg.org/spec/API4KP/api4kp-kao/DocumentationTemplate">
        <rdfs:subClassOf rdf:resource="https://www.omg.org/spec/API4KP/api4kp-kao/InformationAsset"/>
        <rdfs:comment>An organized collection of determinable concepts, possibly associated to questions, which are meant to be resolved in a particular context</rdfs:comment>
        <rdfs:label>Documentation Template</rdfs:label>
        <skos:scopeNote>more general than questionnaires, whose questions are meant to be answered by a human agent (possibly with computer aid), documentation templates can be used  by software agents as well</skos:scopeNote>
    </owl:Class>
    


    <!-- https://www.omg.org/spec/API4KP/api4kp-kao/Equation -->

    <owl:Class rdf:about="https://www.omg.org/spec/API4KP/api4kp-kao/Equation">
        <rdfs:subClassOf rdf:resource="https://www.omg.org/spec/API4KP/api4kp-kao/FunctionalExpression"/>
        <rdfs:comment>A functional expression, defined in terms of two functional expressions connected by means of the well known equality operator.</rdfs:comment>
        <rdfs:label>Equation</rdfs:label>
    </owl:Class>
    


    <!-- https://www.omg.org/spec/API4KP/api4kp-kao/ExplicitRoleKnowledgeAsset -->

    <owl:Class rdf:about="https://www.omg.org/spec/API4KP/api4kp-kao/ExplicitRoleKnowledgeAsset">
        <rdfs:subClassOf rdf:resource="https://www.omg.org/spec/API4KP/api4kp/KnowledgeAsset"/>
        <skos:definition>knowledge asset that is categorized in terms of its relationship(s) to one or more different knowledge assets</skos:definition>
        <skos:prefLabel>knowledge asset with explicit role</skos:prefLabel>
    </owl:Class>
    


    <!-- https://www.omg.org/spec/API4KP/api4kp-kao/FactualKnowledge -->

    <owl:Class rdf:about="https://www.omg.org/spec/API4KP/api4kp-kao/FactualKnowledge">
        <rdfs:subClassOf rdf:resource="https://www.omg.org/spec/API4KP/api4kp-kao/ConceptualModel"/>
        <rdfs:comment>Facts are suitable to be asserted</rdfs:comment>
        <rdfs:comment>Knowledge that is held to be a faithful conceptualization of the state of affairs in a given domain by all agents that share (and understand) it.</rdfs:comment>
        <rdfs:label>Factual Knowledge</rdfs:label>
    </owl:Class>
    


    <!-- https://www.omg.org/spec/API4KP/api4kp-kao/FormalOntology -->

    <owl:Class rdf:about="https://www.omg.org/spec/API4KP/api4kp-kao/FormalOntology">
        <rdfs:subClassOf rdf:resource="https://www.omg.org/spec/API4KP/api4kp-kao/ConceptualModel"/>
        <rdfs:comment>conceptual model that is based on formal principles, such as that allow to make inferences and/or verify the consistency of the model</rdfs:comment>
        <rdfs:label>Formal Ontology</rdfs:label>
    </owl:Class>
    


    <!-- https://www.omg.org/spec/API4KP/api4kp-kao/FunctionalExpression -->

    <owl:Class rdf:about="https://www.omg.org/spec/API4KP/api4kp-kao/FunctionalExpression">
        <rdfs:subClassOf rdf:resource="https://www.omg.org/spec/API4KP/api4kp-kao/AssessmentModel"/>
        <rdfs:comment>Knowledge about the application of well-known information processing methods, possibly chained together, which are stateless, functional and idempotent in nature.</rdfs:comment>
        <rdfs:label>Functional Expression</rdfs:label>
        <skos:example>&apos;mass&apos; times the square of the speed of light</skos:example>
    </owl:Class>
    


    <!-- https://www.omg.org/spec/API4KP/api4kp-kao/InferentialAsset -->

    <owl:Class rdf:about="https://www.omg.org/spec/API4KP/api4kp-kao/InferentialAsset">
        <rdfs:subClassOf rdf:resource="https://www.omg.org/spec/API4KP/api4kp-kao/CategorizedKnowledgeAsset"/>
        <rdfs:subClassOf rdf:resource="https://www.omg.org/spec/API4KP/api4kp/Definition"/>
        <rdfs:comment>an agent can use inferential knowledge to assess the current, or predict the future state of a variable, quality or other characteristic of a system (e.g. a patient) which may not be directly observable, but can be estimated on the basis of other more primitive pieces of data.</rdfs:comment>
        <rdfs:comment>reasoning driven by inferential assets is functional, stateless and idempotent: inferential assets are better expressed using expression languages, mathematical/statistical languages, or (sub-languages of) logic languages that focus on logical implications.</rdfs:comment>
        <rdfs:label xml:lang="en">inference-oriented knowledge asset</rdfs:label>
        <skos:definition>knowledge asset that uses some inferential aspects, and only inferential, descriptive and uncertainty-related assets.</skos:definition>
        <skos:example>A BMI Calculator</skos:example>
        <skos:example xml:lang="en">A FRAX Fracture Risk Score Calculator</skos:example>
        <skos:example xml:lang="en">A Pain assessment scale</skos:example>
        <skos:example xml:lang="en">The Cockcroft-Gault equation</skos:example>
        <skos:example xml:lang="en">The Scoring Model used to calculate the CHA2DS2-VASc score</skos:example>
        <skos:prefLabel xml:lang="en">assessment, predictive and inferential models</skos:prefLabel>
        <skos:scopeNote xml:lang="en">TODO: move to CKAO

This is a broad category that includes e.g.: 
a) Mathematical equations and models used in a clinical or health-related calculation
b) Clinical or health-related scoring formulas for the purposes of predicting or classifying something, often by assigning points based on observations (e.g. stroke risk, asthma severity, mortality); includes information about the required inputs and the interpretation of the resulting score/s  
c) Associations, Correlations and Causal Relationships between phenomena, some of which may not be directly observable</skos:scopeNote>
        <skos:scopeNote>includes both logical (qualitative) and statistical (quantitative) inference.</skos:scopeNote>
        <skos:scopeNote>inferential assets may depend on semantic knowledge assets as background knowledge, and be a dependency/component of rule, process and measure assets.</skos:scopeNote>
    </owl:Class>
    


    <!-- https://www.omg.org/spec/API4KP/api4kp-kao/InformationAsset -->

    <owl:Class rdf:about="https://www.omg.org/spec/API4KP/api4kp-kao/InformationAsset">
        <rdfs:subClassOf rdf:resource="https://www.omg.org/spec/API4KP/api4kp-kao/CategorizedKnowledgeAsset"/>
        <rdfs:label>Information-Oriented Knowledge Asset</rdfs:label>
        <skos:definition>Knowledge about how to acquire, represent, organize, store and distribute data, about some domain of interest, using structured formats.</skos:definition>
        <skos:example>A logical information model for the documentation of a Blood Pressure test panel, such that it could be expressed by means of a CIMI model</skos:example>
        <skos:example>A pediatric documentation template, such that it could be manifested in a digital, interactive, form-based data acquisition tool</skos:example>
        <skos:prefLabel>Structured Information and Data Capture Models</skos:prefLabel>
        <skos:scopeNote>Notice that conceptual models of the domain, as opposed to logical models of information about the domain, are categorized under &quot;Terminology, Ontology and Assertional KBs&quot;.</skos:scopeNote>
        <skos:scopeNote>This category includes assets whose manifestations are meant to be used during the entire lifecycle, including documentation templates and questionnaires (acquisition), as well as logical information models and schemas (storage) and messaging models used for data sharing and interoperability.</skos:scopeNote>
    </owl:Class>
    <owl:Axiom>
        <owl:annotatedSource rdf:resource="https://www.omg.org/spec/API4KP/api4kp-kao/InformationAsset"/>
        <owl:annotatedProperty rdf:resource="http://www.w3.org/2004/02/skos/core#example"/>
        <owl:annotatedTarget>A logical information model for the documentation of a Blood Pressure test panel, such that it could be expressed by means of a CIMI model</owl:annotatedTarget>
        <rdfs:seeAlso rdf:resource="http://www.clinicalelement.com/cimi-browser/#/20180124/CIMI/CIMI-CORE-CompoundClinicalStatement.blood_pressure_panel.v1.0.0"/>
    </owl:Axiom>
    <owl:Axiom>
        <owl:annotatedSource rdf:resource="https://www.omg.org/spec/API4KP/api4kp-kao/InformationAsset"/>
        <owl:annotatedProperty rdf:resource="http://www.w3.org/2004/02/skos/core#example"/>
        <owl:annotatedTarget>A pediatric documentation template, such that it could be manifested in a digital, interactive, form-based data acquisition tool</owl:annotatedTarget>
        <rdfs:seeAlso>https://healthit.ahrq.gov/health-it-tools-and-resources/pediatric-resources/pediatric-documentation-templates/pediatric-asthma-template</rdfs:seeAlso>
    </owl:Axiom>
    


    <!-- https://www.omg.org/spec/API4KP/api4kp-kao/InformationModel -->

    <owl:Class rdf:about="https://www.omg.org/spec/API4KP/api4kp-kao/InformationModel">
        <rdfs:subClassOf rdf:resource="https://www.omg.org/spec/API4KP/api4kp-kao/InformationAsset"/>
        <rdfs:comment>(Meta) model that defines which information should be captured about some kind of domain</rdfs:comment>
        <rdfs:label>Information Model</rdfs:label>
        <skos:altLabel>logical data model</skos:altLabel>
    </owl:Class>
    


    <!-- https://www.omg.org/spec/API4KP/api4kp-kao/InquirySpecification -->

    <owl:Class rdf:about="https://www.omg.org/spec/API4KP/api4kp-kao/InquirySpecification">
        <rdfs:subClassOf rdf:resource="https://www.omg.org/spec/API4KP/api4kp-kao/ProcessAsset"/>
        <rdfs:comment>The definition of how (and possibly when and where) to ask a question, following some kind of protocol, for the purpose of receiving a specific answer, with the goal of gaining information in the process</rdfs:comment>
        <rdfs:label>Inquiry Specification</rdfs:label>
    </owl:Class>
    


    <!-- https://www.omg.org/spec/API4KP/api4kp-kao/InteractiveTechnique -->

    <owl:Class rdf:about="https://www.omg.org/spec/API4KP/api4kp-kao/InteractiveTechnique">
        <rdfs:subClassOf rdf:resource="https://www.omg.org/spec/API4KP/api4kp/KnowledgeProcessingTechnique"/>
        <rdfs:subClassOf>
            <owl:Restriction>
                <owl:onProperty rdf:resource="https://www.omg.org/spec/API4KP/api4kp/has-part"/>
                <owl:someValuesFrom rdf:resource="https://www.omg.org/spec/API4KP/api4kp-kao/ComputationalTechnique"/>
            </owl:Restriction>
        </rdfs:subClassOf>
        <rdfs:subClassOf>
            <owl:Restriction>
                <owl:onProperty rdf:resource="https://www.omg.org/spec/API4KP/api4kp/has-part"/>
                <owl:someValuesFrom rdf:resource="https://www.omg.org/spec/API4KP/api4kp-kao/NaturalisticTechnique"/>
            </owl:Restriction>
        </rdfs:subClassOf>
        <rdfs:label>HCI interactive technique</rdfs:label>
        <skos:definition>Technique that is based on the interaction of a Human and a Computer, in the context of a task where at least one of each participates as an agent</skos:definition>
    </owl:Class>
    


    <!-- https://www.omg.org/spec/API4KP/api4kp-kao/LogicBasedTechnique -->

    <owl:Class rdf:about="https://www.omg.org/spec/API4KP/api4kp-kao/LogicBasedTechnique">
        <rdfs:subClassOf rdf:resource="https://www.omg.org/spec/API4KP/api4kp-kao/QualitativeTechnique"/>
        <rdfs:comment>Technique based on formal logic</rdfs:comment>
        <rdfs:label>logic based technique</rdfs:label>
    </owl:Class>
    


    <!-- https://www.omg.org/spec/API4KP/api4kp-kao/MetricAsset -->

    <owl:Class rdf:about="https://www.omg.org/spec/API4KP/api4kp-kao/MetricAsset">
        <rdfs:subClassOf rdf:resource="https://www.omg.org/spec/API4KP/api4kp-kao/CategorizedKnowledgeAsset"/>
        <rdfs:comment>Knowledge of this kind usually builds directly on Assessment Models (for the quantification) and Process Models (to relate the measures to the processes and their goals).</rdfs:comment>
        <rdfs:label>Metric-Oriented Knowledge Asset</rdfs:label>
        <rdfs:seeAlso rdf:resource="https://www.cms.gov/Medicare/Quality-Initiatives-Patient-Assessment-Instruments/QualityMeasures/index.html"/>
        <skos:definition>Knowledge that pertains to how certain features (qualitative and/or quantitative) of a system can be observed, quantified, aggregated, compared to a baseline and objective values and ultimately used to evaluate the performance of (parts of) that system and its processes</skos:definition>
        <skos:prefLabel>KPIs, Measurements and Metrics</skos:prefLabel>
    </owl:Class>
    


    <!-- https://www.omg.org/spec/API4KP/api4kp-kao/MultiAgentDecisionTaskModel -->

    <owl:Class rdf:about="https://www.omg.org/spec/API4KP/api4kp-kao/MultiAgentDecisionTaskModel">
        <rdfs:subClassOf rdf:resource="https://www.omg.org/spec/API4KP/api4kp-kao/DecisionTaskModel"/>
        <rdfs:comment>Decision Task Model that requires the participation of two or more agents</rdfs:comment>
        <rdfs:label>Multi-Agent Decision Task Model</rdfs:label>
    </owl:Class>
    


    <!-- https://www.omg.org/spec/API4KP/api4kp-kao/NLPTechnique -->

    <owl:Class rdf:about="https://www.omg.org/spec/API4KP/api4kp-kao/NLPTechnique">
        <rdfs:subClassOf rdf:resource="https://www.omg.org/spec/API4KP/api4kp-kao/ComputationalTechnique"/>
        <rdfs:label>natural language processing technique</rdfs:label>
        <skos:definition>Computational Technique based on computations applied to expressions in natural language</skos:definition>
    </owl:Class>
    


    <!-- https://www.omg.org/spec/API4KP/api4kp-kao/NaturalisticTechnique -->

    <owl:Class rdf:about="https://www.omg.org/spec/API4KP/api4kp-kao/NaturalisticTechnique">
        <rdfs:subClassOf rdf:resource="https://www.omg.org/spec/API4KP/api4kp/KnowledgeProcessingTechnique"/>
        <rdfs:comment>I.e. technique such that a computer would not be able to apply it, and achieve the goal of a task executed (following a method) using this technique</rdfs:comment>
        <rdfs:label>naturalistic technique</rdfs:label>
        <skos:definition>Technique that requires a human agent to be leveraged to full effectiveness</skos:definition>
    </owl:Class>
    


    <!-- https://www.omg.org/spec/API4KP/api4kp-kao/OperationalConceptDefinition -->

    <owl:Class rdf:about="https://www.omg.org/spec/API4KP/api4kp-kao/OperationalConceptDefinition">
        <rdfs:subClassOf rdf:resource="https://www.omg.org/spec/API4KP/api4kp-kao/ExplicitRoleKnowledgeAsset"/>
        <rdfs:subClassOf rdf:resource="https://www.omg.org/spec/API4KP/api4kp/ConstructiveDefinition"/>
        <rdfs:subClassOf rdf:resource="https://www.omg.org/spec/API4KP/api4kp/KnowledgeProcessingMethodSpecification"/>
        <rdfs:subClassOf>
            <owl:Restriction>
                <owl:onProperty rdf:resource="https://www.omg.org/spec/API4KP/api4kp/defines"/>
                <owl:someValuesFrom rdf:resource="https://www.omg.org/spec/API4KP/api4kp/ResolvableConcept"/>
            </owl:Restriction>
        </rdfs:subClassOf>
        <rdfs:comment>TODO: move to definition
some definitions have conditional applicability, i.e. they are associated to some constraint whose satisfaction is directly correlated to the confidence in the results of the application of the definition</rdfs:comment>
        <skos:definition>constructive definition of a (resolvable) Concept that specifies how to resolve that Concept in some context, i.e. a specification of if and how to prove that the concept applies to the context, abstracting it.</skos:definition>
        <skos:prefLabel>operational concept definition</skos:prefLabel>
    </owl:Class>
    


    <!-- https://www.omg.org/spec/API4KP/api4kp-kao/PredictiveModel -->

    <owl:Class rdf:about="https://www.omg.org/spec/API4KP/api4kp-kao/PredictiveModel">
        <rdfs:subClassOf rdf:resource="https://www.omg.org/spec/API4KP/api4kp-kao/AssessmentModel"/>
        <rdfs:comment>assessment of some state that is unobservable due to being in the future</rdfs:comment>
        <rdfs:label>Predictive Model</rdfs:label>
    </owl:Class>
    


    <!-- https://www.omg.org/spec/API4KP/api4kp-kao/ProcessAsset -->

    <owl:Class rdf:about="https://www.omg.org/spec/API4KP/api4kp-kao/ProcessAsset">
        <rdfs:subClassOf rdf:resource="https://www.omg.org/spec/API4KP/api4kp-kao/CategorizedKnowledgeAsset"/>
        <rdfs:comment>Specifications can be imperative (define what to do) or adaptive (define what not to do), depending on how many degrees of freedom are left to an agent</rdfs:comment>
        <rdfs:comment>The knowledge pertains specifically to the orchestration of the activities in relation to the goals, but usually relies on more ontologic, foundational definitions of the tasks to be performed as part of the process (as well as their related participants, roles, resources, etc.)</rdfs:comment>
        <rdfs:label>Process-Oriented Knowledge Asset</rdfs:label>
        <skos:definition>Knowledge about how to perform (complex) activities, properly orchestrated over time, so to achieve certain objectives and goals</skos:definition>
        <skos:prefLabel>Plans, Processes, Pathways and Protocol Definitions</skos:prefLabel>
        <skos:scopeNote>Does not cover &apos;natural&apos; processes that do not occur as a consequence of an agent&apos;s explicit intentions</skos:scopeNote>
    </owl:Class>
    


    <!-- https://www.omg.org/spec/API4KP/api4kp-kao/Protocol -->

    <owl:Class rdf:about="https://www.omg.org/spec/API4KP/api4kp-kao/Protocol">
        <rdfs:subClassOf rdf:resource="https://www.omg.org/spec/API4KP/api4kp-kao/ProcessAsset"/>
        <rdfs:comment>A shared, endorsed, justified, imperative specification of the expected behavior of one or more agents in a specific situation</rdfs:comment>
        <rdfs:label>Protocol</rdfs:label>
    </owl:Class>
    


    <!-- https://www.omg.org/spec/API4KP/api4kp-kao/QualitativeTechnique -->

    <owl:Class rdf:about="https://www.omg.org/spec/API4KP/api4kp-kao/QualitativeTechnique">
        <rdfs:subClassOf rdf:resource="https://www.omg.org/spec/API4KP/api4kp-kao/ComputationalTechnique"/>
        <rdfs:label>qualitative computational technique</rdfs:label>
        <skos:altLabel>Symbolic Technique</skos:altLabel>
        <skos:definition>Computational Technique based on symbolic and/or logic-based principles</skos:definition>
    </owl:Class>
    


    <!-- https://www.omg.org/spec/API4KP/api4kp-kao/QuantitativeTechnique -->

    <owl:Class rdf:about="https://www.omg.org/spec/API4KP/api4kp-kao/QuantitativeTechnique">
        <rdfs:subClassOf rdf:resource="https://www.omg.org/spec/API4KP/api4kp-kao/ComputationalTechnique"/>
        <rdfs:label>quantitative computational technique</rdfs:label>
        <skos:altLabel>Subsymbolic Technique</skos:altLabel>
        <skos:definition>Computational Technique that is based on mathematical, statistical and/or numerical principles</skos:definition>
    </owl:Class>
    


    <!-- https://www.omg.org/spec/API4KP/api4kp-kao/QueryTechnique -->

    <owl:Class rdf:about="https://www.omg.org/spec/API4KP/api4kp-kao/QueryTechnique">
        <rdfs:subClassOf rdf:resource="https://www.omg.org/spec/API4KP/api4kp/KnowledgeProcessingTechnique"/>
        <rdfs:label>query based technique</rdfs:label>
        <skos:definition>Technique that involves requesting another agent to actually perform the task, from which the products can be obtained</skos:definition>
    </owl:Class>
    


    <!-- https://www.omg.org/spec/API4KP/api4kp-kao/Questionnaire -->

    <owl:Class rdf:about="https://www.omg.org/spec/API4KP/api4kp-kao/Questionnaire">
        <rdfs:subClassOf rdf:resource="https://www.omg.org/spec/API4KP/api4kp-kao/DocumentationTemplate"/>
        <rdfs:comment xml:lang="en">An organized collection of questions intended to solicit information from patients, providers or other individuals in the healthcare domain</rdfs:comment>
        <rdfs:label xml:lang="en">Questionnaire</rdfs:label>
        <skos:example xml:lang="en">First Visit Questionnaire</skos:example>
        <skos:prefLabel xml:lang="en">Questionnaire</skos:prefLabel>
    </owl:Class>
    <owl:Axiom>
        <owl:annotatedSource rdf:resource="https://www.omg.org/spec/API4KP/api4kp-kao/Questionnaire"/>
        <owl:annotatedProperty rdf:resource="http://www.w3.org/2004/02/skos/core#example"/>
        <owl:annotatedTarget xml:lang="en">First Visit Questionnaire</owl:annotatedTarget>
        <rdfs:seeAlso rdf:resource="http://mayoweb.mayo.edu/sp-forms/mc20600-mc20699/mchs20617.pdf"/>
    </owl:Axiom>
    


    <!-- https://www.omg.org/spec/API4KP/api4kp-kao/SemanticAsset -->

    <owl:Class rdf:about="https://www.omg.org/spec/API4KP/api4kp-kao/SemanticAsset">
        <rdfs:subClassOf rdf:resource="https://www.omg.org/spec/API4KP/api4kp-kao/CategorizedKnowledgeAsset"/>
        <rdfs:comment>Assets in this category can be classified along the semantic spectrum</rdfs:comment>
        <rdfs:comment>Knowledge of this kind is usually structural, universal, and expressed using declarative languages</rdfs:comment>
        <rdfs:label>Semantic-Oriented Knowledge Asset</rdfs:label>
        <rdfs:seeAlso rdf:datatype="http://www.w3.org/2001/XMLSchema#anyURI">http://slidegur.com/doc/5719791/presentation</rdfs:seeAlso>
        <skos:definition>Foundational Knowledge about (Clinical) Concepts, their definitions and mutual relationships, together with their linguistic and syntactic expressions.</skos:definition>
        <skos:example rdf:datatype="http://www.w3.org/2001/XMLSchema#anyURI">A Drug/Drug interaction Assertional KB</skos:example>
        <skos:example>The Mayo Clinic Asthma Value Set</skos:example>
        <skos:example>The Ontology of Knowledge Assets, of which this OWL-based representation is an expression</skos:example>
        <skos:prefLabel>Terminology, Ontology and Assertional KBs</skos:prefLabel>
    </owl:Class>
    <owl:Axiom>
        <owl:annotatedSource rdf:resource="https://www.omg.org/spec/API4KP/api4kp-kao/SemanticAsset"/>
        <owl:annotatedProperty rdf:resource="http://www.w3.org/2004/02/skos/core#example"/>
        <owl:annotatedTarget>The Mayo Clinic Asthma Value Set</owl:annotatedTarget>
        <rdfs:seeAlso rdf:resource="http://ckm.ontology.mayo.edu/ontology/%5C%5Cmfad.mfroot.org%5Crchdept%5CTerms%5CTerminology%20Web%5C2_ValueSets%5CMCBT_ClinicalProblemAsthma.pdf"/>
    </owl:Axiom>
    


    <!-- https://www.omg.org/spec/API4KP/api4kp-kao/SemanticDecisionModel -->

    <owl:Class rdf:about="https://www.omg.org/spec/API4KP/api4kp-kao/SemanticDecisionModel">
        <rdfs:subClassOf rdf:resource="https://www.omg.org/spec/API4KP/api4kp-kao/DecisionModel"/>
        <rdfs:comment>Decision Model that includes an unambiguous definition of every concept involved</rdfs:comment>
        <rdfs:label>Semantic Decision Model</rdfs:label>
    </owl:Class>
    


    <!-- https://www.omg.org/spec/API4KP/api4kp-kao/SemanticInformationModel -->

    <owl:Class rdf:about="https://www.omg.org/spec/API4KP/api4kp-kao/SemanticInformationModel">
        <rdfs:subClassOf rdf:resource="https://www.omg.org/spec/API4KP/api4kp-kao/InformationModel"/>
        <rdfs:subClassOf>
            <owl:Restriction>
                <owl:onProperty rdf:resource="https://www.omg.org/spec/API4KP/api4kp/has-part"/>
                <owl:someValuesFrom rdf:resource="https://www.omg.org/spec/API4KP/api4kp-kao/SemanticInformationModel"/>
            </owl:Restriction>
        </rdfs:subClassOf>
        <rdfs:comment>Information Model designed such that instances have one and only one interpretation</rdfs:comment>
        <rdfs:label>Semantic Information Model</rdfs:label>
    </owl:Class>
    


    <!-- https://www.omg.org/spec/API4KP/api4kp-kao/ServiceBasedTechnique -->

    <owl:Class rdf:about="https://www.omg.org/spec/API4KP/api4kp-kao/ServiceBasedTechnique">
        <rdfs:subClassOf rdf:resource="https://www.omg.org/spec/API4KP/api4kp/KnowledgeProcessingTechnique"/>
        <rdfs:comment>Technique based on delegation to another entity</rdfs:comment>
        <rdfs:label>service based technique</rdfs:label>
    </owl:Class>
    


    <!-- https://www.omg.org/spec/API4KP/api4kp-kao/ServiceDescription -->

    <owl:Class rdf:about="https://www.omg.org/spec/API4KP/api4kp-kao/ServiceDescription">
        <rdfs:subClassOf rdf:resource="https://www.omg.org/spec/API4KP/api4kp-kao/ProcessAsset"/>
        <rdfs:label>Service Description</rdfs:label>
    </owl:Class>
    


    <!-- https://www.omg.org/spec/API4KP/api4kp-kao/ServiceProfile -->

    <owl:Class rdf:about="https://www.omg.org/spec/API4KP/api4kp-kao/ServiceProfile">
        <rdfs:subClassOf rdf:resource="https://www.omg.org/spec/API4KP/api4kp-kao/ServiceDescription"/>
        <rdfs:comment>Service Description that refines (by constraint), and thus depends on, some Service Description</rdfs:comment>
        <rdfs:label>Service Profile</rdfs:label>
    </owl:Class>
    


    <!-- https://www.omg.org/spec/API4KP/api4kp-kao/ValueSet -->

    <owl:Class rdf:about="https://www.omg.org/spec/API4KP/api4kp-kao/ValueSet">
        <rdfs:subClassOf rdf:resource="https://www.omg.org/spec/API4KP/api4kp-kao/SemanticAsset"/>
        <rdfs:comment xml:lang="en">A set of pairs of &quot;codes&quot;, drawn from one or more code systems, and human-readable terms that represent clinical concepts (e.g. &quot;diabetes type II&quot;)</rdfs:comment>
        <rdfs:label xml:lang="en">Value Set</rdfs:label>
        <skos:example xml:lang="en">The Asthma Value Set</skos:example>
        <skos:prefLabel xml:lang="en">Value Set</skos:prefLabel>
    </owl:Class>
    <owl:Axiom>
        <owl:annotatedSource rdf:resource="https://www.omg.org/spec/API4KP/api4kp-kao/ValueSet"/>
        <owl:annotatedProperty rdf:resource="http://www.w3.org/2004/02/skos/core#example"/>
        <owl:annotatedTarget xml:lang="en">The Asthma Value Set</owl:annotatedTarget>
        <rdfs:seeAlso rdf:resource="http://ckm.ontology.mayo.edu/ontology/%5C%5Cmfad.mfroot.org%5Crchdept%5CTerms%5CTerminology%20Web%5C2_ValueSets%5CMCBT_ClinicalProblemAsthma.pdf"/>
    </owl:Axiom>
    


    <!-- https://www.omg.org/spec/API4KP/api4kp/Grammar -->

    <owl:Class rdf:about="https://www.omg.org/spec/API4KP/api4kp/Grammar">
        <rdfs:subClassOf rdf:resource="https://www.omg.org/spec/API4KP/api4kp-kao/InformationAsset"/>
    </owl:Class>
    


    <!-- https://www.omg.org/spec/API4KP/api4kp/Lexicon -->

    <owl:Class rdf:about="https://www.omg.org/spec/API4KP/api4kp/Lexicon">
        <rdfs:subClassOf rdf:resource="https://www.omg.org/spec/API4KP/api4kp-kao/SemanticAsset"/>
    </owl:Class>
</rdf:RDF>



<!-- Generated by the OWL API (version 4.5.9.2019-02-01T07:24:44Z) https://github.com/owlcs/owlapi -->

