<?xml version="1.0" encoding="UTF-8"?>
<!DOCTYPE rdf:RDF [
	<!ENTITY AnnotationVocabulary "https://www.omg.org/spec/EDMC-FIBO/FND/Utilities/AnnotationVocabulary/">
	<!ENTITY AnnotationVocabulary1 "http://www.omg.org/spec/EDMC-FIBO/FND/Utilities/AnnotationVocabulary/">
	<!ENTITY api4kp "https://www.omg.org/spec/API4KP/api4kp/">
	<!ENTITY api4kp-krr "https://www.omg.org/spec/API4KP/api4kp-krr/">
	<!ENTITY dct "http://purl.org/dc/terms/">
	<!ENTITY dol "http://www.omg.org/spec/DOL/DOL-terms/">
	<!ENTITY lcc-lr "https://www.omg.org/spec/LCC/Languages/LanguageRepresentation/">
	<!ENTITY owl "http://www.w3.org/2002/07/owl#">
	<!ENTITY rdf "http://www.w3.org/1999/02/22-rdf-syntax-ns#">
	<!ENTITY rdfs "http://www.w3.org/2000/01/rdf-schema#">
	<!ENTITY skos "http://www.w3.org/2004/02/skos/core#">
	<!ENTITY sm "http://www.omg.org/techprocess/ab/SpecificationMetadata/">
	<!ENTITY xsd "http://www.w3.org/2001/XMLSchema#">
]>
<rdf:RDF xml:base="https://www.omg.org/spec/API4KP/api4kp-krr/"
	xmlns="https://www.omg.org/spec/API4KP/api4kp-krr/"
	xmlns:AnnotationVocabulary="https://www.omg.org/spec/EDMC-FIBO/FND/Utilities/AnnotationVocabulary/"
	xmlns:AnnotationVocabulary1="http://www.omg.org/spec/EDMC-FIBO/FND/Utilities/AnnotationVocabulary/"
	xmlns:api4kp="https://www.omg.org/spec/API4KP/api4kp/"
	xmlns:api4kp-krr="https://www.omg.org/spec/API4KP/api4kp-krr/"
	xmlns:dct="http://purl.org/dc/terms/"
	xmlns:dol="http://www.omg.org/spec/DOL/DOL-terms/"
	xmlns:lcc-lr="https://www.omg.org/spec/LCC/Languages/LanguageRepresentation/"
	xmlns:owl="http://www.w3.org/2002/07/owl#"
	xmlns:rdf="http://www.w3.org/1999/02/22-rdf-syntax-ns#"
	xmlns:rdfs="http://www.w3.org/2000/01/rdf-schema#"
	xmlns:skos="http://www.w3.org/2004/02/skos/core#"
	xmlns:sm="http://www.omg.org/techprocess/ab/SpecificationMetadata/"
	xmlns:xsd="http://www.w3.org/2001/XMLSchema#">
	
	<owl:Ontology rdf:about="https://www.omg.org/spec/API4KP/api4kp-krr/">
		<rdfs:label>API4KP Knowledge Representation and Reasoning Terminology Ontology</rdfs:label>
		<dct:abstract>This ontology covers the primary knowledge representation and reasoning (KRR) terminology used for describing the concepts used by the API4KP specification.</dct:abstract>
		<dct:creator xml:lang="mayo.edu)">Davide Sottara (sottara.davide</dct:creator>
		<dct:license rdf:datatype="&xsd;anyURI">http://opensource.org/licenses/MIT</dct:license>
		<sm:contentLanguage rdf:datatype="&xsd;anyURI">http://www.w3.org/standards/techs/owl#w3c_all</sm:contentLanguage>
		<sm:copyright>Copyright (c) 2014-2020 88 Solutions</sm:copyright>
		<sm:copyright>Copyright (c) 2014-2020 Adaptive</sm:copyright>
		<sm:copyright>Copyright (c) 2014-2020 Arizona State University</sm:copyright>
		<sm:copyright>Copyright (c) 2014-2020 Athan Services</sm:copyright>
		<sm:copyright>Copyright (c) 2014-2020 Fraunhofer FOKUS</sm:copyright>
		<sm:copyright>Copyright (c) 2014-2020 Freie Universitat Berlin</sm:copyright>
		<sm:copyright>Copyright (c) 2014-2020 Mayo Clinic</sm:copyright>
		<sm:copyright>Copyright (c) 2014-2020 Model Driven Solutions</sm:copyright>
		<sm:copyright>Copyright (c) 2014-2020 Thematix Partners LLC</sm:copyright>
		<sm:copyright>Copyright (c) 2015-2020 Object Management Group, Inc.</sm:copyright>
		<sm:copyright>Copyright (c) 2019-2020 Micro Focus</sm:copyright>
		<sm:dependsOn rdf:datatype="&xsd;anyURI">https://www.omg.org/spec/API4KP/api4kp/</sm:dependsOn>
		<sm:dependsOn rdf:datatype="&xsd;anyURI">https://www.omg.org/spec/DOL/</sm:dependsOn>
		<sm:dependsOn rdf:datatype="&xsd;anyURI">https://www.omg.org/spec/LCC/</sm:dependsOn>
		<sm:fileAbbreviation>krr</sm:fileAbbreviation>
		<sm:filename>api4kp-krr.rdf</sm:filename>
		<owl:imports rdf:resource="http://www.omg.org/spec/DOL/DOL-terms/"/>
		<owl:imports rdf:resource="http://www.omg.org/techprocess/ab/SpecificationMetadata/"/>
		<owl:imports rdf:resource="https://www.omg.org/spec/API4KP/SNAPSHOT/api4kp-lang/"/>
		<owl:imports rdf:resource="https://www.omg.org/spec/API4KP/api4kp/"/>
		<owl:imports rdf:resource="https://www.omg.org/spec/LCC/Languages/LanguageRepresentation/"/>
		<owl:versionIRI rdf:resource="https://www.omg.org/spec/API4KP/SNAPSHOT/api4kp-krr/"/>
	</owl:Ontology>
	
	<owl:Class rdf:about="&dol;Mapping">
	</owl:Class>
	
	<owl:ObjectProperty rdf:about="&dol;usesLanguage">
	</owl:ObjectProperty>
	
	<owl:Class rdf:about="&api4kp-krr;BasicEnvironment">
		<rdfs:subClassOf rdf:resource="&api4kp-krr;FocusedEnvironment"/>
		<rdfs:subClassOf>
			<owl:Restriction>
				<owl:onProperty rdf:resource="&api4kp-krr;hasEnvironmentMapping"/>
				<owl:cardinality rdf:datatype="&xsd;nonNegativeInteger">1</owl:cardinality>
			</owl:Restriction>
		</rdfs:subClassOf>
		<skos:definition>a focused environment having exactly one member</skos:definition>
		<skos:prefLabel>basic environment</skos:prefLabel>
	</owl:Class>
	
	<owl:Class rdf:about="&api4kp-krr;BasicMachinableKnowledgeResource">
		<rdfs:subClassOf rdf:resource="&api4kp;BasicKnowledgeResource"/>
		<owl:disjointWith rdf:resource="&api4kp-krr;CompositeComputableKnowledgeResource"/>
		<owl:equivalentClass>
			<owl:Class>
				<owl:intersectionOf rdf:parseType="Collection">
					<rdf:Description rdf:about="&api4kp-krr;MachinableKnowledgeResource">
					</rdf:Description>
					<owl:Restriction>
						<owl:onProperty rdf:resource="&api4kp;hasStructuringComponent"/>
						<owl:cardinality rdf:datatype="&xsd;nonNegativeInteger">0</owl:cardinality>
					</owl:Restriction>
				</owl:intersectionOf>
			</owl:Class>
		</owl:equivalentClass>
		<skos:altLabel>unstructured (KRR) knowledge resource</skos:altLabel>
		<skos:definition>unstructured native machine readable knowledge resource</skos:definition>
		<skos:example>KE1: the instance of the OWL 2 DL abstract syntax for the latest version of a biomedical ontology from an ontology series KA1 defining observable entities, such as the 2015 international version of the SNOMED-CT knowledge base\footnote{http://browser.ihtsdotools.org/} (see also the definition of Basic Knowledge Asset).
This ontology differs from other versions of the series only in the natural language definitions.</skos:example>
		<skos:note>well-formed, stand-alone formula in the abstract syntax of a machine-readable language</skos:note>
		<skos:prefLabel>basic computable knowledge resource</skos:prefLabel>
		<skos:scopeNote>The use of &quot;basic&quot; in API4KP differs from its usage in DOL - a DOL basic OMS  (ontologies, models and specifications) is a set, and corresponds to a Set-structured piece of knowledge in API4KP.</skos:scopeNote>
	</owl:Class>
	
	<owl:Class rdf:about="&api4kp-krr;CategoricalEnvironment">
		<rdfs:subClassOf rdf:resource="&api4kp-krr;EnvironmentWithIdentities"/>
		<skos:definition>a composable environment with identies whose composition operation is associative</skos:definition>
		<skos:definition>environment with an associative composition operation for mappings, that is closed under composition and contains an identity mapping for every member</skos:definition>
		<skos:prefLabel>categorical environment</skos:prefLabel>
	</owl:Class>
	
	<owl:Class rdf:about="&api4kp-krr;ComposableEnvironment">
		<rdfs:subClassOf rdf:resource="&api4kp-krr;Environment"/>
		<skos:definition>an environment having a composition operation where the composition of its mappings is a mapping of the environment whenever the composition is well-defined</skos:definition>
		<skos:editorialNote>The composition M2 o M1 of two mappings M1 and M2 is well-defined when M1 maps to the same thing that M2 maps from. (The codomain of M1 is the domain of M2).</skos:editorialNote>
		<skos:prefLabel>composable environment</skos:prefLabel>
	</owl:Class>
	
	<owl:Class rdf:about="&api4kp-krr;CompositeComputableKnowledgeResource">
		<rdfs:subClassOf rdf:resource="&api4kp;CompositeKnowledgeResource"/>
		<rdfs:subClassOf>
			<owl:Restriction>
				<owl:onProperty rdf:resource="&api4kp;has-structural-component"/>
				<owl:someValuesFrom rdf:resource="&api4kp-krr;MachinableKnowledgeResource"/>
			</owl:Restriction>
		</rdfs:subClassOf>
		<skos:definition>collection of machine readable knowledge resources, which are not necessarily in the same language and may themselves have structure.</skos:definition>
		<skos:example>KE2: a heterogeneous collection of streaming data and RDF graphs, together with static OWL ontologies and CL texts, and ECA rules describing actions of a CDS</skos:example>
		<skos:example>KE3: the OWL 2 DL ontology series KA1, viewed as a collection of expressions rather than an equivalence class</skos:example>
		<skos:prefLabel>composite (KRR) knowledge resource</skos:prefLabel>
	</owl:Class>
	
	<owl:Class rdf:about="&api4kp-krr;ComputationalComplexityClass">
		<rdfs:subClassOf rdf:resource="&api4kp;DefinedConcept"/>
		<rdfs:seeAlso>https://complexityzoo.uwaterloo.ca/Complexity_Zoo</rdfs:seeAlso>
		<rdfs:seeAlso>https://en.wikipedia.org/wiki/List_of_complexity_classes</rdfs:seeAlso>
		<skos:definition>abstraction that relates the size of a problem to the amount of resources (space and time) needed to solve the problem using a given algorithm</skos:definition>
		<skos:prefLabel>computational complexity class</skos:prefLabel>
	</owl:Class>
	
	<owl:Class rdf:about="&api4kp-krr;EmptyEnvironment">
		<rdfs:subClassOf rdf:resource="&api4kp-krr;Environment"/>
		<rdfs:subClassOf>
			<owl:Restriction>
				<owl:onProperty rdf:resource="&api4kp-krr;hasEnvironmentMapping"/>
				<owl:cardinality rdf:datatype="&xsd;nonNegativeInteger">0</owl:cardinality>
			</owl:Restriction>
		</rdfs:subClassOf>
		<owl:disjointWith rdf:resource="&api4kp-krr;NonemptyEnvironment"/>
		<skos:prefLabel>empty environment</skos:prefLabel>
	</owl:Class>
	
	<owl:Class rdf:about="&api4kp-krr;Environment">
		<rdfs:subClassOf rdf:resource="https://www.omg.org/spec/API4KP/api4kp-series/ImmutableEntity"/>
		<skos:definition>mathematical structure of mappings and members, where the domain and codomains of the mappings are members of the environment</skos:definition>
		<skos:example>a KRR language environment containing semantics-preserving translations from RDF and OWL into CL, assisting in the integrated interpretation of a stream of RDF graphs and OWL ontologies</skos:example>
		<skos:prefLabel>environment</skos:prefLabel>
	</owl:Class>
	
	<owl:Class rdf:about="&api4kp-krr;EnvironmentWithIdentities">
		<rdfs:subClassOf rdf:resource="&api4kp-krr;ComposableEnvironment"/>
		<skos:definition>a composable environment having an identity mapping for each member</skos:definition>
		<skos:editorialNote>an identity mapping is a mapping whose domain and codomain are the same, and when composed with another mapping is equal to the original mapping</skos:editorialNote>
		<skos:prefLabel>environment with identity</skos:prefLabel>
	</owl:Class>
	
	<owl:Class rdf:about="&api4kp-krr;FocusedEnvironment">
		<rdfs:subClassOf rdf:resource="&api4kp-krr;NonemptyEnvironment"/>
		<skos:definition>a nonempty environment which has a member F (called the focus or focus member) such that for every other member A, there is a mapping in the environment from A to F</skos:definition>
		<skos:prefLabel>focused environment</skos:prefLabel>
	</owl:Class>
	
	<owl:Class rdf:about="&api4kp-krr;HeterogeneousComputableKnowledgeResource">
		<rdfs:subClassOf rdf:resource="&api4kp-krr;MachinableKnowledgeResource"/>
		<owl:equivalentClass>
			<owl:Class>
				<owl:intersectionOf rdf:parseType="Collection">
					<rdf:Description rdf:about="&api4kp-krr;HeterogeneousKnowledgeResource">
					</rdf:Description>
					<rdf:Description rdf:about="&api4kp-krr;MachinableKnowledgeResource">
					</rdf:Description>
				</owl:intersectionOf>
			</owl:Class>
		</owl:equivalentClass>
		<skos:definition>heterogeneous knowledge resource that uses a machine readable language as primary language</skos:definition>
		<skos:prefLabel>heterogeneous computable knowledge resource</skos:prefLabel>
	</owl:Class>
	
	<owl:Class rdf:about="&api4kp-krr;HeterogeneousKnowledgeResource">
		<owl:equivalentClass>
			<owl:Class>
				<owl:intersectionOf rdf:parseType="Collection">
					<rdf:Description rdf:about="&api4kp;KnowledgeResource">
					</rdf:Description>
					<owl:Restriction>
						<owl:onProperty rdf:resource="&dol;usesLanguage"/>
						<owl:onClass rdf:resource="&lcc-lr;Language"/>
						<owl:minQualifiedCardinality rdf:datatype="&xsd;nonNegativeInteger">2</owl:minQualifiedCardinality>
					</owl:Restriction>
				</owl:intersectionOf>
			</owl:Class>
		</owl:equivalentClass>
		<skos:definition>knowledge resource expressed by means of 2 or more languages</skos:definition>
		<skos:prefLabel>heterogeneous knowledge resource</skos:prefLabel>
	</owl:Class>
	
	<owl:Class rdf:about="&api4kp-krr;HybridKnowledgeBase">
		<rdfs:subClassOf rdf:resource="&api4kp-krr;ImmutableKnowledgeBase"/>
		<rdfs:subClassOf>
			<owl:Restriction>
				<owl:onProperty rdf:resource="&api4kp;manifestedIn"/>
				<owl:someValuesFrom rdf:resource="&api4kp-krr;CompositeComputableKnowledgeResource"/>
			</owl:Restriction>
		</rdfs:subClassOf>
		<skos:definition>A knowledge base composed by multiple parts that have different computational semantics and pragmatics, and thus are likely based on different logics</skos:definition>
		<skos:prefLabel>hybrid knowledge base</skos:prefLabel>
	</owl:Class>
	
	<owl:Class rdf:about="&api4kp-krr;HybridKnowledgeEnvironment">
		<rdfs:subClassOf rdf:resource="&api4kp-krr;CategoricalEnvironment"/>
		<rdfs:subClassOf rdf:resource="&api4kp-krr;LanguageEnvironment"/>
		<rdfs:subClassOf rdf:resource="&api4kp-krr;PreservingEnvironment"/>
		<rdfs:subClassOf>
			<owl:Class>
				<owl:intersectionOf rdf:parseType="Collection">
					<rdf:Description rdf:about="&api4kp-krr;LanguageEnvironment">
					</rdf:Description>
					<owl:Class>
						<owl:complementOf rdf:resource="&api4kp-krr;FocusedEnvironment"/>
					</owl:Class>
				</owl:intersectionOf>
			</owl:Class>
		</rdfs:subClassOf>
		<rdfs:comment>categorical, preserving language environment where multiple KRR languages, and mappings thereof, are supported</rdfs:comment>
		<skos:prefLabel>hybrid knowledge environment</skos:prefLabel>
	</owl:Class>
	
	<owl:Class rdf:about="&api4kp-krr;ImmutableKnowledgeBase">
		<rdfs:subClassOf rdf:resource="&api4kp-krr;KnowledgeBase"/>
		<rdfs:subClassOf rdf:resource="&api4kp;KnowledgeAsset"/>
		<rdfs:comment>An KB can be immutable by nature. Otherwise, any snapshot of a KB at a given point in time (including the time of its creation) is considered immutable.</rdfs:comment>
		<skos:definition>Knowledge Base that is immutable</skos:definition>
		<skos:prefLabel>immutable knowledgebase</skos:prefLabel>
	</owl:Class>
	
	<owl:Class rdf:about="&api4kp-krr;KnowledgeBase">
		<rdfs:subClassOf rdf:resource="&api4kp;WorkOfKnowledge"/>
		<rdfs:comment>A knowledge base is formed by one or more pieces of knowledge, related in different way, such that each piece plays some kind of role.</rdfs:comment>
		<skos:definition>A work of knowledge designed to support reasoning activities</skos:definition>
		<skos:prefLabel>knowledge base</skos:prefLabel>
	</owl:Class>
	
	<owl:Class rdf:about="&api4kp-krr;LanguageEnvironment">
		<rdfs:subClassOf rdf:resource="&api4kp-krr;Environment"/>
		<rdfs:subClassOf>
			<owl:Restriction>
				<owl:onProperty rdf:resource="&api4kp-krr;hasEnvironmentMember"/>
				<owl:allValuesFrom rdf:resource="https://www.omg.org/spec/API4KP/api4kp-lang/KnowledgeRepresentationAndReasoningLanguage"/>
			</owl:Restriction>
		</rdfs:subClassOf>
		<skos:definition>environment whose members are languages</skos:definition>
		<skos:prefLabel>language environment</skos:prefLabel>
	</owl:Class>
	
	<owl:Class rdf:about="&api4kp-krr;MachinableKnowledgeResource">
		<rdfs:subClassOf rdf:resource="&api4kp;KnowledgeResource"/>
		<rdfs:subClassOf>
			<owl:Restriction>
				<owl:onProperty rdf:resource="&dol;usesLanguage"/>
				<owl:someValuesFrom rdf:resource="https://www.omg.org/spec/API4KP/api4kp-lang/MachineReadableLanguage"/>
			</owl:Restriction>
		</rdfs:subClassOf>
		<skos:definition>Set of Expressions in one or more machine readable languages, in the context of a Logical Environment determining how these Expressions are jointly interpreted.</skos:definition>
		<skos:example>Examples;
Example A: OWL Ground fact expressing that Socrates is a philosopher.
Example B: Common Logic sentence expressing that Socrates is a philosopher.
Example C: RDF graph expressing that the author of Moby Dick is Herman Melville.
Example D: SPARQL query for the names of philosphers.

Example E: A and B, together with a mapping that allows OWL to be converted to Common Logic.</skos:example>
		<skos:prefLabel>computable knowledge resource</skos:prefLabel>
	</owl:Class>
	
	<owl:Class rdf:about="&api4kp-krr;MutableKnowledgeBase">
		<rdfs:subClassOf rdf:resource="https://www.omg.org/spec/API4KP/api4kp-series/Series"/>
		<skos:definition>knowledge base that evolves over time as structuring operations are applied to it, &apos;in place&apos;</skos:definition>
		<skos:prefLabel>mutable knowledge base</skos:prefLabel>
	</owl:Class>
	
	<owl:Class rdf:about="&api4kp-krr;NativeComputableKnowledgeResource">
		<owl:equivalentClass>
			<owl:Class>
				<owl:intersectionOf rdf:parseType="Collection">
					<rdf:Description rdf:about="&api4kp-krr;MachinableKnowledgeResource">
					</rdf:Description>
					<rdf:Description rdf:about="&api4kp-krr;NativeKnowledgeResource">
					</rdf:Description>
					<owl:Restriction>
						<owl:onProperty rdf:resource="&dol;usesLanguage"/>
						<owl:onClass rdf:resource="https://www.omg.org/spec/API4KP/api4kp-lang/KnowledgeRepresentationAndReasoningLanguage"/>
						<owl:qualifiedCardinality rdf:datatype="&xsd;nonNegativeInteger">1</owl:qualifiedCardinality>
					</owl:Restriction>
				</owl:intersectionOf>
			</owl:Class>
		</owl:equivalentClass>
		<skos:definition>computable knowledge resource that uses exactly 1 language that is a machine readable language</skos:definition>
		<skos:prefLabel>native computable knowledge resource</skos:prefLabel>
	</owl:Class>
	
	<owl:Class rdf:about="&api4kp-krr;NativeKnowledgeResource">
		<owl:equivalentClass>
			<owl:Class>
				<owl:intersectionOf rdf:parseType="Collection">
					<rdf:Description rdf:about="&api4kp;KnowledgeResource">
					</rdf:Description>
					<owl:Restriction>
						<owl:onProperty rdf:resource="&dol;usesLanguage"/>
						<owl:onClass rdf:resource="&lcc-lr;Language"/>
						<owl:qualifiedCardinality rdf:datatype="&xsd;nonNegativeInteger">1</owl:qualifiedCardinality>
					</owl:Restriction>
				</owl:intersectionOf>
			</owl:Class>
		</owl:equivalentClass>
		<skos:definition>knowledge resource that uses exactly one language</skos:definition>
		<skos:prefLabel>native knowledge resource</skos:prefLabel>
	</owl:Class>
	
	<owl:Class rdf:about="&api4kp-krr;NonemptyEnvironment">
		<rdfs:subClassOf rdf:resource="&api4kp-krr;Environment"/>
		<rdfs:subClassOf>
			<owl:Restriction>
				<owl:onProperty rdf:resource="&api4kp-krr;hasEnvironmentMapping"/>
				<owl:someValuesFrom rdf:resource="&dol;Mapping"/>
			</owl:Restriction>
		</rdfs:subClassOf>
		<skos:prefLabel>nonempty environment</skos:prefLabel>
	</owl:Class>
	
	<owl:Class rdf:about="&api4kp-krr;PivotalKnowledgeEnvironment">
		<rdfs:subClassOf rdf:resource="&api4kp-krr;CategoricalEnvironment"/>
		<rdfs:subClassOf rdf:resource="&api4kp-krr;FocusedEnvironment"/>
		<rdfs:subClassOf rdf:resource="&api4kp-krr;LanguageEnvironment"/>
		<rdfs:subClassOf rdf:resource="&api4kp-krr;PreservingEnvironment"/>
		<skos:definition>focused, categorical, preserving language environment where the focus is a KRR language</skos:definition>
		<skos:prefLabel>pivotal knowledge environment</skos:prefLabel>
		<skos:scopeNote>The special case where all languages in an knowledge environment are KRR languages supporting model-theoretic semantics without side-effects (logics), and the preserving property is characterized by a logical graph reduces to a heterogeneous logical environment as defined in DOL.</skos:scopeNote>
	</owl:Class>
	
	<owl:Class rdf:about="&api4kp-krr;PreservingEnvironment">
		<rdfs:subClassOf rdf:resource="&api4kp-krr;Environment"/>
		<skos:definition>environment where every mapping preserves a specified property</skos:definition>
		<skos:prefLabel>preserving environment</skos:prefLabel>
	</owl:Class>
	
	<owl:ObjectProperty rdf:about="&api4kp-krr;accordingTo">
		<rdfs:range rdf:resource="&api4kp-krr;Environment"/>
		<skos:definition>relationship between a collection and an environment whereby the results of application of a mapping of the environment to a member of the collection are also members of the environment</skos:definition>
		<skos:prefLabel>according to</skos:prefLabel>
	</owl:ObjectProperty>
	
	<owl:ObjectProperty rdf:about="&api4kp-krr;allPreserve">
		<rdfs:domain rdf:resource="&api4kp-krr;PreservingEnvironment"/>
		<skos:prefLabel>all preserve</skos:prefLabel>
	</owl:ObjectProperty>
	
	<owl:ObjectProperty rdf:about="&api4kp-krr;hasEnvironmentMapping">
		<rdfs:range rdf:resource="&dol;Mapping"/>
		<owl:inverseOf rdf:resource="&api4kp-krr;isEnvironmentMappingOf"/>
		<skos:prefLabel>has environment mapping</skos:prefLabel>
	</owl:ObjectProperty>
	
	<owl:ObjectProperty rdf:about="&api4kp-krr;hasEnvironmentMember">
		<rdfs:subPropertyOf rdf:resource="&lcc-lr;hasMember"/>
		<rdfs:domain rdf:resource="&api4kp-krr;NonemptyEnvironment"/>
		<skos:prefLabel>has environment member</skos:prefLabel>
	</owl:ObjectProperty>
	
	<owl:ObjectProperty rdf:about="&api4kp-krr;hasFocusMember">
		<rdfs:subPropertyOf rdf:resource="&api4kp-krr;hasEnvironmentMember"/>
		<skos:prefLabel>has focus member</skos:prefLabel>
	</owl:ObjectProperty>
	
	<owl:ObjectProperty rdf:about="&api4kp-krr;hasSubenvironment">
		<rdfs:subPropertyOf rdf:resource="&api4kp;hasProperPart"/>
		<owl:inverseOf rdf:resource="&api4kp-krr;isSubenvironmentOf"/>
		<skos:prefLabel>has subenvironment</skos:prefLabel>
	</owl:ObjectProperty>
	
	<owl:ObjectProperty rdf:about="&api4kp-krr;isEnvironmentMappingOf">
		<skos:prefLabel>is environment mapping of</skos:prefLabel>
	</owl:ObjectProperty>
	
	<owl:ObjectProperty rdf:about="&api4kp-krr;isSubenvironmentOf">
		<rdfs:subPropertyOf rdf:resource="&api4kp;properPartOf"/>
		<rdfs:domain rdf:resource="&api4kp-krr;Environment"/>
		<rdfs:range rdf:resource="&api4kp-krr;Environment"/>
		<skos:definition>relationship between two environments that is a partial order where the language and logic graphs of the first enviroment are subgraphs, resp., of the language and logic graphs of the second environment</skos:definition>
		<skos:prefLabel xml:lang="en">is subenvironment of</skos:prefLabel>
	</owl:ObjectProperty>
	
	<owl:ObjectProperty rdf:about="&api4kp-krr;preserves">
		<rdfs:subPropertyOf rdf:resource="&api4kp;preserves"/>
		<rdfs:label>preserves</rdfs:label>
		<rdfs:domain rdf:resource="&dol;Mapping"/>
		<owl:propertyChainAxiom rdf:parseType="Collection">
			<rdf:Description rdf:about="&api4kp-krr;isEnvironmentMappingOf">
			</rdf:Description>
			<rdf:Description rdf:about="&api4kp-krr;allPreserve">
			</rdf:Description>
		</owl:propertyChainAxiom>
	</owl:ObjectProperty>
	
	<owl:Class rdf:about="https://www.omg.org/spec/API4KP/api4kp-lang/KnowledgeRepresentationAndReasoningLanguage">
		<rdfs:label>knowledge representation and reasoning language</rdfs:label>
		<skos:definition>OMS language, query language, or result language</skos:definition>
	</owl:Class>
	
	<owl:Class rdf:about="https://www.omg.org/spec/API4KP/api4kp-lang/MachineReadableLanguage">
	</owl:Class>
	
	<owl:Class rdf:about="&api4kp;ComputableKnowledgeArtifact">
		<skos:example>Example: my copy in my Download folder of the encoding in UTF-8 of the serialization in Manchester syntax of an OWL ontology.</skos:example>
	</owl:Class>
	
	<owl:ObjectProperty rdf:about="&api4kp;concisely-expresses">
	</owl:ObjectProperty>
	
	<owl:ObjectProperty rdf:about="&api4kp;has-structural-component">
	</owl:ObjectProperty>
	
	<owl:ObjectProperty rdf:about="&api4kp;preserves">
	</owl:ObjectProperty>

</rdf:RDF>