<?xml version="1.0" encoding="UTF-8"?>
<!DOCTYPE rdf:RDF [
	<!ENTITY api4kp "https://www.omg.org/spec/API4KP/api4kp/">
	<!ENTITY api4kp-kp "https://www.omg.org/spec/API4KP/api4kp-kp/">
	<!ENTITY dct "http://purl.org/dc/terms/">
	<!ENTITY dol "http://www.omg.org/spec/DOL/DOL-terms/">
	<!ENTITY lcc-lr "https://www.omg.org/spec/LCC/Languages/LanguageRepresentation/">
	<!ENTITY owl "http://www.w3.org/2002/07/owl#">
	<!ENTITY rdf "http://www.w3.org/1999/02/22-rdf-syntax-ns#">
	<!ENTITY rdfs "http://www.w3.org/2000/01/rdf-schema#">
	<!ENTITY skos "http://www.w3.org/2004/02/skos/core#">
	<!ENTITY sm "http://www.omg.org/techprocess/ab/SpecificationMetadata/">
	<!ENTITY xsd "http://www.w3.org/2001/XMLSchema#">
]>
<rdf:RDF xml:base="https://www.omg.org/spec/API4KP/api4kp-kp/"
	xmlns:api4kp="https://www.omg.org/spec/API4KP/api4kp/"
	xmlns:api4kp-kp="https://www.omg.org/spec/API4KP/api4kp-kp/"
	xmlns:dct="http://purl.org/dc/terms/"
	xmlns:dol="http://www.omg.org/spec/DOL/DOL-terms/"
	xmlns:lcc-lr="https://www.omg.org/spec/LCC/Languages/LanguageRepresentation/"
	xmlns:owl="http://www.w3.org/2002/07/owl#"
	xmlns:rdf="http://www.w3.org/1999/02/22-rdf-syntax-ns#"
	xmlns:rdfs="http://www.w3.org/2000/01/rdf-schema#"
	xmlns:skos="http://www.w3.org/2004/02/skos/core#"
	xmlns:sm="http://www.omg.org/techprocess/ab/SpecificationMetadata/"
	xmlns:xsd="http://www.w3.org/2001/XMLSchema#">
	
	<owl:Ontology rdf:about="https://www.omg.org/spec/API4KP/api4kp-kp/">
		<rdfs:label>API4KP Ontology of Knowledge Platforms</rdfs:label>
		<dct:abstract>This ontology formalizes the notion of a Knowledge Platform.</dct:abstract>
		<dct:creator>Davide Sottara (sottara.davide at mayo.edu)</dct:creator>
		<dct:license rdf:datatype="&xsd;anyURI">http://opensource.org/licenses/MIT</dct:license>
		<sm:contentLanguage rdf:datatype="&xsd;anyURI">https://www.w3.org/TR/owl2-quick-reference/</sm:contentLanguage>
		<sm:copyright>Copyright (c) 2014-2020 Athan Services</sm:copyright>
		<sm:copyright>Copyright (c) 2014-2020 Fraunhofer Gesellschaft</sm:copyright>
		<sm:copyright>Copyright (c) 2014-2020 Freie Universität Berlin</sm:copyright>
		<sm:copyright>Copyright (c) 2014-2020 Mayo Foundation for Medical Education and Research (MFMER)</sm:copyright>
		<sm:copyright>Copyright (c) 2014-2020 Thematix Partners LLC</sm:copyright>
		<sm:copyright>Copyright (c) 2015-2020 Object Management Group, Inc.</sm:copyright>
		<sm:copyright>Copyright (c) 2019-2020 Universität Leipzig</sm:copyright>
		<sm:copyright>Copyright (c) 2020 Micro Focus</sm:copyright>
		<sm:dependsOn rdf:datatype="&xsd;anyURI">https://www.omg.org/spec/API4KP/api4kp/</sm:dependsOn>
		<sm:dependsOn rdf:datatype="&xsd;anyURI">https://www.omg.org/spec/DOL/</sm:dependsOn>
		<sm:dependsOn rdf:datatype="&xsd;anyURI">https://www.omg.org/spec/LCC/</sm:dependsOn>
		<sm:fileAbbreviation>api4kp-kp</sm:fileAbbreviation>
		<sm:filename>api4kp-kp.rdf</sm:filename>
		<owl:imports rdf:resource="http://www.omg.org/techprocess/ab/SpecificationMetadata/"/>
		<owl:imports rdf:resource="https://www.omg.org/spec/API4KP/api4kp/"/>
		<owl:imports rdf:resource="https://www.omg.org/spec/DOL/20171106/DOL-terms.rdf"/>
		<owl:imports rdf:resource="https://www.omg.org/spec/LCC/Languages/LanguageRepresentation/"/>
		<owl:versionIRI rdf:resource="https://www.omg.org/spec/API4KP/SNAPSHOT/api4kp-kp/"/>
	</owl:Ontology>
	
	<owl:Class rdf:about="&api4kp-kp;Algorithm">
		<rdfs:subClassOf rdf:resource="&api4kp;WorkOfKnowledge"/>
		<rdfs:label>algorithm</rdfs:label>
		<skos:definition>finite sequence of well-defined, computer-implementable instructions, typically to solve a class of problems or to perform a computation</skos:definition>
	</owl:Class>
	
	<owl:Class rdf:about="&api4kp-kp;ComputerProgram">
		<rdfs:subClassOf rdf:resource="&api4kp;KnowledgeExpression"/>
		<rdfs:label>computer program</rdfs:label>
		<skos:definition>the expression of an algorithm in some programming language</skos:definition>
	</owl:Class>
	
	<owl:Class rdf:about="&api4kp-kp;ComputingEnvironment">
		<rdfs:subClassOf>
			<owl:Restriction>
				<owl:onProperty rdf:resource="&api4kp-kp;hosts"/>
				<owl:someValuesFrom rdf:resource="&api4kp-kp;DeployedSoftware"/>
			</owl:Restriction>
		</rdfs:subClassOf>
		<rdfs:label>computing environment</rdfs:label>
		<skos:definition>combination of general purpose hardware and software designed to interpret programs that drive the execution of information processing tasks</skos:definition>
		<skos:scopeNote>includes physical and virtual machines, operating systems, containers and other computing platform/infrastructure components</skos:scopeNote>
	</owl:Class>
	
	<owl:Class rdf:about="&api4kp-kp;DeployedSoftware">
		<rdfs:subClassOf rdf:resource="&api4kp;ArtificialAgent"/>
		<rdfs:subClassOf>
			<owl:Restriction>
				<owl:onProperty rdf:resource="&api4kp-kp;isDeploymentOf"/>
				<owl:someValuesFrom rdf:resource="&api4kp-kp;Software"/>
			</owl:Restriction>
		</rdfs:subClassOf>
		<rdfs:subClassOf>
			<owl:Restriction>
				<owl:onProperty rdf:resource="&api4kp;performs"/>
				<owl:someValuesFrom rdf:resource="&api4kp-kp;SoftwareExecution"/>
			</owl:Restriction>
		</rdfs:subClassOf>
		<rdfs:label>deployed software</rdfs:label>
		<skos:altLabel>deployed software module</skos:altLabel>
		<skos:definition>the result of installing a particular software application or agent into some computing environment</skos:definition>
	</owl:Class>
	
	<owl:Class rdf:about="&api4kp-kp;DescriptionLogicReasoner">
		<rdfs:subClassOf rdf:resource="&api4kp-kp;Reasoner"/>
		<rdfs:label>description logic reasoner</rdfs:label>
		<skos:definition>reasoner optimized for logic based classification, subsumption and query answering tasks that conforms to one or more description logic(s)</skos:definition>
	</owl:Class>
	
	<owl:Class rdf:about="&api4kp-kp;KnowledgeBasedExecution">
		<rdfs:subClassOf rdf:resource="&api4kp-kp;SoftwareExecution"/>
		<rdfs:label>knowledge based execution</rdfs:label>
		<skos:definition>software execution that uses and/or generates some knowledge artfact</skos:definition>
	</owl:Class>
	
	<owl:Class rdf:about="&api4kp-kp;KnowledgePlatform">
		<rdfs:subClassOf rdf:resource="&api4kp-kp;ComputingEnvironment"/>
		<rdfs:label>knowledge platform</rdfs:label>
		<owl:equivalentClass>
			<owl:Class>
				<owl:intersectionOf rdf:parseType="Collection">
					<rdf:Description rdf:about="&api4kp-kp;ComputingEnvironment">
					</rdf:Description>
					<owl:Restriction>
						<owl:onProperty rdf:resource="&api4kp-kp;hosts"/>
						<owl:someValuesFrom>
							<owl:Class>
								<owl:intersectionOf rdf:parseType="Collection">
									<rdf:Description rdf:about="&api4kp-kp;KnowledgePlatformModule">
									</rdf:Description>
									<owl:Restriction>
										<owl:onProperty rdf:resource="&api4kp;performs"/>
										<owl:someValuesFrom rdf:resource="&api4kp;KnowledgeProcessingActivity"/>
									</owl:Restriction>
								</owl:intersectionOf>
							</owl:Class>
						</owl:someValuesFrom>
					</owl:Restriction>
				</owl:intersectionOf>
			</owl:Class>
		</owl:equivalentClass>
		<skos:definition>computing environment designed to host reasoners, and consume knowledge artifacts</skos:definition>
	</owl:Class>
	
	<owl:Class rdf:about="&api4kp-kp;KnowledgePlatformModule">
		<rdfs:subClassOf rdf:resource="&api4kp-kp;DeployedSoftware"/>
		<rdfs:subClassOf>
			<owl:Restriction>
				<owl:onProperty rdf:resource="&api4kp;internallyRepresents"/>
				<owl:someValuesFrom rdf:resource="&api4kp;KnowledgeResource"/>
			</owl:Restriction>
		</rdfs:subClassOf>
		<rdfs:subClassOf>
			<owl:Restriction>
				<owl:onProperty rdf:resource="&api4kp;isProperPartOf"/>
				<owl:someValuesFrom rdf:resource="&api4kp-kp;KnowledgePlatform"/>
			</owl:Restriction>
		</rdfs:subClassOf>
		<rdfs:subClassOf>
			<owl:Restriction>
				<owl:onProperty rdf:resource="&api4kp;performs"/>
				<owl:someValuesFrom rdf:resource="&api4kp-kp;KnowledgeBasedExecution"/>
			</owl:Restriction>
		</rdfs:subClassOf>
		<rdfs:label>knowledge platform module</rdfs:label>
		<skos:definition>deployed software component that is part of a knowledge platform and performs knowledge-based tasks</skos:definition>
	</owl:Class>
	
	<owl:Class rdf:about="&api4kp-kp;ProcessEngine">
		<rdfs:subClassOf rdf:resource="&api4kp-kp;Reasoner"/>
		<rdfs:label>process engine</rdfs:label>
		<skos:definition>reasoner that supports stateful, temporal reasoning centered on tasks, roles and events</skos:definition>
	</owl:Class>
	
	<owl:Class rdf:about="&api4kp-kp;ProductionRuleEngine">
		<rdfs:subClassOf rdf:resource="&api4kp-kp;RuleEngine"/>
		<rdfs:label>production rule engine</rdfs:label>
		<skos:definition>rule engine optimized for production (condition-action) rules</skos:definition>
	</owl:Class>
	
	<owl:Class rdf:about="&api4kp-kp;Reasoner">
		<rdfs:subClassOf rdf:resource="&api4kp-kp;Software"/>
		<rdfs:label>reasoner</rdfs:label>
		<rdfs:comment>software that has the capability of performing reasoning operations</rdfs:comment>
		<skos:altLabel>reasoning engine</skos:altLabel>
	</owl:Class>
	
	<owl:Class rdf:about="&api4kp-kp;RuleEngine">
		<rdfs:subClassOf rdf:resource="&api4kp-kp;Reasoner"/>
		<rdfs:label>rule engine</rdfs:label>
		<skos:definition>reasoner that supports inferences performed on rule bases</skos:definition>
	</owl:Class>
	
	<owl:Class rdf:about="&api4kp-kp;Server">
		<rdfs:subClassOf rdf:resource="&api4kp-kp;DeployedSoftware"/>
		<rdfs:label>server</rdfs:label>
		<skos:definition>deployed software that can perform computations as a service, on a client&apos;s request</skos:definition>
	</owl:Class>
	
	<owl:Class rdf:about="&api4kp-kp;Software">
		<rdfs:subClassOf rdf:resource="&api4kp;KnowledgeArtifact"/>
		<rdfs:label>software</rdfs:label>
		<skos:definition>distributable application or library that carries a computer program</skos:definition>
	</owl:Class>
	
	<owl:Class rdf:about="&api4kp-kp;SoftwareExecution">
		<rdfs:subClassOf rdf:resource="&api4kp;KnowledgeProcessingActivity"/>
		<rdfs:label>software execution</rdfs:label>
		<rdfs:comment>The process by which a (virtual) machine interpretes and executes the instructions that are fragments of a computer program.</rdfs:comment>
		<skos:altLabel>software run</skos:altLabel>
		<skos:scopeNote>at a minimum, a software execution is a knowledge processing activity in the sense that the computing machine follows the &quot;plan&quot; stated by the computer program</skos:scopeNote>
	</owl:Class>
	
	<owl:ObjectProperty rdf:about="&api4kp-kp;hosts">
		<rdfs:label>hosts</rdfs:label>
		<rdfs:domain rdf:resource="&api4kp-kp;ComputingEnvironment"/>
		<rdfs:range rdf:resource="&api4kp-kp;DeployedSoftware"/>
		<skos:definition>relationship between an execution environment, and a software component that has been launched and/or deployed in that environment</skos:definition>
	</owl:ObjectProperty>
	
	<owl:ObjectProperty rdf:about="&api4kp-kp;isDeploymentOf">
		<rdfs:label>is deployment of</rdfs:label>
		<rdfs:domain rdf:resource="&api4kp-kp;DeployedSoftware"/>
		<rdfs:range rdf:resource="&api4kp-kp;Software"/>
		<skos:definition>relationship between a a software component that has been launched and/or deployed in some environment and its basic form</skos:definition>
	</owl:ObjectProperty>

</rdf:RDF>