<?xml version="1.0" encoding="UTF-8"?>
<!DOCTYPE rdf:RDF [
	<!ENTITY AnnotationVocabulary "https://www.omg.org/spec/EDMC-FIBO/FND/Utilities/AnnotationVocabulary/">
	<!ENTITY AnnotationVocabulary1 "http://www.omg.org/spec/EDMC-FIBO/FND/Utilities/AnnotationVocabulary/">
	<!ENTITY api4kp "https://www.omg.org/spec/API4KP/api4kp/">
	<!ENTITY api4kp-rel "https://www.omg.org/spec/API4KP/api4kp-rel/">
	<!ENTITY dct "http://purl.org/dc/terms/">
	<!ENTITY dol "http://www.omg.org/spec/DOL/DOL-terms/">
	<!ENTITY lcc-lr "https://www.omg.org/spec/LCC/Languages/LanguageRepresentation/">
	<!ENTITY olex "http://www.w3.org/ns/lemon/ontolex#">
	<!ENTITY owl "http://www.w3.org/2002/07/owl#">
	<!ENTITY rdf "http://www.w3.org/1999/02/22-rdf-syntax-ns#">
	<!ENTITY rdfs "http://www.w3.org/2000/01/rdf-schema#">
	<!ENTITY skos "http://www.w3.org/2004/02/skos/core#">
	<!ENTITY sm "http://www.omg.org/techprocess/ab/SpecificationMetadata/">
	<!ENTITY xsd "http://www.w3.org/2001/XMLSchema#">
]>
<rdf:RDF xml:base="https://www.omg.org/spec/API4KP/api4kp-rel/"
	xmlns="https://www.omg.org/spec/API4KP/api4kp-rel/"
	xmlns:AnnotationVocabulary="https://www.omg.org/spec/EDMC-FIBO/FND/Utilities/AnnotationVocabulary/"
	xmlns:AnnotationVocabulary1="http://www.omg.org/spec/EDMC-FIBO/FND/Utilities/AnnotationVocabulary/"
	xmlns:api4kp="https://www.omg.org/spec/API4KP/api4kp/"
	xmlns:api4kp-rel="https://www.omg.org/spec/API4KP/api4kp-rel/"
	xmlns:dct="http://purl.org/dc/terms/"
	xmlns:dol="http://www.omg.org/spec/DOL/DOL-terms/"
	xmlns:lcc-lr="https://www.omg.org/spec/LCC/Languages/LanguageRepresentation/"
	xmlns:olex="http://www.w3.org/ns/lemon/ontolex#"
	xmlns:owl="http://www.w3.org/2002/07/owl#"
	xmlns:rdf="http://www.w3.org/1999/02/22-rdf-syntax-ns#"
	xmlns:rdfs="http://www.w3.org/2000/01/rdf-schema#"
	xmlns:skos="http://www.w3.org/2004/02/skos/core#"
	xmlns:sm="http://www.omg.org/techprocess/ab/SpecificationMetadata/"
	xmlns:xsd="http://www.w3.org/2001/XMLSchema#">
	
	<owl:Ontology rdf:about="https://www.omg.org/spec/API4KP/api4kp-rel/">
		<rdfs:label>API4KP Ontology of Knowledge Resources Relationships</rdfs:label>
		<dct:abstract>A module of the API4KP ontology that focuses on relationships between Knowledge Resources</dct:abstract>
		<dct:creator>Davide Sottara (sottara.davide at mayo.edu)</dct:creator>
		<dct:license rdf:datatype="&xsd;anyURI">http://opensource.org/licenses/MIT</dct:license>
		<sm:contentLanguage rdf:datatype="&xsd;anyURI">http://www.w3.org/standards/techs/owl#w3c_all</sm:contentLanguage>
		<sm:copyright>Copyright (c) 2014-2020 88 Solutions</sm:copyright>
		<sm:copyright>Copyright (c) 2014-2020 Adaptive</sm:copyright>
		<sm:copyright>Copyright (c) 2014-2020 Arizona State University</sm:copyright>
		<sm:copyright>Copyright (c) 2014-2020 Athan Services</sm:copyright>
		<sm:copyright>Copyright (c) 2014-2020 Fraunhofer FOKUS</sm:copyright>
		<sm:copyright>Copyright (c) 2014-2020 Freie Universitat Berlin</sm:copyright>
		<sm:copyright>Copyright (c) 2014-2020 Mayo Clinic</sm:copyright>
		<sm:copyright>Copyright (c) 2014-2020 Model Driven Solutions</sm:copyright>
		<sm:copyright>Copyright (c) 2014-2020 Thematix Partners LLC</sm:copyright>
		<sm:copyright>Copyright (c) 2015-2020 Object Management Group, Inc.</sm:copyright>
		<sm:copyright>Copyright (c) 2019-2020 Micro Focus</sm:copyright>
		<sm:dependsOn rdf:datatype="&xsd;anyURI">https://www.omg.org/spec/API4KP/api4kp/</sm:dependsOn>
		<sm:fileAbbreviation>api4kp-rel</sm:fileAbbreviation>
		<sm:filename>api4kp-rel.rdf</sm:filename>
		<owl:imports rdf:resource="http://www.omg.org/spec/DOL/20171101/DOL-terms/"/>
		<owl:imports rdf:resource="http://www.omg.org/techprocess/ab/SpecificationMetadata/"/>
		<owl:imports rdf:resource="https://www.omg.org/spec/API4KP/SNAPSHOT/api4kp/"/>
		<owl:imports rdf:resource="https://www.omg.org/spec/LCC/Languages/LanguageRepresentation/"/>
		<owl:versionIRI rdf:resource="https://www.omg.org/spec/API4KP/SNAPSHOT/api4kp-rel/"/>
	</owl:Ontology>
	
	<owl:AnnotationProperty rdf:about="&skos;altLabel">
	</owl:AnnotationProperty>
	
	<owl:AnnotationProperty rdf:about="&skos;definition">
	</owl:AnnotationProperty>
	
	<owl:AnnotationProperty rdf:about="&skos;note">
	</owl:AnnotationProperty>
	
	<owl:AnnotationProperty rdf:about="&skos;scopeNote">
	</owl:AnnotationProperty>
	
	<owl:ObjectProperty rdf:about="&api4kp-rel;abridges">
		<rdfs:subPropertyOf rdf:resource="&api4kp;abbreviates"/>
		<rdfs:comment>the expression is &apos;minimal&apos; in the sense that no fragment can be removed while still realizing the same knowledge asset</rdfs:comment>
		<skos:definition>is a minimal expression that preserves, or allows to reconstruct by inference, all the concepts used by the target expression</skos:definition>
		<skos:prefLabel>abridges</skos:prefLabel>
	</owl:ObjectProperty>
	
	<owl:ObjectProperty rdf:about="&api4kp-rel;compendiates">
		<rdfs:subPropertyOf rdf:resource="&api4kp-rel;summarizes"/>
		<skos:definition>summarizes using a minimum number of fragments, and only uses concepts that are most closely related to the main subject</skos:definition>
		<skos:prefLabel>compendiates</skos:prefLabel>
	</owl:ObjectProperty>
	
	<owl:ObjectProperty rdf:about="&api4kp-rel;conformsWith">
		<rdfs:subPropertyOf rdf:resource="&api4kp-rel;isComplementedBy"/>
		<skos:definition>satisfies the constraints in the target resource</skos:definition>
		<skos:prefLabel>conforms with</skos:prefLabel>
		<skos:scopeNote>the compliant resource is supposed to be, express or carry some kind of specification</skos:scopeNote>
	</owl:ObjectProperty>
	
	<owl:ObjectProperty rdf:about="&api4kp-rel;effectuates">
		<rdfs:subPropertyOf rdf:resource="&api4kp-rel;isComplementedBy"/>
		<rdfs:label>effectuates</rdfs:label>
		<rdfs:comment>the knowledge of the products can be used to predict and validate what the products will look like</rdfs:comment>
		<skos:definition>is used in activities that generate entities of which the target resource is knowledge of</skos:definition>
	</owl:ObjectProperty>
	
	<owl:ObjectProperty rdf:about="&api4kp-rel;imports">
		<rdfs:subPropertyOf rdf:resource="&api4kp-rel;isSupplementedBy"/>
		<rdfs:subPropertyOf rdf:resource="&api4kp-rel;references"/>
		<rdfs:label>imports</rdfs:label>
		<skos:definition>references a (part of a) supplemental knowledge resource, with the expectation that some structuring operation is performed to resolve the dependency before this resource is used</skos:definition>
	</owl:ObjectProperty>
	
	<owl:ObjectProperty rdf:about="&api4kp-rel;includesByReference">
		<rdfs:subPropertyOf rdf:resource="&api4kp-rel;imports"/>
		<rdfs:comment>inclusions must be resolved, and the resolution of the dependency does not preserve the identity of the target resource</rdfs:comment>
		<rdfs:domain rdf:resource="&api4kp;KnowledgeExpression"/>
		<rdfs:range rdf:resource="&api4kp;KnowledgeExpression"/>
		<skos:definition>imports a resource that is a necessary supplement, and expects that that resource is injected into itself</skos:definition>
		<skos:prefLabel>includes by reference</skos:prefLabel>
	</owl:ObjectProperty>
	
	<owl:ObjectProperty rdf:about="&api4kp-rel;isComplementedBy">
		<rdfs:subPropertyOf rdf:resource="&api4kp;dependsOn"/>
		<skos:definition>optional dependency on a resource whose availability is beneficial</skos:definition>
		<skos:prefLabel>is complemented by</skos:prefLabel>
	</owl:ObjectProperty>
	
	<owl:ObjectProperty rdf:about="&api4kp-rel;isCompressionOf">
		<rdfs:subPropertyOf rdf:resource="&api4kp;abbreviates"/>
		<skos:definition>uses a minimal subset of the fragments and/or symbols of the target expression while trying to maximize the concepts used by both expressions</skos:definition>
		<skos:prefLabel>is compression of</skos:prefLabel>
	</owl:ObjectProperty>
	
	<owl:ObjectProperty rdf:about="&api4kp-rel;isDigestOf">
		<rdfs:subPropertyOf rdf:resource="&api4kp-rel;summarizes"/>
		<rdfs:range rdf:resource="&api4kp;CompositeKnowledgeResource"/>
		<skos:definition>summarizes a composite resource having fragments that summarize each one of the components</skos:definition>
		<skos:prefLabel>is digest of</skos:prefLabel>
	</owl:ObjectProperty>
	
	<owl:ObjectProperty rdf:about="&api4kp-rel;isIsomorphicVariantOf">
		<rdf:type rdf:resource="&owl;SymmetricProperty"/>
		<rdf:type rdf:resource="&owl;TransitiveProperty"/>
		<rdfs:subPropertyOf rdf:resource="&api4kp;isVariantOf"/>
		<rdfs:domain>
			<owl:Class>
				<owl:intersectionOf rdf:parseType="Collection">
					<rdf:Description rdf:about="&api4kp;CompositeKnowledgeResource">
					</rdf:Description>
					<owl:Class>
						<owl:unionOf rdf:parseType="Collection">
							<rdf:Description rdf:about="&api4kp;KnowledgeArtifact">
							</rdf:Description>
							<rdf:Description rdf:about="&api4kp;KnowledgeExpression">
							</rdf:Description>
						</owl:unionOf>
					</owl:Class>
				</owl:intersectionOf>
			</owl:Class>
		</rdfs:domain>
		<rdfs:range>
			<owl:Class>
				<owl:intersectionOf rdf:parseType="Collection">
					<rdf:Description rdf:about="&api4kp;CompositeKnowledgeResource">
					</rdf:Description>
					<owl:Class>
						<owl:unionOf rdf:parseType="Collection">
							<rdf:Description rdf:about="&api4kp;KnowledgeArtifact">
							</rdf:Description>
							<rdf:Description rdf:about="&api4kp;KnowledgeExpression">
							</rdf:Description>
						</owl:unionOf>
					</owl:Class>
				</owl:intersectionOf>
			</owl:Class>
		</rdfs:range>
		<skos:definition>has the same components, but a different configuration</skos:definition>
		<skos:prefLabel>is isomorphic variant of</skos:prefLabel>
	</owl:ObjectProperty>
	
	<owl:ObjectProperty rdf:about="&api4kp-rel;isLosslessCompressionOf">
		<rdfs:subPropertyOf rdf:resource="&api4kp-rel;isCompressionOf"/>
		<skos:definition>compression that preserves all the concepts used by the target expression, or allows to reconstruct them by inference</skos:definition>
		<skos:prefLabel>is lossless compression of</skos:prefLabel>
	</owl:ObjectProperty>
	
	<owl:ObjectProperty rdf:about="&api4kp-rel;isRearrangementOf">
		<rdf:type rdf:resource="&owl;SymmetricProperty"/>
		<rdf:type rdf:resource="&owl;TransitiveProperty"/>
		<rdfs:subPropertyOf rdf:resource="&api4kp-rel;isIsomorphicVariantOf"/>
		<rdfs:domain>
			<owl:Class>
				<owl:intersectionOf rdf:parseType="Collection">
					<rdf:Description rdf:about="&api4kp;CompositeKnowledgeResource">
					</rdf:Description>
					<owl:Class>
						<owl:unionOf rdf:parseType="Collection">
							<rdf:Description rdf:about="&api4kp;KnowledgeArtifact">
							</rdf:Description>
							<rdf:Description rdf:about="&api4kp;KnowledgeExpression">
							</rdf:Description>
						</owl:unionOf>
					</owl:Class>
				</owl:intersectionOf>
			</owl:Class>
		</rdfs:domain>
		<rdfs:range>
			<owl:Class>
				<owl:intersectionOf rdf:parseType="Collection">
					<rdf:Description rdf:about="&api4kp;CompositeKnowledgeResource">
					</rdf:Description>
					<owl:Class>
						<owl:unionOf rdf:parseType="Collection">
							<rdf:Description rdf:about="&api4kp;KnowledgeArtifact">
							</rdf:Description>
							<rdf:Description rdf:about="&api4kp;KnowledgeExpression">
							</rdf:Description>
						</owl:unionOf>
					</owl:Class>
				</owl:intersectionOf>
			</owl:Class>
		</rdfs:range>
		<skos:definition>derived by means of an operation that preserved the structural components, but altered the structure</skos:definition>
		<skos:prefLabel>is rearrangement of</skos:prefLabel>
	</owl:ObjectProperty>
	
	<owl:ObjectProperty rdf:about="&api4kp-rel;isSupplementedBy">
		<rdfs:subPropertyOf rdf:resource="&api4kp;dependsOn"/>
		<rdfs:label>supplements</rdfs:label>
		<rdfs:comment>supplemental dependencies may be mandatory if their lack of availabliity makes the use of the depending resource impossible</rdfs:comment>
		<skos:definition>dependency on a resource whose lack of availability is detrimental</skos:definition>
		<skos:prefLabel>is supplemented by</skos:prefLabel>
	</owl:ObjectProperty>
	
	<owl:ObjectProperty rdf:about="&api4kp-rel;references">
		<rdfs:subPropertyOf rdf:resource="&api4kp;dependsOn"/>
		<rdfs:comment>has at least one proper, identifiable part (e.g. concept, fragment) that is related to a (part of) a different knowledge resource, but not to (part of) the same resource</rdfs:comment>
		<skos:prefLabel>references</skos:prefLabel>
	</owl:ObjectProperty>
	
	<owl:ObjectProperty rdf:about="&api4kp-rel;summarizes">
		<rdfs:subPropertyOf rdf:resource="&api4kp;abbreviates"/>
		<rdfs:label>summarization of</rdfs:label>
		<rdfs:domain rdf:resource="&api4kp;KnowledgeExpression"/>
		<rdfs:range rdf:resource="&api4kp;KnowledgeExpression"/>
		<skos:definition>uses a subset of the concepts of the target expression</skos:definition>
		<skos:prefLabel>summarizes</skos:prefLabel>
	</owl:ObjectProperty>
	
	<owl:Class rdf:about="&api4kp;AbstractExpression">
	</owl:Class>
	
	<owl:Class rdf:about="&api4kp;CompositeKnowledgeResource">
	</owl:Class>
	
	<owl:Class rdf:about="&api4kp;ConcreteExpression">
	</owl:Class>
	
	<owl:Class rdf:about="&api4kp;EncodedKnowledgeExpression">
	</owl:Class>
	
	<owl:Class rdf:about="&api4kp;KnowledgeExpression">
	</owl:Class>
	
	<owl:Class rdf:about="&api4kp;KnowledgeRepresentation">
	</owl:Class>
	
	<owl:Class rdf:about="&api4kp;KnowledgeResource">
	</owl:Class>
	
	<owl:Class rdf:about="&api4kp;StructuredKnowledgeResource">
	</owl:Class>
	
	<owl:Class rdf:about="&api4kp;WorkOfKnowledge">
	</owl:Class>
	
	<owl:ObjectProperty rdf:about="&api4kp;abbreviates">
		<rdfs:subPropertyOf rdf:resource="&api4kp;associatedTo"/>
		<rdfs:domain rdf:resource="&api4kp;KnowledgeExpression"/>
		<rdfs:range rdf:resource="&api4kp;KnowledgeExpression"/>
		<skos:definition>uses a smaller number of symbols, fragments, and/or concepts than the target expression, while sharing at least subject and topic</skos:definition>
		<skos:prefLabel>abbreviates</skos:prefLabel>
	</owl:ObjectProperty>
	
	<owl:ObjectProperty rdf:about="&api4kp;associatedTo">
		<rdfs:domain rdf:resource="&api4kp;KnowledgeResource"/>
		<rdfs:range rdf:resource="&api4kp;KnowledgeResource"/>
		<skos:definition>generically related to</skos:definition>
		<skos:prefLabel>associated to</skos:prefLabel>
	</owl:ObjectProperty>
	
	<owl:ObjectProperty rdf:about="&api4kp;dependsOn">
		<rdfs:subPropertyOf rdf:resource="&api4kp;associatedTo"/>
		<rdfs:comment>an asset may depend on another asset if the latter is background knowledge that facilitates the understanding of the former.</rdfs:comment>
		<rdfs:domain rdf:resource="&api4kp;KnowledgeResource"/>
		<rdfs:range rdf:resource="&api4kp;KnowledgeResource"/>
		<skos:altLabel>leverages</skos:altLabel>
		<skos:definition>such that its use is impacted by the availability of the target resource</skos:definition>
		<skos:prefLabel xml:lang="en">depends on</skos:prefLabel>
		<skos:scopeNote>includes mandatory vs optional dependencies, named vs type-based dependencies, and early vs late resolution</skos:scopeNote>
	</owl:ObjectProperty>
	
	<rdf:Description rdf:about="&api4kp;hasProperPart">
		<rdfs:subPropertyOf rdf:resource="&api4kp;associatedTo"/>
	</rdf:Description>
	
	<owl:ObjectProperty rdf:about="&api4kp;isAdaptationOf">
		<rdfs:subPropertyOf rdf:resource="&api4kp;isDerivedFrom"/>
		<rdfs:domain rdf:resource="&api4kp;KnowledgeAsset"/>
		<rdfs:range rdf:resource="&api4kp;KnowledgeAsset"/>
		<skos:definition>derivative that shares the same subject as the original, but is modified to facilitate the internalization by a certain class of agents</skos:definition>
		<skos:prefLabel>is adaptation of</skos:prefLabel>
	</owl:ObjectProperty>
	
	<owl:ObjectProperty rdf:about="&api4kp;isDerivedFrom">
		<rdfs:subPropertyOf rdf:resource="&api4kp;associatedTo"/>
		<rdfs:comment>a resource may be a derivative of any number of resources, all which need to contribute at least some concept.</rdfs:comment>
		<rdfs:domain rdf:resource="&api4kp;KnowledgeResource"/>
		<rdfs:range rdf:resource="&api4kp;KnowledgeResource"/>
		<skos:definition>created as the product of an activity that used another resource as an input, and such that some of the concepts used in the input resource ended up being used in this resource</skos:definition>
		<skos:prefLabel>is derived from</skos:prefLabel>
	</owl:ObjectProperty>
	
	<owl:ObjectProperty rdf:about="&api4kp;isFlatteningOf">
		<rdfs:subPropertyOf rdf:resource="&api4kp;isDerivedFrom"/>
		<rdfs:domain rdf:resource="&api4kp;BasicKnowledgeResource"/>
		<rdfs:range rdf:resource="&api4kp;CompositeKnowledgeResource"/>
		<skos:definition>derived through the application of a flattening operator to a Composite resource</skos:definition>
		<skos:prefLabel>is flattening of</skos:prefLabel>
	</owl:ObjectProperty>
	
	<owl:ObjectProperty rdf:about="&api4kp;isParaphraseOf">
		<rdfs:subPropertyOf rdf:resource="&api4kp;isVariantOf"/>
		<rdfs:comment>the abstract semantic graphs that are obtained from the parsing of the expressions are isomorphic</rdfs:comment>
		<rdfs:domain>
			<owl:Class>
				<owl:unionOf rdf:parseType="Collection">
					<rdf:Description rdf:about="&api4kp;AbstractExpression">
					</rdf:Description>
					<rdf:Description rdf:about="&api4kp;ConcreteExpression">
					</rdf:Description>
				</owl:unionOf>
			</owl:Class>
		</rdfs:domain>
		<rdfs:range>
			<owl:Class>
				<owl:unionOf rdf:parseType="Collection">
					<rdf:Description rdf:about="&api4kp;AbstractExpression">
					</rdf:Description>
					<rdf:Description rdf:about="&api4kp;ConcreteExpression">
					</rdf:Description>
				</owl:unionOf>
			</owl:Class>
		</rdfs:range>
		<skos:definition>expresses the same knowledge asset using the same language (and/or serialization) but different terms and/or sentence structure</skos:definition>
		<skos:prefLabel>is paraphrase of</skos:prefLabel>
	</owl:ObjectProperty>
	
	<owl:ObjectProperty rdf:about="&api4kp;isRevisionOf">
		<rdfs:subPropertyOf rdf:resource="&api4kp;isDerivedFrom"/>
		<rdfs:domain rdf:resource="&api4kp;KnowledgeResource"/>
		<rdfs:range rdf:resource="&api4kp;KnowledgeResource"/>
		<skos:definition>derivative that is focused on parts of a knowledge resource whose interpretation no longer holds</skos:definition>
		<skos:prefLabel>is later revision of</skos:prefLabel>
		<skos:scopeNote>revised resources are often treated as new versions, but can also become new resources altogether</skos:scopeNote>
	</owl:ObjectProperty>
	
	<owl:ObjectProperty rdf:about="&api4kp;isTranscodificationOf">
		<rdfs:subPropertyOf rdf:resource="&api4kp;isVariantOf"/>
		<rdfs:domain rdf:resource="&api4kp;EncodedKnowledgeExpression"/>
		<rdfs:range rdf:resource="&api4kp;EncodedKnowledgeExpression"/>
		<skos:definition>expresses the same knowledge asset using the same language, serialization, sentence structure, alphabet, but different encodings</skos:definition>
		<skos:prefLabel>is transcodification of</skos:prefLabel>
		<skos:scopeNote>can be used to relate compressed documents (e.g. ZIPped) and their decompressed counterparts</skos:scopeNote>
	</owl:ObjectProperty>
	
	<owl:ObjectProperty rdf:about="&api4kp;isTranscreationOf">
		<rdfs:subPropertyOf rdf:resource="&api4kp;isAdaptationOf"/>
		<rdfs:domain rdf:resource="&api4kp;KnowledgeAsset"/>
		<rdfs:range rdf:resource="&api4kp;KnowledgeAsset"/>
		<skos:definition>adaptation that changes the formal semantics of some parts of the source asset</skos:definition>
		<skos:prefLabel>is transcreation of</skos:prefLabel>
	</owl:ObjectProperty>
	
	<owl:ObjectProperty rdf:about="&api4kp;isTranscriptionOf">
		<rdfs:subPropertyOf rdf:resource="&api4kp;isVariantOf"/>
		<rdfs:domain rdf:resource="&api4kp;ConcreteExpression"/>
		<rdfs:range rdf:resource="&api4kp;ConcreteExpression"/>
		<skos:definition>expresses the same knowledge asset using the same language, but a different serialization</skos:definition>
		<skos:prefLabel>is transcription of</skos:prefLabel>
	</owl:ObjectProperty>
	
	<owl:ObjectProperty rdf:about="&api4kp;isTranslationOf">
		<rdfs:subPropertyOf rdf:resource="&api4kp;isVariantOf"/>
		<rdfs:domain rdf:resource="&api4kp;AbstractExpression"/>
		<rdfs:range rdf:resource="&api4kp;AbstractExpression"/>
		<skos:definition>expresses the same knowledge asset using a different language</skos:definition>
		<skos:prefLabel>is translation of</skos:prefLabel>
	</owl:ObjectProperty>
	
	<owl:ObjectProperty rdf:about="&api4kp;isTransliterationOf">
		<rdfs:subPropertyOf rdf:resource="&api4kp;isVariantOf"/>
		<rdfs:domain rdf:resource="&api4kp;ConcreteExpression"/>
		<rdfs:range rdf:resource="&api4kp;ConcreteExpression"/>
		<skos:definition>expresses the same knowledge using the same language, serialization, sentence structure, but a different alphabet</skos:definition>
		<skos:prefLabel>is transliteration of</skos:prefLabel>
	</owl:ObjectProperty>
	
	<owl:ObjectProperty rdf:about="&api4kp;isVariantOf">
		<rdf:type rdf:resource="&owl;SymmetricProperty"/>
		<rdf:type rdf:resource="&owl;TransitiveProperty"/>
		<rdfs:subPropertyOf rdf:resource="&api4kp;associatedTo"/>
		<rdfs:domain>
			<owl:Class>
				<owl:unionOf rdf:parseType="Collection">
					<rdf:Description rdf:about="&api4kp;KnowledgeArtifact">
					</rdf:Description>
					<rdf:Description rdf:about="&api4kp;KnowledgeExpression">
					</rdf:Description>
				</owl:unionOf>
			</owl:Class>
		</rdfs:domain>
		<rdfs:range>
			<owl:Class>
				<owl:unionOf rdf:parseType="Collection">
					<rdf:Description rdf:about="&api4kp;KnowledgeArtifact">
					</rdf:Description>
					<rdf:Description rdf:about="&api4kp;KnowledgeExpression">
					</rdf:Description>
				</owl:unionOf>
			</owl:Class>
		</rdfs:range>
		<skos:definition>expresses or carries the same knowledge asset as, but differs in at least one of language, serialization, lexicon, alphabet, encoding, or internal arrangement thereof</skos:definition>
		<skos:prefLabel>is variant of</skos:prefLabel>
	</owl:ObjectProperty>

</rdf:RDF>